# Section 6.1 : Average Function Value

The first application of integrals that we'll take a look at is the average
value of a function. The following fact tells us how to compute this.

**Average Function Value**

> The average value of a continuous function $f(x)$ over the interval $[a, b]$
> is given by,
>
> $$ f_{avg} = \frac{1}{b - a}\int_{a}^{b}{f(x)\, dx} $$

To see a justification of this formula see the
[**Proof of Various Integral
Properties**](https://tutorial.math.lamar.edu/Classes/CalcI/ProofIntProp.aspx#Extras_IntPf_AvgVal)
section of the Extras chapter.

Let's work a couple of quick examples.

---

**Example 1** Determine the average value of each of the following functions on
the given interval.

**(a)** $f(t) = t^2 - 5t + 6\cos(\pi t)$ on $\left[-1, \dfrac{5}{2}\right]$

**Solution**

There's really not a whole lot to do in this problem other than just use the
formula.

$$ f_{avg} = \frac{1}{\frac{5}{2} - (-1)}\int_{-1}^{\frac{5}{2}}{t^2 - 5t + 6\cos(\pi t)\, dt} $$

$$ \quad = \left. \frac{2}{7}\left(\frac{1}{3}t^3 - \frac{5}{2}t^2 + \frac{6}{\pi}\sin(\pi t)\right) \right|_{-1}^{\frac{5}{2}} $$

$$ \quad = \frac{12}{7\pi} - \frac{13}{6} $$

$$ \quad = -1.620993 $$

You caught the substitution needed for the third term right?

Side Note: Paul means this:

$$ u = \cos(\pi t) \quad du = (\pi\sin(\pi t))dt \quad \frac{1}{\pi}du = \sin(\pi)t $$

So, the average value of this function of the given interval is -1.620993.

**(b)** $R(z) = \sin(2z)\mathbf{e}^{1 - \cos(2z)}$ on $[-\pi, \pi]$

**Solution**

Again, not much to do here other than use the formula. Note that the integral
will need the following substitution.

$$ u = 1 - \cos(2z) $$

Here is the average value of this function,

$$ R_{avg} = \frac{1}{\pi - (-\pi)}\int_{-\pi}^{\pi}{\sin(2z)\mathbf{e}^{1 - \cos(2z)}\, dz} $$

$$ \quad = \left. \frac{1}{4\pi}\mathbf{e}^{1 - \cos(2z)} \right|_{-\pi}^{\pi} $$

$$ \quad = 0 $$

So, in this case the average function value is zero. Do not get excited about
getting zero here. It will happen on occasion. In fact, if you look at the graph
of the function on this interval it's not too hard to see that this is the
correct answer.

![image 6.1_1](https://tutorial.math.lamar.edu/Classes/CalcI/AvgFcnValue_Files/image001.gif)

---

There is also a theorem that is related to the average function value.

**The Mean Value Theorem for Integrals**

> If $f(x)$ is a continuous function on $[a, b]$ then there is a number $c$ in
> $[a, b]$ such that,
>
> $$  \int_{a}^{b}{f(x)\, dx} = f(c)(b - a) $$

Note that this is very similar to the
[**Mean Value Theorem**](https://tutorial.math.lamar.edu/Classes/CalcI/MeanValueTheorem.aspx#MVT)
that we saw in the Derivatives Applications chapter. See the
[**Proof of Various
Integral Properties**](https://tutorial.math.lamar.edu/Classes/CalcI/ProofIntProp.aspx#Extras_IntPf_AvgVal)
section of the Extras chapter for the proof.

Note that one way to think of this theorem is the following. First rewrite the
result as,

$$ \frac{1}{b - q}\int_{a}^{b}{f(x)\, dx} = f(c) $$

and from this we can see that this theorem is telling us that there is a number
$a < c < b$ such that $f_{avg} = f(c)$. Or, in other words, if $f(x)$ is a
continuous function then somewhere in $[a, b]$ the function will take on its
average value.

Let's take a quick look at an example using this theorem.

---

**Example 2** Determine the number $c$ that satisfies the Mean Value Theorem for
Integrals for the function $f(x) = x^2 + 3x + 2$ on the interval $[1, 4]$.

**Solution**

First let's notice that the function is a polynomial and so is continuous on the
given interval. This means that we can use the Mean Value Theorem. So, let's do
that.

$$ \int_{1}^{4}{x^2 + 3x + 2\, dx} = \left(c^2 + 3c + 2\right)(4 - 1) $$

$$ \left. \left(\frac{1}{3}x^3 + \frac{3}{2}x^2 + 2x\right) \right|_{1}^{4} = 3\left(c^2 + 3c + 2\right) $$

$$ \frac{99}{2} = 3c^2 + 9c + 6 $$

$$ 0 = 3c^2 + 9c - \frac{87}{2} $$

This is a quadratic equation that we can solve. Using the quadratic formula we
get the following two solutions,

$$ c = \frac{-3 + \sqrt{67}}{2} = 2.593 $$

$$ c = \frac{-3 - \sqrt{67}}{2} = -5.593 $$

Clearly the second number is not in the interval and so that isn't the one that
we’re after. The first however is in the interval and so that’s the number we
want.

Note that it is possible for both numbers to be in the interval so don't expect
only one to be in the interval.

---

## Practice Problems

For problems 1 & 2 determine $f_{avg}$ for the function on the given interval.

**1.** $f(x) = 8x - 3 + 5\mathbf{e}^{2 - x}$ on $[0, 2]$

**Solution**

$$ f_{avg} = \frac{1}{b - a}\int_{a}^{b}{f(x)\, dx} $$

$$ f_{avg} = \frac{1}{2 - 0}\int_{0}^{2}{8x - 3 + 5\mathbf{e}^{2 - x}\, dx} $$

$$ f_{avg} = \frac{1}{2}\int_{0}^{2}{8x - 3 + 5\mathbf{e}^{2 - x}\, dx} $$

$$ u = 2 - x \quad du = (-1)dx \quad \Rightarrow \quad -du = dx $$

$$ x = 0 \quad u = 2 - (0) = 2 $$

$$ x = 2 \quad u = 2 - (2) = 0 $$

$$ \int_{0}^{2}{8x - 3 + 5\mathbf{e}^{2 - x}\, dx} = \int_{0}^{2}{8x - 3\, dx} - 5\int_{2}^{0}{\mathbf{e}^u\, du} $$

$$ \int_{0}^{2}{8x - 3 + 5\mathbf{e}^{2 - x}\, dx} = \left. \left(4x^2 - 3x\right) \right|_{0}^{2} - 5 \left. \left(\mathbf{e}^u\right) \right|_{2}^{0} $$

$$ \int_{0}^{2}{8x - 3 + 5\mathbf{e}^{2 - x}\, dx} = \left(4(2)^2 - 3(2) - \left(4(0)^2 - 3(0)\right)\right)- 5\left(\mathbf{e}^{(0)} - \mathbf{e}^{(2)}\right) $$

$$ \int_{0}^{2}{8x - 3 + 5\mathbf{e}^{2 - x}\, dx} = (10)- 5\left(-\mathbf{e}^2\right) $$

$$ \int_{0}^{2}{8x - 3 + 5\mathbf{e}^{2 - x}\, dx} = 10 + 5\mathbf{e}^2 $$

$$ \int_{0}^{2}{8x - 3 + 5\mathbf{e}^{2 - x}\, dx} = 5\left(2 + \mathbf{e}^2\right) $$

$$ \boxed{f_{avg} = \frac{1}{2}\int_{0}^{2}{8x - 3 + 5\mathbf{e}^{2 - x}\, dx} = \frac{5}{2}\left(2 + \mathbf{e}^2\right)} $$

**2.** $f(x) = \cos(2x) - \sin\left(\dfrac{x}{2}\right)$ on
$\left[-\dfrac{\pi}{2}, \pi\right]$

**Solution**

$$ f_{avg} = \frac{1}{\pi - \left(-\frac{\pi}{2}\right)}\int_{-\frac{\pi}{2}}^{\pi}{\cos(2x) - \sin\left(\frac{x}{2}\right)\, dx} $$

$$ f_{avg} = \frac{2}{3\pi}\int_{-\frac{\pi}{2}}^{\pi}{\cos(2x) - \sin\left(\frac{x}{2}\right)\, dx} $$

$$ u = 2x \quad du = 2dx \quad \Rightarrow \quad \frac{1}{2}du = dx $$

$$ x = -\frac{\pi}{2} \quad u = 2\left(-\frac{\pi}{2}\right) = -\pi  $$

$$ x = \pi \quad u = 2(\pi) = 2\pi $$

$$ v = \frac{x}{2} \quad dv = \left(\frac{1}{2}\right)dx \quad \Rightarrow \quad 2dv = dx $$

$$ x = -\frac{\pi}{2} \quad v = \frac{\left(-\dfrac{\pi}{2}\right)}{2} = -\frac{\pi}{4} $$

$$ x = \pi \quad v = \frac{(\pi)}{2} = \frac{\pi}{2} $$

$$ \int_{-\frac{\pi}{2}}^{\pi}{\cos(2x) - \sin\left(\frac{x}{2}\right)\, dx} = \frac{1}{2}\int_{-\pi}^{2\pi}{\cos(u)\, du} - 2\int_{-\frac{\pi}{4}}^{\frac{\pi}{2}}{\sin(v)\, dv} $$

$$ \quad = \frac{1}{2}\left. \left(\sin(u)\right) \right|_{-\pi}^{2\pi} - 2\left. \left(-\cos(v)\right) \right|_{-\frac{\pi}{4}}^{\frac{\pi}{2}} $$

$$ \quad = \frac{1}{2}\left(\sin(2\pi) - \sin(-\pi)\right) - 2\left(-\cos\left(\frac{\pi}{2}\right) - \left(-\cos\left(-\frac{\pi}{4}\right)\right)\right) $$

$$ \quad = \frac{1}{2}(0 - 0) - 2\left(0 + \frac{1}{\sqrt{2}}\right) $$

$$ \quad = -\frac{2}{\sqrt{2}} = -\sqrt{2} $$

$$ \boxed{f_{avg} = \frac{2}{3\pi}\int_{-\frac{\pi}{2}}^{\pi}{\cos(2x) - \sin\left(\frac{x}{2}\right)\, dx} = \frac{2}{3\pi}\left(-\sqrt{2}\right) = -\frac{2\sqrt{2}}{3\pi}} $$

**3.** Find $f_{avg}$ for $f(x) = 4x^2 - x + 5$ on $[-2, 3]$ and determine the
value(s) of $c$ in $[-2, 3]$ for which $f(c) = f_{avg}$.

**Solution**

$$ \int_{a}^{b}{f(x)\, dx} = f(c)(b - a) $$

Or:

$$ f_{avg} = \frac{1}{b - a}\int_{a}^{b}{f(x)\, dx} = f(c) $$

$$ \frac{1}{3 - (-2)}\int_{-2}^{3}{4x^2 - x + 5\, dx} = \left(4c^2 - c + 5\right) $$

$$ \int_{-2}^{3}{4x^2 - x + 5\, dx} = \left. \frac{4}{3}x^3 - \frac{1}{2}x^2 + 5x \right|_{-2}^{3} $$

$$ \int_{-2}^{3}{4x^2 - x + 5\, dx} = \left[\left(\frac{4}{3}(3)^3 - \frac{1}{2}(3)^2 + 5(3)\right) - \left(\frac{4}{3}(-2)^3 - \frac{1}{2}(-2)^2 + 5(-2)\right)\right] $$

$$ \int_{-2}^{3}{4x^2 - x + 5\, dx} = \left[\left(36 - \frac{9}{2} + 15\right) - \left(-\frac{32}{3} - 2 - 10\right)\right] $$

$$ \int_{-2}^{3}{4x^2 - x + 5\, dx} = 36 - \frac{9}{2} + 15 + \frac{32}{3} + 2 + 10 $$

$$ \int_{-2}^{3}{4x^2 - x + 5\, dx} = \frac{415}{6} $$

$$ f_{avg} = \frac{1}{3 - (-2)}\left(\frac{415}{6}\right) $$

$$ \boxed{f_{avg} = \frac{1}{5}\left(\frac{415}{6}\right) = \frac{83}{6}} $$

$$ \frac{83}{6} = 4c^2 - c + 5 $$

$$ 4c^2 - c + 5 = \frac{83}{6} $$

$$ 4c^2 - c + 5 - \frac{83}{6} = 0 $$

$$ 4c^2 - c - \frac{53}{6} = 0 $$

$$ c = \frac{-(-1) \pm \sqrt{(-1)^2 - 4(4)\left(-\dfrac{53}{6}\right)}}{2(4)} $$

$$ c = \frac{1 \pm \dfrac{\sqrt{1281}}{3}}{8} $$

$$ c = \frac{1}{8} \pm \frac{\sqrt{1281}}{24} $$

$$ c = \frac{1}{8} + \frac{\sqrt{1281}}{24} \approx 1.616294181 $$

$$ c = \frac{1}{8} - \frac{\sqrt{1281}}{24} \approx -1.366294181 $$

Both values for $c$ fall within the given range of $[-2, 3]$, so both values are
our answer:

$$ \boxed{c = \frac{1}{8} \pm \frac{\sqrt{1281}}{24}} $$

---

## Assignment Problems

For problems 1 - 4 determine $f_{avg}$ for the function on the given interval.

**1.** $f(x) = 8x^4 - 7x^3 + 2$ on $[-2, 1]$

**Solution**

$$ f_{avg} = \frac{1}{b - a}\int_{a}^{b}{f(x)\, dx} $$

$$ f_{avg} = \frac{1}{1 - (-2)}\int_{-2}^{1}{8x^4 - 7x^3 + 2\, dx} $$

$$ f_{avg} = \frac{1}{3}\int_{-2}^{1}{8x^4 - 7x^3 + 2\, dx} $$

$$ \int_{-2}^{1}{8x^4 - 7x^3 + 2\, dx} = \left. \left(\frac{8}{5}x^5 - \frac{7}{4}x^4 + 2x\right) \right|_{-2}^{1} $$

$$ \int_{-2}^{1}{8x^4 - 7x^3 + 2\, dx} = \left(\frac{8}{5}(1)^5 - \frac{7}{4}(1)^4 + 2(1)\right) - \left(\frac{8}{5}(-2)^5 - \frac{7}{4}(-2)^4 + 2(-2)\right) $$

$$ \int_{-2}^{1}{8x^4 - 7x^3 + 2\, dx} = \left(\frac{8}{5} - \frac{7}{4} + 2\right) - \left(-\frac{256}{5} - 28 - 4\right) $$

$$ \int_{-2}^{1}{8x^4 - 7x^3 + 2\, dx} = \frac{8}{5} - \frac{7}{4} + 2 + \frac{256}{5} + 28 + 4 $$

$$ \int_{-2}^{1}{8x^4 - 7x^3 + 2\, dx} = \frac{1701}{20} $$

$$ \boxed{f_{avg} = \frac{1}{3}\left(\frac{1701}{20}\right) = \frac{567}{20}} $$

**2.** $f(x) = (4 - x)\mathbf{e}^{x^2 - 8x}$ on $[1, 4]$

**Solution**

$$ f_{avg} = \frac{1}{4 - 1}\int_{1}^{4}{(4 - x)\mathbf{e}^{x^2 - 8x}\, dx} $$

$$ f_{avg} = \frac{1}{3}\int_{1}^{4}{(4 - x)\mathbf{e}^{x^2 - 8x}\, dx} $$

$$ \int_{1}^{4}{(4 - x)\mathbf{e}^{x^2 - 8x}\, dx} $$

$$ u = x^2 - 8x \quad du = (2x - 8)dx = -2(4 - x)dx \quad \Rightarrow \quad -\frac{1}{2}du = (4 - x)dx $$

$$ x = 1 \quad u = (1)^2 - 8(1) = -7 $$

$$ x = 4 \quad u = (4)^2 - 8(4) = -16 $$

$$ \int_{1}^{4}{(4 - x)\mathbf{e}^{x^2 - 8x}\, dx} = -\frac{1}{2}\int_{-7}^{-16}{\mathbf{e}^u\, du} $$

$$ \quad = -\frac{1}{2}\left. \left(\mathbf{e}^u\right) \right|_{-7}^{-16} $$

$$ \quad = -\frac{1}{2}\left(\mathbf{e}^{-16} - \mathbf{e}^{-7}\right) $$

$$ f_{avg} = \frac{1}{3}\left[-\frac{1}{2}\left(\mathbf{e}^{-16} - \mathbf{e}^{-7}\right)\right] $$

$$ \boxed{f_{avg} = -\frac{1}{6}\left(\mathbf{e}^{-16} - \mathbf{e}^{-7}\right)} $$

**3.** $f(x) = 6x - \dfrac{4x}{x^2 + 1}$ on $[-3, 0]$

**Solution**

$$ f_{avg} = \frac{1}{0 - (-3)}\int_{-3}^{0}{6x - \frac{4x}{x^2 + 1}\, dx} $$

$$ f_{avg} = \frac{1}{3}\int_{-3}^{0}{6x - \frac{4x}{x^2 + 1}\, dx} $$

$$ \int_{-3}^{0}{6x - \frac{4x}{x^2 + 1}\, dx} = 6\int_{-3}^{0}{x\, dx} - 4\int_{-3}^{0}{\frac{x}{1 + x^2}\, dx} $$

$$ u = 1 + x^2 \quad du = (2x)dx \quad \frac{1}{2}du = (x)dx $$

$$ x = -3 \quad u = 1 + (-3)^2 = 10 $$

$$ x = 0 \quad u = 1 + (0)^2 = 1 $$

$$ \int_{-3}^{0}{6x - \frac{4x}{x^2 + 1}\, dx} = 6\int_{-3}^{0}{x\, dx} - 2\int_{10}^{1}{\frac{1}{u}\, du} $$

$$ \quad = 6\left. \left(\frac{1}{2}x^2\right) \right|_{-3}^{0} - 2\left. \left(\ln|u|\right) \right|_{10}^{1} $$

$$ \quad = 6\left(\frac{1}{2}(0)^2 - \frac{1}{2}(-3)^2\right) - 2\left(\ln|(1)| - \ln|(10)|\right) $$

$$ \quad = 6\left(-\frac{9}{2}\right) - 2\left(\ln(1) - \ln(10)\right) $$

$$ \quad = -27 - 2\left(0 - \ln(10)\right) $$

$$ \quad = -27 + 2\ln(10) $$

$$ f_{avg} = \frac{1}{3}\left[-27 + 2\ln(10)\right] $$

$$ \boxed{f_{avg} = -9 + \frac{2}{3}\ln(10)} $$

**4.** $f(x) = \cos(3x)\left[2 + \sin(3x)\right]^4$ on
$\left[0, \dfrac{\pi}{6}\right]$

**Solution**

$$ f_{avg} = \frac{1}{\frac{\pi}{6} - 0}\int_{0}^{\frac{\pi}{6}}{\cos(3x)\left[2 + \sin(3x)\right]^4\, dx} $$

$$ f_{avg} = \frac{6}{\pi}\int_{0}^{\frac{\pi}{6}}{\cos(3x)\left[2 + \sin(3x)\right]^4\, dx} $$

$$ \int_{0}^{\frac{\pi}{6}}{\cos(3x)\left[2 + \sin(3x)\right]^4\, dx} $$

$$ u = 2 + \sin(3x) \quad du = 3\cos(3x)dx \quad \Rightarrow \quad \frac{1}{3}du = \cos(3x)dx $$

$$ x = 0 \quad u = 2 + \sin(3(0)) = 2 $$

$$ x = \frac{\pi}{6} \quad u = 2 + \sin\left(3\left(\frac{\pi}{6}\right)\right) = 3 $$

$$ \int_{0}^{\frac{\pi}{6}}{\cos(3x)\left[2 + \sin(3x)\right]^4\, dx} = \frac{1}{3}\int_{2}^{3}{u^4\, du} $$

$$ \quad = \frac{1}{3}\left. \left(\frac{1}{5}u^5\right) \right|_{2}^{3} $$

$$ \quad = \frac{1}{3}\left(\frac{1}{5}(3)^5 - \frac{1}{5}(2)^5\right) $$

$$ \quad = \frac{1}{3}\left(\frac{243}{5} - \frac{32}{5}\right) $$

$$ \quad = \frac{1}{3}\left(\frac{211}{5}\right) $$

$$ \quad = \frac{211}{15} $$

$$ f_{avg} = \frac{6}{\pi}\left(\frac{211}{15}\right) $$

$$ f_{avg} = \frac{1266}{15\pi} $$

$$ \boxed{f_{avg} = \frac{422}{5\pi}} $$

For problems 5 - 8 find $f_{avg}$ for the function on the given interval and
determine the value of $c$ in the given interval for which $f(c) = f_{avg}$.

**5.** $f(x) = 10 - 4x - 6x^2$ on $[2, 6]$

**Solution**

$$ f_{avg} = \frac{1}{b - a}\int_{a}^{b}{f(x)\, dx} = f(c) $$

$$ f_{avg} = \frac{1}{6 - 2}\int_{2}^{6}{10 - 4x - 6x^2\, dx} = 10 - 4c - 6c^2 $$

$$ f_{avg} = \frac{1}{4}\int_{2}^{6}{10 - 4x - 6x^2\, dx} = 10 - 4c - 6c^2 $$

$$ \int_{2}^{6}{10 - 4x - 6x^2\, dx} $$

$$ \int_{2}^{6}{10 - 4x - 6x^2\, dx} = \left. \left(10x - 2x^2 - 2x^3\right) \right|_{2}^{6} $$

$$ \int_{2}^{6}{10 - 4x - 6x^2\, dx} = \left(10(6) - 2(6)^2 - 2(6)^3\right) - \left(10(2) - 2(2)^2 - 2(2)^3\right) $$

$$ \int_{2}^{6}{10 - 4x - 6x^2\, dx} = (60 - 72 - 432) - (20 - 8 - 16) $$

$$ \int_{2}^{6}{10 - 4x - 6x^2\, dx} = 60 - 72 - 432 - 20 + 8 + 16 $$

$$ \int_{2}^{6}{10 - 4x - 6x^2\, dx} = -440 $$

$$ f_{avg} = \frac{1}{4}(-440) $$

$$ f_{avg} = -110 $$

$$ 10 - 4c - 6c^2 = -110 $$

$$ 6c^2 + 4c - 10 = 110 $$

$$ 6c^2 + 4c - 10 - 110 = 0 $$

$$ 6c^2 + 4c - 120 = 0 $$

$$ 3c^2 + 2c - 60 = 0 $$

$$ c = \frac{-(2) \pm \sqrt{(2)^2 - 4(3)(-120)}}{2(3)} $$

$$ c = \frac{-2 \pm 38}{6} $$

$$ c = \frac{-1 \pm 19}{3} $$

$$ c = \frac{-1 - 19}{3} = -\frac{20}{3} \approx -6.666666667 $$

$$ c = \frac{-1 + 19}{3} = 6 $$

Only the second value of $c$ falls within our given range of $[2, 6]$, thusly
this is our answer for the value of $c$:

$$ \boxed{c = \frac{-1 + 19}{3} = 6} $$

**6.** $f(x) = 7x^2 + 2x - 3$ on $[-1, 1]$

**Solution**

$$ f_{avg} = \frac{1}{1 - (-1)}\int_{-1}^{1}{7x^2 + 2x - 3\, dx} = 7c^2 - 2c - 3 $$

$$ f_{avg} = \frac{1}{2}\int_{-1}^{1}{7x^2 + 2x - 3\, dx} = 7c^2 - 2c - 3 $$

$$ \int_{-1}^{1}{7x^2 + 2x - 3\, dx} = \left. \left(\frac{7}{3}x^3 + x^2 - 3x\right) \right|_{-1}^{1} $$

$$ \quad = \left(\frac{7}{3}(1)^3 + (1)^2 - 3(1)\right) - \left(\frac{7}{3}(-1)^3 + (-1)^2 - 3(-1)\right) $$

$$ \quad = \left(\frac{7}{3} + 1 - 3\right) - \left(-\frac{7}{3} + 1 + 3\right) $$

$$ \quad = \frac{7}{3} + 1 - 3 + \frac{7}{3} - 1 - 3 $$

$$ \quad = -\frac{4}{3} $$

$$ f_{avg} = \frac{1}{2}\left(-\frac{4}{3}\right) $$

$$ \boxed{f_{avg} = -\frac{2}{3}} $$

$$ 7c^2 - 2c - 3 = -\frac{2}{3} $$

$$ 7c^2 - 2c - 3 + \frac{2}{3} = 0 $$

$$ 7c^2 - 2c - \frac{7}{3} = 0 $$

$$ c = \frac{-(-2) \pm \sqrt{(-2)^2 - 4(7)\left(-\dfrac{7}{3}\right)}}{2(7)} $$

$$ c = \frac{2 \pm \dfrac{4}{3}\sqrt{39}}{14} $$

$$ c = \frac{1}{7} \pm \frac{4}{3(14)}\sqrt{39} $$

$$ c = \frac{1}{7} \pm \frac{2}{21}\sqrt{39} $$

$$ c = \frac{1}{7} - \frac{2}{21}\sqrt{39} \approx -0.4519045713 $$

$$ c = \frac{1}{7} + \frac{2}{21}\sqrt{39} \approx 0.7376188570 $$

Both of these values for $c$ fall within the given range of $[-1, 1]$, so both
values of $c$ are our answer:

$$ \boxed{c = \frac{1}{7} \pm \frac{2}{21}\sqrt{39}} $$

**7.** $f(x) = 9 - 2\mathbf{e}^{4x + 1}$ on $[-1, 2]$

**Solution**

$$ f_{avg} = \frac{1}{2 - (-1)}\int_{-1}^{2}{9 - 2\mathbf{e}^{4x + 1}\, dx} = 9 - 2\mathbf{e}^{4c + 1} $$

$$ f_{avg} = \frac{1}{3}\int_{-1}^{2}{9 - 2\mathbf{e}^{4x + 1}\, dx} = 9 - 2\mathbf{e}^{4c + 1} $$

$$ \int_{-1}^{2}{9 - 2\mathbf{e}^{4x + 1}\, dx} $$

$$ u = 4x + 1 \quad du = (4)dx \quad \Rightarrow \quad \frac{1}{4}du = dx $$

$$ x = -1 \quad u = 4(-1) + 1 = -3 $$

$$ x = 2 \quad u = 4(2) + 1 = 9 $$

$$ \int_{-1}^{2}{9 - 2\mathbf{e}^{4x + 1}\, dx} = \int_{-1}^{2}{9\, dx} - \frac{1}{2}\int_{-3}^{9}{\mathbf{e}^u\, du} $$

$$ \quad = \left. (9x) \right|_{-1}^{2} - \frac{1}{2}\left. \left(\mathbf{e}^u\right) \right|_{-3}^{9} $$

$$ \quad = \left[9(2) - 9(-1)\right] - \frac{1}{2}\left[\mathbf{e}^{(9)} - \mathbf{e}^{(-3)}\right] $$

$$ \quad = 27 - \frac{1}{2}\left(\mathbf{e}^9 - \mathbf{e}^{-3}\right) $$

$$ f_{avg} = \frac{1}{3}\left[27 - \frac{1}{2}\left(\mathbf{e}^9 - \mathbf{e}^{-3}\right)\right] $$

$$ \boxed{f_{avg} = 9 - \frac{1}{6}\left(\mathbf{e}^9 - \mathbf{e}^{-3}\right)} $$

$$ 9 - 2\mathbf{e}^{4c + 1} = 9 - \frac{1}{6}\left(\mathbf{e}^9 - \mathbf{e}^{-3}\right) $$

$$ -2\mathbf{e}^{4c + 1} = -\frac{1}{6}\left(\mathbf{e}^9 - \mathbf{e}^{-3}\right) $$

$$ \mathbf{e}^{4c + 1} = \frac{1}{12}\left(\mathbf{e}^9 - \mathbf{e}^{-3}\right) $$

$$ 4c + 1 = \ln\left[\frac{1}{12}\left(\mathbf{e}^9 - \mathbf{e}^{-3}\right)\right] $$

$$ c = \frac{\ln\left[\dfrac{1}{12}\left(\mathbf{e}^9 - \mathbf{e}^{-3}\right)\right] - 1}{4} \approx 1.378771801 $$

This value for $c$ lies within the given range of $[-1, 2]$, and so is our
answer for the value of $c$:

$$ \boxed{c = \frac{\ln\left[\dfrac{1}{12}\left(\mathbf{e}^9 - \mathbf{e}^{-3}\right)\right] - 1}{4}} $$

**8.** $f(x) = 8 - \cos\left(\dfrac{x}{4}\right)$ on $[0, 4\pi]$

**Solution**

$$ f_{avg} = \frac{1}{4\pi - 0}\int_{0}^{4\pi}{8 - \cos\left(\frac{x}{4}\right)\, dx} = 8 - \cos\left(\frac{c}{4}\right) $$

$$ f_{avg} = \frac{1}{4\pi}\int_{0}^{4\pi}{8 - \cos\left(\frac{x}{4}\right)\, dx} = 8 - \cos\left(\frac{c}{4}\right) $$

$$ \int_{0}^{4\pi}{8 - \cos\left(\frac{x}{4}\right)\, dx} $$

$$ \int_{0}^{4\pi}{8 - \cos\left(\frac{x}{4}\right)\, dx} = \int_{0}^{4\pi}{8 \, dx} - \int_{0}^{4\pi}{\cos\left(\frac{x}{4}\right)\, dx} $$

$$ u = \frac{x}{4} \quad du = \left(\frac{1}{4}\right)dx \quad \Rightarrow \quad 4du = dx $$

$$ x = 0 \quad u = \frac{(0)}{4} = 0 $$

$$ x = 4\pi \quad u = \frac{(4\pi)}{4} = \pi $$

$$ \int_{0}^{4\pi}{8 - \cos\left(\frac{x}{4}\right)\, dx} = \int_{0}^{4\pi}{8 \, dx} - 4\int_{0}^{\pi}{\cos(u)\, du} $$

$$ \quad = \left. (8x) \right|_{0}^{4\pi} - 4\left. \left(\sin(u)\right) \right|_{0}^{\pi} $$

$$ \quad = (8(4\pi) - 8(0)) - 4\left(\sin(\pi) - \sin(0)\right) $$

$$ \quad = (32\pi) - 4(0 - 0) $$

$$ \quad = 32\pi $$

$$ f_{avg} = \frac{1}{4\pi}(32\pi) $$

$$ \boxed{f_{avg} = 8} $$

$$ 8 - \cos\left(\frac{c}{4}\right) = 8 $$

$$ 8 - \cos\left(\frac{c}{4}\right) - 8 = 0 $$

$$ -\cos\left(\frac{c}{4}\right) = 0 $$

$$ \cos\left(\frac{c}{4}\right) = 0 $$

$$ \frac{c}{4} = \cos^{-1}(0) $$

$$ c = 4\cos^{-1}(0) $$

$$ c = 2\pi $$

And obviously this value for $c$ lies within the given range of $[0, 4\pi]$, so
this is our answer for the value of $c$:

$$ \boxed{c = 2\pi} $$
