# Section 2.6 : Infinite Limits

In this section we will take a look at limits whose value is infinity or minus
infinity. These kinds of limit will show up fairly regularly in later sections
and in other courses and so you’ll need to be able to deal with them when you
run across them.

The first thing we should probably do here is to define just what we mean when
we say that a limit has a value of infinity or minus infinity.

**Definition**

> We say
>
> $$ \lim\limits_{x \to a}f(x) = \infty $$
>
> if we can make $f(x)$ arbitrarily large for all $x$ sufficiently close to
> $x = a$, from both sides, without actually letting $x = a$.
>
> We say
>
> $$ \lim\limits_{x \to a}f(x) = -\infty $$
>
> if we can make $f(x)$ arbitrarily large and negative for all $x$ sufficiently
> close to $x = a$, from both sides, without actually letting $x = a$.

These definitions can be appropriately modified for the one-sided limits as
well. To see a more precise and mathematical definition of this kind of limit
see the
[The Definition of the Limit](https://tutorial.math.lamar.edu/Classes/CalcI/DefnOfLimit.aspx)
section at the end of this chapter.

Let’s start off with a fairly typical example illustrating infinite limits.

---

**Example 1** Evaluate each of the following limits.

$$ \lim\limits_{x \to 0^{+}}\frac{1}{x} \quad \quad \lim\limits_{x \to 0^{-}}\frac{1}{x} \quad \quad \lim\limits_{x \to 0}\frac{1}{x} $$

**Solution**

So, we’re going to be taking a look at a couple of one-sided limits as well as
the normal limit here. In all three cases notice that we can’t just plug in
$x = 0$. If we did we would get division by zero. Also recall that the
definitions above can be easily modified to give similar definitions for the two
one-sided limits which we’ll be needing here.

Now, there are several ways we could proceed here to get values for these
limits. One way is to plug in some points and see what value the function is
approaching. In the preceding section we said that we were no longer going to do
this, but in this case it is a good way to illustrate just what’s going on with
this function.

So, here is a table of values of $x$'s from both the left and the right. Using
these values we’ll be able to estimate the value of the two one-sided limits and
once we have that done we can use the
[fact](https://tutorial.math.lamar.edu/Classes/CalcI/OneSidedLimits.aspx#Limit_Fact)
that the normal limit will exist only if the two one-sided limits exist and have
the same value.

| $x$       | $\dfrac{1}{x}$ | $x$      | $\dfrac{1}{x}$ |
| --------- | -------------- | -------- | -------------- |
| $-0.1$    | $-10$          | $0.1$    | $10$           |
| $-0.01$   | $-100$         | $0.01$   | $100$          |
| $-0.001$  | $-1000$        | $0.001$  | $1000$         |
| $-0.0001$ | $-10000$       | $0.0001$ | $10000$        |

From this table we can see that as we make $x$ smaller and smaller the function
$\frac{1}{x}$ gets larger and larger and will retain the same sign that $x$
originally had. It should make sense that this trend will continue for any
smaller value of $x$ that we chose to use. The function is a constant (one in
this case) divided by an increasingly small number. The resulting fraction
should be an increasingly large number and as noted above the fraction will
retain the same sign as $x$.

We can make the function as large and positive as we want for all $x$'s
sufficiently close to zero while staying positive (_i.e._ on the right).
Likewise, we can make the function as large and negative as we want for all
$x$'s sufficiently close to zero while staying negative (_i.e._ on the left).
So, from our definition above it looks like we should have the following values
for the two one sided limits.

$$ \lim\limits_{x \to 0^{+}}\frac{1}{x} = \infty \quad \quad \lim\limits_{x \to 0^{-}}\frac{1}{x} = -\infty $$

Another way to see the values of the two one sided limits here is to graph the
function. Again, in the previous section we mentioned that we won’t do this too
often as most functions are not something we can just quickly sketch out as well
as the problems with accuracy in reading values off the graph. In this case
however, it’s not too hard to sketch a graph of the function and, in this case
as we’ll see accuracy is not really going to be an issue. So, here is a quick
sketch of the graph.

![image 2.6_1](./2.6_1.png)

So, we can see from this graph that the function does behave much as we
predicted that it would from our table values. The closer $x$ gets to zero from
the right the larger (in the positive sense) the function gets, while the closer
$x$ gets to zero from the left the larger (in the negative sense) the function
gets.

Finally, the normal limit, in this case, will not exist since the two one-sided
limits have different values.

So, in summary here are the values of the three limits for this example.

$$ \lim\limits_{x \to 0^{+}}\frac{1}{x} = \infty \quad \quad \lim\limits_{x \to 0^{-}}\frac{1}{x} = -\infty \quad \quad \lim\limits_{x \to 0}\frac{1}{x} \text{ does not exist} $$

---

For most of the remaining examples in this section we’ll attempt to “talk our
way through” each limit. This means that we’ll see if we can analyze what should
happen to the function as we get very close to the point in question without
actually plugging in any values into the function. For most of the following
examples this kind of analysis shouldn’t be all that difficult to do. We’ll also
verify our analysis with a quick graph.

So, let’s do a couple more examples.

---

**Example 2** Evaluate each of the following limits.

$$ \lim\limits_{x \to 0^{+}}\frac{6}{x^2} \quad \quad \lim\limits_{x \to 0^{-}}\frac{6}{x^2} \quad \quad \lim\limits_{x \to 0}\frac{6}{x^2} $$

**Solution**

As with the previous example let’s start off by looking at the two one-sided
limits. Once we have those we’ll be able to determine a value for the normal
limit.

So, let’s take a look at the right-hand limit first and as noted above let’s see
if we can figure out what each limit will be doing without actually plugging in
any values of $x$ into the function. As we take smaller and smaller values of
$x$, while staying positive, squaring them will only make them smaller (recall
squaring a number between zero and one will make it smaller) and of course it
will stay positive. So, we have a positive constant divided by an increasingly
small positive number. The result should then be an increasingly large positive
number. It looks like we should have the following value for the right-hand
limit in this case,

$$ \lim\limits_{x \to 0^{+}}\frac{6}{x^2} = \infty $$

Now, let’s take a look at the left-hand limit. In this case we’re going to take
smaller and smaller values of $x$, while staying negative this time. When we
square them they’ll get smaller, but upon squaring the result is now positive.
So, we have a positive constant divided by an increasingly small positive
number. The result, as with the right-hand limit, will be an increasingly large
positive number and so the left-hand limit will be,

$$ \lim\limits_{x \to 0^{-}}\frac{6}{x^2} = \infty $$

Now, in this example, unlike the first one, the normal limit will exist and be
infinity since the two one-sided limits both exist and have the same value. So,
in summary here are all the limits for this example as well as a quick graph
verifying the limits.

$$ \lim\limits_{x \to 0^{+}}\frac{6}{x^2} = \infty \quad \quad \lim\limits_{x \to 0^{-}}\frac{6}{x^2} = \infty \quad \quad \lim\limits_{x \to 0}\frac{6}{x^2} = \infty  $$

![image 2.6_2](./2.6_2.png)

---

With this next example we’ll move away from just an $x$ in the denominator, but
as we’ll see in the next couple of examples they work pretty much the same way.

---

**Example 3** Evaluate each of the following limits.

$$ \lim\limits_{x \to -2^+}\frac{-4}{x + 2} \quad \quad \lim\limits_{x \to -2^-}\frac{-4}{x + 2} \quad \quad \lim\limits_{x \to -2}\frac{-4}{x + 2} $$

Let’s again start with the right-hand limit. With the right-hand limit we know
that we have,

$$ x > -2 \quad \quad \Rightarrow \quad \quad x + 2 > 0 $$

Also, as $x$ gets closer and closer to -2 then $x + 2$ will be getting closer
and closer to zero, while staying positive as noted above. So, for the
right-hand limit, we’ll have a negative constant divided by an increasingly
small positive number. The result will be an increasingly large and negative
number. So, it looks like the right-hand limit will be negative infinity.

For the left-hand limit we have,

$$ x < -2 \quad \quad \Rightarrow \quad \quad x + 2 < 0 $$

and $x + 2$ will get closer and closer to zero (and be negative) as $x$ gets
closer and closer to -2. In this case then we’ll have a negative constant
divided by an increasingly small negative number. The result will then be an
increasingly large positive number and so it looks like the left-hand limit will
be positive infinity.

Finally, since two one sided limits are not the same the normal limit won’t
exist.

Here are the official answers for this example as well as a quick graph of the
function for verification purposes.

$$ \lim\limits_{x \to -2^+}\frac{-4}{x + 2} = -\infty \quad \quad \lim\limits_{x \to -2^-}\frac{-4}{x + 2} = \infty \quad \quad \lim\limits_{x \to -2}\frac{-4}{x + 2} \text{ doesn't exist} $$

![image 2.6_3](./2.6_3.png)

---

At this point we should briefly acknowledge the idea of vertical asymptotes.
Each of the three previous graphs have had one. Recall from an Algebra class
that a vertical asymptote is a vertical line (the dashed line at $x = -2$ in the
previous example) in which the graph will go towards infinity and/or minus
infinity on one or both sides of the line.

In an Algebra class they are a little difficult to define other than to say
pretty much what we just said. Now that we have infinite limits under our belt
we can easily define a vertical asymptote as follows,

**Definition**

> The function $f(x)$ will have a vertical asymptote at $x = a$ if we have any
> of the following limits at $x = a$.
>
> $$ \lim\limits_{x \to a^-}f(x) = \pm \infty \quad \quad \lim\limits_{x \to a^+}f(x) = \pm \infty \quad \quad \lim\limits_{x \to a}f(x) = \pm \infty $$

Note that it only requires one of the above limits for a function to have a
vertical asymptote at $x = a$.

Using this definition we can see that the first two examples had vertical
asymptotes at $x = 0$ while the third example had a vertical asymptote at
$x = -2$.

We aren’t really going to do a lot with vertical asymptotes here but wanted to
mention them at this point since we’d reached a good point to do that.

Let’s now take a look at a couple more examples of infinite limits that can
cause some problems on occasion.

---

**Example 4** Evaluate each of the following limits.

$$ \lim\limits_{x \to 4^+}\frac{3}{(4 - x)^3} \quad \quad \lim\limits_{x \to 4^-}\frac{3}{(4 - x)^3} \quad \quad \lim\limits_{x \to 4}\frac{3}{(4 - x)^3} $$

**Solution**

Let’s start with the right-hand limit. For this limit we have,

$$ x > 4 \quad \quad \Rightarrow \quad \quad 4 - x < 0 \quad \quad \Rightarrow \quad \quad (4 - x)^3 < 0 $$

also, $4 - x \rightarrow 0$ as $x \rightarrow 4$. So, we have a positive
constant divided by an increasingly small negative number. The results will be
an increasingly large negative number and so it looks like the right-hand limit
will be negative infinity.

For the left-handed limit we have,

$$ x < 4 \quad \quad \Rightarrow \quad \quad 4 - x > 0 \quad \quad \Rightarrow \quad \quad (4 - x)^3 > 0 $$

and we still have, $4 - x \rightarrow 0$ as $x \rightarrow 4$. In this case we
have a positive constant divided by an increasingly small positive number. The
results will be an increasingly large positive number and so it looks like the
left-hand limit will be positive infinity.

The normal limit will not exist since the two one-sided limits are not the same.
The official answers to this example are then,

$$ \lim\limits_{x \to 4^+}\frac{3}{(4 - x)^3} = -\infty \quad \quad \lim\limits_{x \to 4^-}\frac{3}{(4 - x)^3} = \infty \quad \quad \lim\limits_{x \to 4}\frac{3}{(4 - x)^3} \text{ doesn't exist} $$

![image 2.6_4](./2.6_4.png)

---

All the examples to this point have had a constant in the numerator and we
should probably take a quick look at an example that doesn’t have a constant in
the numerator.

---

**Example 5** Evaluate each of the following limits.

$$ \lim\limits_{x \to 3^+}\frac{2x}{x - 3} \quad \quad \lim\limits_{x \to 3^-}\frac{2x}{x - 3} \quad \quad \lim\limits_{x \to 3}\frac{2x}{x - 3} $$

**Solution**

Let’s take a look at the right-handed limit first. For this limit we’ll have,

$$ x > 3 \quad \quad \Rightarrow \quad \quad x - 3 > 0 $$

The main difference here with this example is the behavior of the numerator as
we let $x$ get closer and closer to 3. In this case we have the following
behavior for both the numerator and denominator.

$$ x - 3 \rightarrow 0 \quad \text{ and } \quad 2x \rightarrow 6 \quad \text{ as } \quad x \rightarrow 3 $$

So, as we let $x$ get closer and closer to 3 (always staying on the right of
course) the numerator, while not a constant, is getting closer and closer to a
positive constant while the denominator is getting closer and closer to zero and
will be positive since we are on the right side.

This means that we’ll have a numerator that is getting closer and closer to a
non-zero and positive constant divided by an increasingly smaller positive
number and so the result should be an increasingly larger positive number. The
right-hand limit should then be positive infinity.

For the left-hand limit we’ll have,

$$ x < 3 \quad \quad \Rightarrow \quad \quad x - 3 < 0 $$

As with the right-hand limit we’ll have the following behaviors for the
numerator and the denominator,

$$ x - 3 \rightarrow 0 \quad \text{ and } \quad 2x \rightarrow -6 \quad \text{ as } \quad x \rightarrow 3 $$

The main difference in this case is that the denominator will now be negative.
So, we’ll have a numerator that is approaching a positive, non-zero constant
divided by an increasingly small negative number. The result will be an
increasingly large and negative number.

The formal answers for this example are then,

$$ \lim\limits_{x \to 3^+}\frac{2x}{x - 3} = \infty \quad \quad \lim\limits_{x \to 3^-}\frac{2x}{x - 3} = -\infty \quad \quad \lim\limits_{x \to 3^+}\frac{2x}{x - 3} \text{ doesn't exist} $$

As with most of the examples in this section the normal limit does not exist
since the two one-sided limits are not the same.

Here’s a quick graph to verify our limits.

![image 2.6_5](./2.6_5.png)

---

So far all we’ve done is look at limits of rational expressions, let’s do a
couple of quick examples with some different functions.

---

**Example 6** Evaluate

$$ \lim\limits_{x \to 0^+}\ln(x) $$

**Solution**

First, notice that we can only evaluate the right-handed limit here. We know
that the domain of any logarithm is only the positive numbers and so we can’t
even talk about the left-handed limit because that would necessitate the use of
negative numbers. Likewise, since we can’t deal with the left-handed limit then
we can’t talk about the normal limit.

This limit is pretty simple to get from a quick sketch of the graph.

![image 2.6_6](./2.6_6.png)

From this we can see that,

$$ \lim\limits_{x \to 0^+}\ln(x) = -\infty $$

---

**Example 7** Evaluate both of the following limits.

$$ \lim\limits_{x \to \frac{\pi}{2}^+}\tan(x) \quad \quad \lim\limits_{x \to \frac{\pi}{2}^-}\tan(x) $$

**Solution**

Here’s a quick sketch of the graph of the tangent function.

![image 2.6_7](./2.6_7.png)

From this it’s easy to see that we have the following values for each of these
limits,

$$ \lim\limits_{x \to \frac{\pi}{2}^+}\tan(x) = -\infty \quad \quad \lim\limits_{x \to \frac{\pi}{2}^-}\tan(x) = \infty $$

Note that the normal limit will not exist because the two one-sided limits are
not the same.

---

We’ll leave this section with a few facts about infinite limits.

**Facts**

> Given the functions $f(x)$ and $g(x)$ suppose we have,
>
> $$ \lim\limits_{x \to c}f(x) = \infty \quad \quad \lim\limits_{x \to c}g(x) = L $$
>
> for some real numbers $c$ and $L$. Then,
>
> 1. $\lim\limits_{x \to c}\left[f(x) \pm g(x)\right] = \infty$
> 2. If $L > 0$ then $\lim\limits_{x \to c}\left[f(x)g(x)\right] = \infty$
> 3. If $L < 0$ then $\lim\limits_{x \to c}\left[f(x)g(x)\right] = -\infty$
> 4. $\lim\limits_{x \to c}\dfrac{g(x)}{f(x)} = 0$

To see the proof of this set of facts see the
[Proof of Various Limit Properties](https://tutorial.math.lamar.edu/Classes/CalcI/LimitProofs.aspx#Extras_Limit_InfLimitFacts)
section in the Extras chapter.

Note as well that the above set of facts also holds for one-sided limits. They
will also hold if $\lim\limits_{x \to c}f(x) = -\infty$ , with a change of sign
on the infinities in the first three parts. The proofs of these changes to the
facts are nearly identical to the proof of the original facts and so are left to
the you.

---

## Practice Problems

For problems 1 – 6 evaluate the indicated limits, if they exist.

**1.** For $f(x) = \dfrac{9}{(x - 3)^5}$ evaluate,

**(a)** $\lim\limits_{x \to 3^-}f(x)$

**Solution**

$$ x \to 3^- \quad \Rightarrow \quad x - 3 < 0 \quad \text{ therefore } \quad (x - 3)^5 < 0  $$

$$ \boxed{\lim\limits_{x \to 3^-}f(x) = -\infty} $$

**(b)** $\lim\limits_{x \to 3^+}f(x)$

**Solution**

$$ x \to 3^+ \quad \Rightarrow \quad x - 3 > 0 \quad \text{ therefore } \quad (x - 3)^5 > 0 $$

$$ \boxed{\lim\limits_{x \to 3^+}f(x) = \infty} $$

**\(c\)** $\lim\limits_{x \to 3}f(x)$

**Solution**

$$ \lim\limits_{x \to 3^-} \neq \lim\limits_{x \to 3^+} $$

$$ \boxed{\lim\limits_{x \to 3}f(x) \text{ does not exist}} $$

**2.** For $h(t) = \dfrac{2t}{6 + t}$ evaluate,

**(a)** $\lim\limits_{t \to -6^-}h(t)$

**Solution**

$$ t < -6 \quad \Rightarrow \quad 6 + t < 0 $$

Also:

$$ t \to -6^- \quad \Rightarrow \quad 2t \to -12 $$

The signs on both the numerator and denominator trend towards $-\infty$, but
because they are divided, the signs cancel out, veering this function towards
$\infty$ on the left-handed side limit.

$$ \boxed{\lim\limits_{t \to -6^-}h(t) = \infty} $$

**(b)** $\lim\limits_{t \to -6^+}h(t)$

**Solution**

$$ t \to -6^+ \quad \Rightarrow \quad 6 + t > 0 $$

Also:

$$ t \to -6^+ \quad \Rightarrow \quad 2t \to -12 $$

The denominator increasingly veers towards an increasingly small positive
number, while the numerator is approaching a negative number. Yielding
$-\infty$. $$ \boxed{\lim\limits_{t \to -6^+}h(t) = -\infty} $$

**\(c\)** $\lim\limits_{t \to -6}h(t)$

**Solution**

$$ \lim\limits_{t \to -6^-}h(t) \neq \lim\limits_{t \to -6^+}h(t) $$

$$ \boxed{\lim\limits_{t \to -6}h(t) \text{ does not exist}} $$

**3.** For $g(z) = \dfrac{z + 3}{(z + 1)^2}$ evaluate,

**(a)** $\lim\limits_{z \to -1^-}g(z)$

**Solution**

For the denominator:

$$ z \to -1^- \quad \Rightarrow \quad z + 1 < 0 \text{, } z < -1 $$

However the squaring on the denominator indicates that our denominator will
always be positive despite the fact that we will always have a negative number
less than $-1$.

For the numerator:

$$ z \to -1^- \quad \Rightarrow \quad z + 3 \to 2 $$

So we approach a positive number on the numerator and also on the denominator.

$$ \boxed{\lim\limits_{z \to -1^-}g(z) = \infty} $$

**(b)** $\lim\limits_{z \to -1^+}g(z)$

**Solution**

For the denominator:

$$ z \to -1^+ \quad \Rightarrow \quad z + 1 > 0 \text{, } z > -1 $$

And of course, squaring a positive number also yields a positive number.

For the numerator:

$$ z \to -1^+ \quad \Rightarrow \quad z + 3 \to 2 $$

This is also a positive number on the numerator. Dividing the numerator by the
denominator yields an increasingly small positive number.

$$ \boxed{\lim\limits_{z \to -1^+}g(z) = \infty} $$

**\(c\)** $\lim\limits_{z \to -1}g(z)$

$$ \lim\limits_{z \to -1^-}g(z) = \lim\limits_{z \to -1^+}g(z) $$

$$ \boxed{\lim\limits_{z \to -1}g(z) = \infty} $$

**Solution**

**4.** For $g(x) = \dfrac{x + 7}{x^2 - 4}$ evaluate,

**(a)** $\lim\limits_{x \to 2^-}g(x)$

**Solution**

Denominator:

$$ x \to 2^- \quad \Rightarrow \quad x^2 - 4 \rightarrow 0^- $$

Right around the limit from the left hand side we have negative numbers as we
get closer and closer to $2$.

Numerator:

$$ x \to 2^- \quad \Rightarrow \quad x + 7 \rightarrow 9^- $$

And we start to approach a positive number on the numerator. A positive divided
by a negative is a negative.

$$ \boxed{\lim\limits_{x \to 2^-}g(x) = -\infty} $$

**(b)** $\lim\limits_{x \to 2^+}g(x)$

**Solution**

Denominator:

$$ x \to 2^+ \quad \Rightarrow \quad x^2 - 4 \rightarrow 0^+ $$

This means the denominator will always be positive when approaching the limit
from the right-hand side.

Numerator:

$$ x \to 2^+ \quad \Rightarrow \quad x + 7 \rightarrow 9^+ $$

Likewise, the numerator will always be positive, since we are taking a number
always greater than positive $2$ and simply adding $7$ to it. This is also an
increasingly positive number.

$$ \boxed{\lim\limits_{x \to 2^+}g(x) = \infty} $$

**\(c\)** $\lim\limits_{x \to 2}g(x)$

$$ \lim\limits_{x \to 2^-}g(x) \neq \lim\limits_{x \to 2^+}g(x)  $$

$$ \boxed{\lim\limits_{x \to 2}g(x) \text{ does not exist}} $$

**Solution**

**5.** For $h(x) = \ln(-x)$ evaluate,

**(a)** $\lim\limits_{x \to 0^-}h(x)$

**Solution**

This is a tricky one, because we know we cannot take negative values as
arguments to logarithms. However, when approaching from the left hand side, and
because we are specifically approaching it from the left of $0$ (_i.e._ $0^-$),
we know that the negatives will always cancel out and we will have a positive
argument. This changes us to evaluating $\ln(x)$ instead, and we approach
$-\infty$ like in the limits of a normal logarithm.

To be clear:

$$ x \to 0^- \quad \Rightarrow \quad -x > 0 $$

$$ \boxed{\lim\limits_{x \to 0^-}h(x) = -\infty} $$

**(b)** $\lim\limits_{x \to 0^+}h(x)$

**Solution**

However, this limit cannot exist, as $x$ approaching $0$ from the right-hand,
_i.e._ positive side of $0$, implies that $x$ will always be negative:

$$ x \to 0^+ \quad \Rightarrow \quad -x < 0 $$

And therefore:

$$ \boxed{\lim\limits_{x \to 0^+}h(x) \text{ does not exist}} $$

**\(c\)** $\lim\limits_{x \to 0}h(x)$

**Solution**

And since the right-hand side limit doesn't exist, neither can the limit itself:

$$ \boxed{\lim\limits_{x \to 0}h(x) \text{ does not exist}} $$

**6.** For $R(y) = \tan(y)$ evaluate,

**(a)** $\lim\limits_{y \to \frac{3\pi}{2}^-}R(y)$

**Solution**

Recalling the standard graph for Tangent, we can see that as we approach all
increments of $\dfrac{\pi}{2}$, we get either increasing smaller (_i.e._
$-\infty$) or increasingly larger (_i.e._ $\infty$). Approaching the
**asymptotes** from the left we can see that we approach positive.

$$ \boxed{\lim\limits_{y \to \frac{3\pi}{2}^-}R(y) = \infty} $$

**(b)** $\lim\limits_{y \to \frac{3\pi}{2}^+}R(y)$

**Solution**

And from the right we approach negative.

$$ \boxed{\lim\limits_{y \to \frac{3\pi}{2}^+}R(y) = -\infty} $$

**\(c\)** $\lim\limits_{y \to \frac{3\pi}{2}}R(y)$

**Solution**

$$ \lim\limits_{y \to \frac{3\pi}{2}^-}R(y) \neq \lim\limits_{y \to \frac{3\pi}{2}^+}R(y) $$

$$ \boxed{\lim\limits_{y \to \frac{3\pi}{2}}R(y) \text{ does not exist}} $$

For problems 7 & 8 find all the vertical asymptotes of the given function.

**7.** $f(x) = \dfrac{7x}{(10 - 3x)^4}$

**Solution**

Recall that we will have vertical asymptotes for any of the conditions where
either one-sided limits reach positive or negative infinity. Therefore
evaluating the two one sided limits of this function will tell us what the
vertical asymptotes are (if any).

We can ascertain our vertical asymptotes by evaluating any factors in the
denominator and setting them to $0$.

$$ 10 - 3x = 0 $$

$$ -3x = -10 $$

$$ x = \frac{10}{3} $$

This is a potential vertical asymptote, let's evaluate the one-sided limits as
$x$ approaches $\dfrac{10}{3}$ to determine if they approach positive or
negative infinity.

$$ \lim\limits_{x \to \frac{10}{3}^-}\frac{7x}{(10x - 3x)^4} \quad \text{ and } \quad \lim\limits_{x \to \frac{10}{3}^+}\frac{7x}{(10x - 3x)^4} $$

From this we can see that:

$$ x \rightarrow \frac{10}{3}^- \quad \Rightarrow \quad x < \frac{10}{3} \quad \Rightarrow \quad \frac{10}{3} - x > 0 \quad \Rightarrow \quad 10 - 3x > 0 $$

$$ x \rightarrow \frac{10}{3}^+ \quad \Rightarrow \quad x > \frac{10}{3} \quad \Rightarrow \quad \frac{10}{3} - x < 0 \quad \Rightarrow \quad 10 - 3x > 0 $$

Because of the even exponent, both of these limit evaluations will result in
veering towards positive infinity though (in the form of a positive fixed number
in the numerator,a nd a positive, increasingly small denominatory). Therefore
our limits are:

$$ \lim\limits_{x \to \frac{10}{3}^-}\frac{7x}{(10 - 3x)^4} = \infty \quad \lim\limits_{x \to \frac{10}{3}^+}\frac{7x}{(10 - 3x)^4} = \infty \quad \lim\limits_{x \to \frac{10}{3}}\frac{7x}{(10 - 3x)^4} = \infty  $$

All indicating that there is:

$$ \boxed{\text{VERTICAL ASYMPTOTE AT: } \frac{10}{3}} $$

**8.** $g(x) = \dfrac{-8}{(x + 5)(x - 9)}$

**Solution**

Again, we can find our potential vertical asymptotes by taking each factor in
the denominator and setting it to $0$:

$$ x + 5 = 0 $$

$$ x = -5 $$

$$ x - 9 = 0 $$

$$ x = 9 $$

We can now check the one-sided limits of each factor and see if they approach
either or both positive/negative infinity:

$$ \lim\limits_{x \to -5^-}\frac{-8}{(x + 5)(x - 9)} \text { and } \lim\limits_{x \to -5^+}\frac{-8}{(x + 5)(x - 9)} $$

$$ \lim\limits_{x \to 9^-}\frac{-8}{(x + 5)(x - 9)} \text { and } \lim\limits_{x \to 9^+}\frac{-8}{(x + 5)(x - 9)} $$

Let's evaluate each of these one-sided limits:

$$ x \rightarrow -5^- \quad \Rightarrow \quad x < -5 \quad \Rightarrow \quad x + 5 < 0 $$

$$ x \rightarrow -5^+ \quad \Rightarrow \quad x > -5 \quad \Rightarrow \quad x + 5 > 0 $$

And since there are no exponents being raised, this does not change the sign of
these factors when evaluating close to their one-sided limits (negative for
left, positive for right). Also note that for all $x$ close enough to $-5$, this
will also mean the other factor $x - 9 < 0$.

This means that when $x \rightarrow -5^-$, the two denominator factors will both
be negative, resulting in a positive product on the denominator. When the
negative constant on the numerator divides by this positive denominator, we will
get an increasingly more negative, increasingly smaller, number. Convesely, this
also means thatn when $x \rightarrow -5^+$, the two denominators will be
opposite signs: $(x + 5)$ will be positive, while $x - 9$ will be negative. When
the negative constant numerator divides this resulting negative denominator, the
result is that it will approach an increasingly more positive, and increasingly
smaller number.

$$ \lim\limits_{x \to -5^-}\frac{-8}{(x + 5)(x - 9)} = -\infty $$

$$ \lim\limits_{x \to -5^+}\frac{-8}{(x + 5)(x - 9)} = \infty $$

We come to a similar conclusion when evaluating the other $x - 9$ factor:

$$ x \to 9^- \quad \Rightarrow \quad x < 9 \quad \Rightarrow \quad x - 9 < 0 $$

$$ x \to 9^+ \quad \Rightarrow \quad x > 9 \quad \Rightarrow \quad x - 9 > 0 $$

As $x \to 9^-$ or $x \to 9^+$, we can assume this is in the realm of
$x \to 5^+$, and therefore $x + 5 > 0$. This means the other factor in both
one-sided limits will always be positive.

As $x \to 9^-$, we can see that this will result in a negative factor, which
when multiplied by it's guaranteed to be positive other factor of $x + 5$, we
get a negative denominator, which when the negative constant numerator divides
by, will be positive.

Conversely, as $x \to 9^+$, we can see that this will result in a positive
factor, which when multiplied by it's guaranteed to be positive other factor of
$x k 5$, we get a positive denominator, which when the negative constant
numerator divides by, will be negative.

$$ \lim\limits_{x \to 9^-}\frac{-8}{(x + 5)(x - 9)} = \infty $$

$$ \lim\limits_{x \to 9^+}\frac{-8}{(x + 5)(x - 9)} = -\infty $$

Both of these evaluations show that both $x - 5$ and $x = 9$ have one-sided
limits (though not "full" limits) that satisfy our definition for having a
vertical asymptotes.

We have therefore proven that we have:

$$ \boxed{\text{VERTICAL ASYMPTOTES AT: } x = -5 \text{ AND } x = 9} $$

---

## Assignment Problems

For problems 1 – 8 evaluate the indicated limits, if they exist.

**1.** For $g(x) = \dfrac{-4}{(x - 1)^2}$ evaluate,

**(a)** $\lim\limits_{x \to 1^-}g(x)$

**Solution**

For the denominator:

$$ x \rightarrow 1^- \quad \Rightarrow \quad x - 1 < 0, x < 1 $$

However:

$$ x \rightarrow 1^- \quad \Rightarrow \quad (x - 1)^2 > 0 $$

Therefore we always have a positive denominator for $x \rightarrow 1^-$. When
divided by the negative numerator constant, this always trends towards
$-\infty$.

$$ \boxed{\lim\limits_{x \to 1^-}g(x) = -\infty} $$

**(b)** $\lim\limits_{x \to 1^+}g(x)$

**Solution**

This is similar to party **(a)** in that the denominator is guaranteed to be
positive.

$$ x \rightarrow 1^+ \quad \Rightarrow \quad x - 1 > 0, x > 1 $$

And of course:

$$ x \rightarrow 1^+ \quad \Rightarrow \quad (x - 1)^2 > 0 $$

And again, we have the negative constant numerator being divided by the always
positive (thanks to the even exponent) denominator, resulting in this also
trending towards negative infinity:

$$ \boxed{\lim\limits_{x \to 1^+}g(x) = -\infty} $$

**\(c\)** $\lim\limits_{x \to 1}g(x)$

**Solution**

Since:

$$ \lim\limits_{x \to 1^-}g(x) = \lim\limits_{x \to 1^+}g(x) $$

This means this limits exists and is equivalent to its two one-sided-limits:

$$ \boxed{\lim\limits_{x \to 1}g(x) = -\infty} $$

**2.** For $h(z) = \dfrac{17}{(4 - z)^3}$ evaluate,

**(a)** $\lim\limits_{z \to 4^-}h(z)$

**Solution**

Considering:

$$ z \to 4^- \quad \Rightarrow \quad 4 - z \rightarrow 0^- $$

This means that:

$$ z \to 4^- \quad \Rightarrow \quad 4 - z > 0, z < 4 $$

And when cubed, maintains its positive sign.

When divided by the constant positive numerator, this means that this left-hand
limit tends towards $\infty$.

$$ \boxed{\lim\limits_{z \to 4^-}h(z) = \infty} $$

**(b)** $\lim\limits_{z \to 4^+}h(z)$

**Solution**

Considering:

$$ z \to 4^+ \quad \Rightarrow \quad 4 - z \rightarrow 0^+ $$

This means that:

$$ z \to 4^+ \quad Rightarrow \quad 4 - z < 0, z > 4 $$

And when cubed, maintains its negative sign.

When divided by the constant positive numerator, this means that this
right-handed limit tends towards $-\infty$.

$$ \boxed{\lim\limits_{z \to 4^+}h(z) = -\infty} $$

**\(c\)** $\lim\limits_{z \to 4}h(z)$

**Solution**

Since

$$ \lim\limits_{z \to 4^-}h(z) \neq \lim\limits_{z \to 4^+}h(z) $$

This limit does not exist.

$$ \boxed{\lim\limits_{z \to 4}h(z) \text{ does not exist}} $$

**3.** For $g(t) = \dfrac{4t^2}{(t + 3)^7}$ evaluate,

**(a)** $\lim\limits_{t \to -3^-}g(t)$

**Solution**

Here we have our variable $t$ in both the numerator and denominator, and both
are raised to an exponent (even on the numerator, odd on the denominator).

Let's consider what this left-hand side limit does as it approaches $-3^-$:

$$ t \rightarrow -3^- \quad \Rightarrow \quad t + 3 < 0 $$

The odd exponent of $(t + 3)^7$ indicates this will maintain its negative sign.

However on the numerator:

$$ t \rightarrow -3^- \quad \Rightarrow \quad t^2 > 0 $$

Because of the even exponent. Thusly we have an positive numerator divided by an
increasingly more negative denominator, causing this left-hand limit to trend
towards $-\infty$.

$$ \boxed{\lim\limits_{t \to -3^-}g(t) = -\infty} $$

**(b)** $\lim\limits_{t \to -3^+}g(t)$

**Solution**

Now, as we consider what happens on the right-hand sided limit, we get a
different outcome:

$$ x \to -3^+ \quad \Rightarrow \quad t + 3 > 0 $$

And $(t + 3)^7$ in this case will maintain the positive sign.

Additionally the numerator still remains positive:

$$ x \to -3^+ \quad \Rightarrow \quad 4t^2 > 0 $$

And two positives divided by each other indicates a positive output(albeit
increasingly smaller values as it veers off from $x = -3$). This means that this
veers off towards $\infty$.

$$ \boxed{\lim\limits_{t \to -3^+}g(t) = \infty} $$

**\(c\)** $\lim\limits_{t \to -3}g(t)$

**Solution**

And of course since:

$$ \lim\limits_{t \to 3^-}g(t) \neq \lim\limits_{t \to 3^+}g(t)  $$

The limit does not exist.

$$ \lim\limits_{t \to -3}g(t) \text{ does not exist} $$

**4.** For $f(x) = \dfrac{1 + x}{x^3 + 8}$ evaluate,

**(a)** $\lim\limits_{x \to -2^-}f(x)$

**Solution**

Let's consider the denominator first:

$$ x \to -2^- \quad \Rightarrow \quad x^3 + 8 < 0 $$

And we have a negative denominator. On the numerator:

$$ x \to -2^- \quad \Rightarrow \quad 1 + x < 0 $$

And two negatives divided creates a positive, and we veer off towards
increasingly smaller **positive** values as we get further and further away from
$x = -2$. In other words, we are veering off towards $\infty$.

$$ \boxed{\lim\limits_{x \to -2^-}f(x) = \infty} $$

**(b)** $\lim\limits_{x \to -2^+}f(x)$

**Solution**

Let's again consider the denominator:

$$ x \to -2^+ \quad \Rightarrow \quad x^3 + 8 > 0 $$

A positive denominator. And the numerator:

$$ x \to -2^+ \quad \Rightarrow \quad 1 + x < 0 $$

And we have a positive numerator. A positive divided by a positive indicates
that we are veering off towards $-\infty$.

$$ \boxed{\lim\limits_{x \to -2^+}f(x) = -\infty} $$

**\(c\)** $\lim\limits_{x \to -2}f(x)$

**Solution**

And since:

$$ \lim\limits_{x \to -2^-}f(x) \neq \lim\limits_{x \to -2^+}f(x) $$

$$ \boxed{\lim\limits_{x \to -2}f(x) \text{ does not exist}} $$

**5.** For $f(x) = \dfrac{x - 1}{(x^2 - 9)^4}$ evaluate,

**(a)** $\lim\limits_{x \to 3^-}f(x)$

**Solution**

Denominator:

$$ x \to 3^- \quad \Rightarrow \quad (x^2 - 9)^4 > 0 $$

Due to the even exponent on the outside of the factor (_i.e._ $4$).

Numerator:

$$ x \to 3^- \quad \Rightarrow \quad x - 1 > 0 $$

This is mainly due to the fact that we are at the limit, trying to stay close to
the left hand side of $x =3$. But yes, we are veering towards $\infty$.

$$ \boxed{\lim\limits_{x \to 3^-}f(x) = \infty} $$

**(b)** $\lim\limits_{x \to 3^+}f(x)$

**Solution**

Denominator:

$$ x \to 3^+ \quad \Rightarrow \quad (x^2 - 9)^4 > 0 $$

And the numerator:

$$ x \to 3^+ \quad \Rightarrow \quad x - 1 > 0 $$

And we have another one-sided-limit that veers off towards $\infty$.

It is worthy to note that if you were to evaluate the one-sided limits as
$x \to -3$, the signs would change and we'd veer off towards $-\infty$ on both
sides. This is because the numerator would change the sign to negative in that
case.

$$ \boxed{\lim\limits_{x \to 3^+}f(x) = \infty} $$

**\(c\)** $\lim\limits_{x \to 3}f(x)$

**Solution**

$$ \lim\limits_{x \to 3^-}f(x) = \lim\limits_{x \to 3^+}f(x) $$

$$ \boxed{\lim\limits_{x \to 3}f(x) = \infty} $$

**6.** For $W(t) = \ln(t + 8)$ evaluate,

**(a)** $\lim\limits_{t \to -8^-}W(t)$

**Solution**

This is just the standard natural logarithm shifted to the left $8$ units.

Since the natural log (or any log) cannot have a real output for a negative
input, we can say that all left-hand limits don't exist.

$$ \boxed{\lim\limits_{t \to -8^-}W(t) \text{ does not exist}} $$

**(b)** $\lim\limits_{t \to -8^+}W(t)$

**Solution**

And on the right hand side, we can say that the natural log veers off towards
$-\infty$.

$$ \boxed{\lim\limits_{t \to -8^+}W(t) = -\infty} $$

**\(c\)** $\lim\limits_{t \to -8}W(t)$

**Solution**

$$ \lim\limits_{t \to -8^-}W(t) \neq \lim\limits_{t \to -8^+}W(t) $$

$$ \boxed{\lim\limits_{t \to -8}W(t) \text{ does not exist}} $$

**7.** For $h(z) = \ln \mid z \mid$ evaluate,

**(a)** $\lim\limits_{z \to 0^-}h(z)$

**Solution**

Here we have an interesting case where we are ensuring that the input to the
natural logarithm will be positive regardless of the sign of the input, as we
first pass it through the absolute value piecewise function. Because of this we
do have a left-hand limit, and it approaches $-\infty$.

$$ \boxed{\lim\limits_{z \to 0^-}h(z) = -\infty} $$

**(b)** $\lim\limits_{z \to 0^+}h(z)$

**Solution**

The absolute value function does not change the output of the standard natural
log function, and it stays veering off towards $-\infty$.

$$ \boxed{\lim\limits_{z \to 0^+}h(z) = -\infty} $$

**\(c\)** $\lim\limits_{z \to 0}h(z)$

**Solution**

$$ \lim\limits_{z \to 0^-}h(z) = \lim\limits_{z \to 0^+}h(z) $$

$$ \boxed{\lim\limits_{z \to 0}h(z) = -\infty} $$

**8.** For $R(y) = \cot(y)$ evaluate,

**(a)** $\lim\limits_{y \to \pi^-}R(y)$

**Solution**

The graph of cotangent looks like the graph of tangent, only reflected about the
$y$-axis. Because of this, as the graph approaches from the left of every $\pi$
interval, it appears to be approaching $-\infty$.

$$ \boxed{\lim\limits_{y \to \pi^-}R(y) = -\infty} $$

**(b)** $\lim\limits_{y \to \pi^+}R(y)$

**Solution**

Likewise, for the right-hand sided limit, we appear to be heading off towards
$\infty$.

$$ \boxed{\lim\limits_{y \to \pi^+}R(y) = \infty} $$

**\(c\)** $\lim\limits_{y \to \pi}R(y)$

**Solution**

$$ \lim\limits_{y \to \pi^-}R(y) \neq \lim\limits_{y \to \pi^+}R(y) $$

$$ \lim\limits_{y \to \pi}R(y) \text{ does not exist} $$

For problems 9 – 12 find all the vertical asymptotes of the given function.

**9.** $h(x) = \dfrac{-6}{9 - x}$

**Solution**

First let's just find where we suspect there is a vertical asymptote by setting
all factors of the denominator to $0$ and evaluating for $x$:

$$ 9 - x = 0 $$

$$ -x = -9 $$

$$ x = 9 $$

If either right or left hand sided limits as $x \to 9$ tend towards $\pm\infty$,
then we know this is a Vertical Asymptote.

Let's first evaluate:

$$ \lim\limits_{x \to 9^-}\frac{-6}{9 - x} $$

$$ x \to 9^- \quad \Rightarrow \quad 9 - x > 0 $$

So we have a positive denominator on the left hand side of $x = 9$ around the
proposed limit.

If we divide the negative constant numerator, we will always get a negative
output, and this veers off towards negative infinity.

$$ \lim\limits_{x \to 9^-}\frac{-6}{9 - x} = -\infty $$

We could stop here, as any left or right side limit just has to veer off towards
$\pm \infty$ to be considered a vertical asymptote. But let's evaluate the right
hand side as well:

$$ \lim\limits_{x \to 9^+}\frac{-6}{9 - x} $$

$$ x \to 9^+ \quad \Rightarrow \quad 9 - x < 0 $$

And a negative numerator divided by a negative denominator always veers off
towards positive infinity.

$$ \lim\limits_{x \to 9^+}\frac{-6}{9 - x} = \infty $$

So even though the limit itself doesn't exist, we have two one-sided-limits that
veer off towards both $-\infty$ and $\infty$, and thusly indeed we have:

$$ \boxed{\text{VERTICAL ASYMPTOTE AT: } x = 9} $$

**10.** $f(x) = \dfrac{x + 8}{x^2(5 - 2x)^3}$

**Solution**

Again, let's evaluate all of the factors in the denominator for potential
Vertical Asymptotes:

$$ x^2 = 0 $$

$$ x = 0 $$

$$ 5 - 2x = 0 $$

$$ -2x = -5 $$

$$ x = \frac{5}{2} $$

So we have two potential Vertical Asymptotes. Let's evaluate the left and right
hand limits of each one:

$$ \lim\limits_{x \to 0^-}\frac{x + 8}{x^2(5 - 2x)^3} $$

$$ x \to 0^- \quad \Rightarrow \quad x^2 > 0 $$

And also note that in this scenario:

$$ x \to 0^- \quad \Rightarrow \quad (5 - 2x)^3 > 0 $$

And the numerator would still be positive as well:

$$ x \to 0^- \quad \Rightarrow \quad x + 8 > 0 $$

So this would veer off towards $+\infty$.

$$ \lim\limits_{x \to 0^-}\frac{x + 8}{x^2(5 - 2x)^3} = \infty $$

Let's evaluate the right-hand side of this Vertical Asymptote now:

$$ \lim\limits_{x \to 0^+}\frac{x + 8}{x^2(5 - 2x)^3} $$

$$ x \to 0^+ \quad \Rightarrow \quad x^2 > 0 $$

Of course this wouldn't change as any even exponent always keeps the output
positive (except for $0$, but because this is a limit, we can guarantee that it
won't be).

Note also that:

$$ x \to 0^+ \quad \Rightarrow \quad (5 - 2x)^3 > 0 $$

The numerator also doesn't change the sign:

$$ x \to 0^+ \quad \Rightarrow \quad x + 8 > 0 $$

And so this also veers off towards positive infinity.

$$ \lim\limits_{x \to 0^+}\frac{x + 8}{x^2(5 - 2x)^3} = \infty $$

And because both one-sided-limits are equivalent for this factor, we have an
outright limit that approaches $+\infty$:

$$ \lim\limits_{x \to 0}\frac{x + 8}{x^2(5 - 2x)^3} = \infty $$

So $x^2$ is definitely a Vertical Asymptote. Let's now check the other factor:

$$ \lim\limits_{x \to \frac{5}{2}^-}\frac{x + 8}{x^2(5 - 2x)^3} $$

$$ x \to \frac{5}{2}^- \quad \Rightarrow \quad (5 - 2x)^3 > 0 $$

Note also that:

$$ x \to \frac{5}{2}^- \quad \Rightarrow \quad x^2 > 0 $$

And also that:

$$ x \to \frac{5}{2}^- \quad \Rightarrow \quad x + 8 > 0 $$

So this veers off towards positive infinity.

$$ \lim\limits_{x \to \frac{5}{2}^-}\frac{x + 8}{x^2(5 - 2x)^3} = \infty $$

Let's check the right-handed limit:

$$ \lim\limits_{x \to \frac{5}{2}^+}\frac{x + 8}{x^2(5 - 2x)^3} $$

$$ x \to \frac{5}{2}^+ \quad \Rightarrow \quad (5 - 2x)^3 < 0 $$

And also note that

$$ x \to \frac{5}{2}^+ \quad \Rightarrow \quad x^2 > 0 $$

And also:

$$ x \to \frac{5}{2}^+ \quad \Rightarrow \quad x + 8 > 0 $$

So we have a positive over a negative and this veers off towards negative
infinity:

$$ \lim\limits_{x \to \frac{5}{2}^+}\frac{x + 8}{x^2(5 - 2x)^3} = -\infty $$

And the limit does not exist since the left and right hand are not equivalent.
That said, this is not a prerequisite, as only one of these one-sided limits
needed to be veering off towards $\pm \infty$ to be considered a Vertical
Asymptote.

Thusly:

$$ \boxed{\text{VERTICAL ASYMPTOTES AT: } x = 0, x = \frac{5}{2}} $$

**11.** $g(t) = \dfrac{5t}{t(t + 7)(t - 12)}$

**Solution**

Let's evaluate all denominator's factors for potential Vertical Asymptotes:

$$ t = 0 $$

We can eliminate this however, as this function is simplified to:

$$ \frac{5t}{t(t + 7)(t - 12)} = \frac{5}{(t + 7)(t - 12)} $$

But this does not mean there isn't a limit at $t \to 0$, just that the limit
doesn't signify a Vertical Asymptote. Let's instead just evaluate for $t = 0$ to
find the limit, but of the simplified function without the $t = 0$ factor:

$$ \lim\limits_{t \to 0}\frac{5}{(t + 7)(t - 12)} $$

$$ t \to 0 \quad \Rightarrow \quad t + 7 \quad 7 $$

$$ t \to 0 \quad \Rightarrow \quad t - 12 \quad -12 $$

The numerator is a constant, so this evaluates to:

$$ \lim\limits_{t \to 0}\frac{5}{(t + 7)(t - 12)} = \frac{5}{(0 + 7)(0 - 12)} = -\frac{5}{84} $$

This limit exists, and thusly:

$$ \lim\limits_{t \to 0^-}\frac{5}{(t + 7)(t - 12)} = -\frac{5}{84} $$

$$ \lim\limits_{t \to 0^+}\frac{5}{(t + 7)(t - 12)} = -\frac{5}{84} $$

Obviously, $-\dfrac{5}{84} \neq \pm \infty$, and therefor $t = 0$ is NOT a
vertical asymptote.

Let's evaluate our other two factors:

$$ t = -7 $$

$$ \lim\limits_{t \to -7^-}\frac{5}{(t + 7)(t - 12)} $$

$$ t \to -7^- \quad \Rightarrow \quad t + 7 < 0 $$

$$ t \to -7^- \quad \Rightarrow \quad t - 12 < 0 $$

These evaluate to a positive on the denominator. With the positive constant
numerator we get:

$$ \frac{+}{(-)(-)} $$

And therefore we veer off towards positive $\infty$.

$$ \lim\limits_{t \to -7^-}\frac{5}{(t + 7)(t - 12)} = \infty $$

Of course, we can stop here as any $\pm \infty$ for these limits will indicate a
Vertical Asymptote, but let's evaluate the right-hand side a well.

$$ \lim\limits_{t \to -7^+}\frac{5}{(t + 7)(t - 12)} $$

$$ t \to -7^+ \quad \Rightarrow \quad t + 7 > 0 $$

$$ t \to -7^+ \quad \Rightarrow \quad t - 12 < 0 $$

So we get a:

$$ \frac{+}{(+)(-)} $$

And we veer off towards $-\infty$.

$$ \lim\limits_{t \to -7^+}\frac{5}{(t + 7)(t - 12)} = -\infty $$

We don't have a full limit here, just two one-sided limits (that don't equate,
hence no limit), but we do have a Vertical Asymptote.

Let's evaluate our final factor:

$$ t = 12 $$

$$ \lim\limits_{t \to 12^-}\frac{5}{(t + 7)(t - 12)} $$

$$ t \to 12^- \quad \Rightarrow \quad t - 12 < 0 $$

$$ t \to 12^- \quad \Rightarrow \quad t - 7 > 0 $$

So we have:

$$ \frac{+}{(+)(-)} $$

So we veer off towards negative infinity:

$$ \lim\limits_{t \to 12^-}\frac{5}{(t + 7)(t - 12)} = -\infty $$

Check the right:

$$ \lim\limits_{t \to 12^+}\frac{5}{(t + 7)(t - 12)} $$

$$ t \to 12^+ \quad \Rightarrow \quad t - 12 > 0 $$

$$ t \to 12^+ \quad \Rightarrow \quad t + 7 > 0 $$

So we have:

$$ \frac{+}{(+)(+)} $$

So we also veer off towards positive infinity:

$$ \lim\limits_{t \to 12^+}\frac{5}{(t + 7)(t - 12)} = \infty $$

Again, we don't have an actual limit here since the two one-sided limits don't
equate, but we do have a Vertical Asymptote.

Our answers are:

$$ \boxed{\text{VERTICAL ASYMPTOTES: } t = -7, t = 12} $$

**12.** $g(z) = \dfrac{z^2 + 1}{(z^2 - 1)^5(z + 15)^6}$

**Solution**

Let's evaluate each of our factors by setting them to $0$:

$$ z^2 - 1 = 0 $$

$$ z^2 = 1 $$

$$ z = \pm 1 $$

$$ z + 15 = 0 $$

$$ z = -15 $$

So our three possible Vertical Asymptotes are:

$$ z = \pm 1 $$

$$ z = -15 $$

Let's look at the one-sided limits of each to find out:

$$ \lim\limits_{z \to 1^-}\frac{z^2 + 1}{(z^2 - 1)^5(z + 15)^6} $$

$$ z \to 1^- \quad \Rightarrow \quad z^2 + 1 < 0 $$

$$ z \to 1^- \quad \Rightarrow \quad (z + 15)^6 > 0 $$

$$ z \to 1^- \quad \Rightarrow \quad z^2 + 1 > 0 $$

So we have:

$$ \frac{+}{(-)(+)} $$

So we veer off toward $-\infty$.

$$ \lim\limits_{z \to 1^-}\frac{z^2 + 1}{(z^2 - 1)^5(z + 15)^6} = -\infty $$

Right hand side:

$$ \lim\limits_{z \to 1^+}\frac{z^2 + 1}{(z^2 - 1)^5(z + 15)^6} $$

$$ z \to 1^+ \quad \Rightarrow \quad z^2 + 1 > 0 $$

$$ z \to 1^+ \quad \Rightarrow \quad (z + 15)^6 > 0 $$

$$ z \to 1^+ \quad \Rightarrow \quad z^2 + 1 > 0 $$

So we have:

$$ \frac{+}{(+)(+)} $$

So we veer off towards $\infty$.

$$ \lim\limits_{z \to 1^+}\frac{z^2 + 1}{(z^2 - 1)^5(z + 15)^6} = \infty $$

And we have a Vertical Asymptote (though not a limit since the two sides are not
equivalent).

Let's evaluate the other factor/potentital Vertical Asymptotes:

$$ z = -1 $$

$$ \lim\limits_{z \to -1^-}\frac{z^2 + 1}{(z^2 - 1)^5(z + 15)^6} $$

$$ z \to -1^- \quad \Rightarrow \quad (z^2 - 1)^5 > 0 $$

$$ z \to -1^- \quad \Rightarrow \quad (z + 15)^6 > 0 $$

$$ z \to -1^- \quad \Rightarrow \quad z^2 + 1 > 0 $$

So we have:

$$ \frac{(+)}{(+)(+)} $$

This veers off towards positive infinity:

$$ \lim\limits_{z \to -1^-}\frac{z^2 + 1}{(z^2 - 1)^5(z + 15)^6} = \infty $$

Right hand side:

$$ \lim\limits_{z \to -1^+}\frac{z^2 + 1}{(z^2 - 1)^5(z + 15)^6} $$

$$ z \to -1^+ \quad \Rightarrow \quad (z^2 - 1)^5 < 0 $$

$$ z \to -1^+ \quad \Rightarrow \quad (z + 15)^6 > 0 $$

$$ z \to -1^+ \quad \Rightarrow \quad z^2 + 1 > 0 $$

$$ \frac{(+)}{(+)(-)} $$

This veers off towards negative infinity.

$$ \lim\limits_{z \to -1^+}\frac{z^2 + 1}{(z^2 - 1)^5(z + 15)^6} = -\infty $$

So we have a Vertical Asymptote (but not a limit) at z = -1

Let's evaluate the other factor/potentital Vertical Asymptotes:

$$ z = -15 $$

$$ \lim\limits_{z \to -15^-}\frac{z^2 + 1}{(z^2 - 1)^5(z + 15)^6} $$

$$ z \to -15^- \quad \Rightarrow \quad (z + 15)^6 > 0  $$

$$ z \to -15^- \quad \Rightarrow \quad (z^2 - 1)^5 > 0 $$

$$ z \to -15^- \quad \Rightarrow \quad z^2 + 1 > 0 $$

So this veers off towards $\infty$.

$$ \lim\limits_{z \to -15^-}\frac{z^2 + 1}{(z^2 - 1)^5(z + 15)^6} = \infty $$

Right hand side

$$ \lim\limits_{z \to -15^+}\frac{z^2 + 1}{(z^2 - 1)^5(z + 15)^6} $$

$$ z \to -15^+ \quad \Rightarrow \quad (z + 15)^6 > 0 $$

$$ z \to -15^+ \quad \Rightarrow \quad (z^2 - 1)^5 > 0 $$

$$ z \to -15^+ \quad \Rightarrow \quad z^2 - 1 > 0 $$

This also veers off towards $\infty$.

So we have a limit and a Vertical Asymptote here.

Our final answer is:

$$ \boxed{\text{VERTICAL ASYMPTOTES AT: } z = 1, z = -1 z = -15} $$
