# 3.6 Combining Functions

---

The topic with functions that we need to deal with is combining functions. For
the most part this means performing basic arithmetic (addition, subtraction,
multiplication, and division) with functions. There is one new way of combining
functions that we’ll need to look at as well.

Let’s start with basic arithmetic of functions. Given two functions $f(x)$ and
$g(x)$ we have the following notation and operations.

$$ (f + g)(x) = f(x) + g(x) $$

$$ (f - g)(x) = f(x) - g(x) $$

$$ (fg)(x) = f(x)g(x) $$

$$ \left(\frac{f}{g}\right) = \frac{f(x)}{g(x)} $$

Sometimes we drop the $(x)$ part and just write the following,

$$ f + g = f(x) + g(x) $$

$$ f - g = f(x) - g(x) $$

$$ fg = f(x)g(x) $$

$$ \frac{f}{g} = \frac{f(x)}{g(x)} $$

Note as well that we put $x$'s in the parenthesis, but we will often put in
numbers as well. Let's take a quick look at an example.

---

**Example 1**

Given $f(x) = 2 + 3x - x^2$ and $g(x) = 2x - 1$ evalute each of the following.

**(a)**

$$ (f + g)(4) $$

$$ (f + g)(4) = (2 + 3(4) - (4)^2) + (2(4) - 1) $$

$$ (f + g)(4) = (2 + 12 - 16) + (8 - 1) $$

$$ (f + g)(4) = -2 + 7 $$

$$ (f + g)(4) = 5 $$

**(b)**

$$ g - f $$

$$ g - f = (2x - 1) - (2 + 3x - x^2) $$

$$ g - f =  2x - 1 - 2 - 3x + x^2 $$

$$ g - f = x^2 - x - 3 $$

**(c\)**

$$ (fg)(x) $$

$$ (fg)(x) = (2 + 3x - x^2)(2x - 1) $$

$$ (fg)(x) = 2(2x - 1) + 3x(2x - 1) - x^2(2x - 1) $$

$$ (fg)(x) = 4x - 2 + 6x^2 - 3x - 2x^3 + x^2 $$

$$ (fg)(x) = -2x^3 + 7x^2 + x - 2 $$

**(d)**

$$ \left(\frac{f}{g}\right)(0) $$

$$ \left(\frac{f}{g}\right)(0) = \frac{2 + 3(0) - (0)^2}{2(0) - 1} $$

$$ \left(\frac{f}{g}\right)(0) = \frac{2}{-1} $$

$$ \left(\frac{f}{g}\right)(0) = -2 $$

---

Now we need to discuss the new method of combining functions. The new method of
combining functions is called **function composition**. Here is the definition.

Given two functions $f(x)$ and $g(x)$ we have the following two definitions.

> 1. The **composition** of $f(x)$ and $g(x)$ (note the order here) is,
>    $(f \circ g) = f[g(x)]$

> 2. The **composition** of $g(x)$ and $f(x)$ (again, note the order) is,
>    $(g \circ f)(x) = g[f(x)]$

We need to note a couple of things here about function composition. First this
is **NOT** multiplication. Regardless of what the notation may suggest to you
this is simply not multiplication.

Second, the order we’ve listed the two functions is very important since more
often than not we will get different answers depending on the order we’ve listed
them.

Finally, function composition is really nothing more than function evaluation.
All we’re really doing is plugging the second function listed into the first
function listed. In the definitions we used $[]$ for the function evaluation
instead of the standard $()$ to avoid confusion with too many sets of
parenthesis, but the evaluation will work the same.

Let’s take a look at a couple of examples.

---

**Example 2**

Given $f(x) = 2 + 3x - x^2$ and $g(x) = 2x - 1$ evaluate each of the following.

**(a)**

$$ (fg)(x) $$

$$ (fg)(x) = (2 + 3x - x^2)(2x - 1) $$

$$ (fg)(x) = 2(2x - 1) + 3x(2x - 1) - x^2(2x - 1) $$

$$ (fg)(x) = 4x - 2 + 6x^2 - 3x - 2x^3 + x^2 $$

$$ (fg)(x) = -2x^3 + 7x^2 + x - 2 $$

**(b)**

$$ (f \circ g)(x) $$

$$ (f \circ g)(x) = f[g(x)] = f[2x - 1] $$

$$ (f \circ g)(x) = 2 + 3(2x - 1) - (2x - 1)^2 $$

$$ (f \circ g)(x) = 2 + 6x - 3 - (2x - 1)(2x - 1) $$

$$ (f \circ g)(x) = 2 + 6x - 3 - (4x^2 - 4x + 1) $$

$$ (f \circ g)(x) = 2 + 6x - 3 - 4x^2 + 4x - 1 $$

$$ (f \circ g)(x) = -4x^2 + 10x - 2 $$

**(c\)**

$$ (g \circ f)(x) $$

$$ (g \circ f)(x) = g[f(x)] = g[2 + 3x - x^2] $$

$$ (g \circ f)(x) = 2(2 + 3x - x^2) - 1 $$

$$ (g \circ f)(x) = 4 + 6x - 2x^2 - 1 $$

$$ (g \circ f)(x) = -2x^2 + 6x + 3 $$

---

The ideas from the previous example are important enough to make again. First,
function composition is NOT function multiplication. Second, the order in which
we do function composition is important. In most case we will get different
answers with a different order. Note however, that there are times when we will
get the same answer regardless of the order.

Let’s work a couple more examples.

---

**Example 3**

Given $f(x) = x^2 - 3$ and $h(x) = \sqrt{x + 1}$ evaluate each of the following.

**(a)**

$$ (f \circ h)(x) $$

$$ (f \circ h)(x) = f[h(x)] = f[\sqrt{x + 1}] $$

$$ (f \circ h)(x) = (\sqrt{x + 1})^2 - 3 $$

$$ (f \circ h)(x) = x + 1 - 3 $$

$$ (f \circ h)(x) = x - 2 $$

**(b)**

$$ (h \circ f)(x) $$

$$ (h \circ f)(x) = h[f(x)] = h[x^2 - 3] $$

$$ (h \circ f)(x) = \sqrt{(x^2 - 3) + 1} $$

$$ (h \circ f)(x) = \sqrt{x^2 - 2} $$

**(c\)**

$$ (f \circ f)(x) $$

$$ (f \circ f)(x) = f[f(x)] = f[x^2 - 3] $$

$$ (f \circ f)(x) =(x^2 - 3)^2 - 3 $$

$$ (f \circ f)(x) =(x^2 - 3)(x^2 - 3) - 3 $$

$$ (f \circ f)(x) =(x^4 - 6x^2 + 9) - 3 $$

$$ (f \circ f)(x) = x^4 - 6x^2 + 6 $$

**(d)**

$$ (h \circ h)(8) $$

$$ (h \circ h)(8) = h[h(8)] = h[\sqrt{8 + 1}] $$

$$ (h \circ h)(8) = \sqrt{\left(\sqrt{8 + 1}\right) + 1} $$

$$ (h \circ h)(8) = \sqrt{\left(\sqrt{9}\right) + 1} $$

$$ (h \circ h)(8) = \sqrt{(3) + 1} $$

$$ (h \circ h)(8) = \sqrt{4} $$

$$ (h \circ h)(8) = 2 $$

**(e)**

$$ (f \circ h)(4) $$

$$ (f \circ h)(4) = f[h(4)] = f[\sqrt{4 + 1}] $$

$$ (f \circ h)(4) = \left(\sqrt{4 + 1}\right)^2 - 3 $$

$$ (f \circ h)(4) = \left(\sqrt{5}\right)^2 - 3 $$

$$ (f \circ h)(4) = 5 - 3 $$

$$ (f \circ h)(4) = 2 $$

---

**Example 4**

Given $f(x) = 3x - 2$ and $g(x) = \dfrac{x}{3} + \dfrac{2}{3}$ evaluate each of
the following.

**(a)**

$$ (f \circ g)(x) $$

$$ (f \circ g)(x) = f[g(x)] = f\left[\frac{x}{3} + \frac{2}{3}\right] $$

$$ (f \circ g)(x) = 3\left(\frac{x}{3} + \frac{2}{3}\right) - 2 $$

$$ (f \circ g)(x) = x + 2 - 2 $$

$$ (f \circ g)(x) = x $$

**(b)**

$$ (g \circ f)(x) $$

$$ (g \circ f)(x) = g[f(x)] = g[3x - 2] $$

$$ (g \circ f)(x) = \frac{(3x - 2)}{3} - \frac{2}{3} $$

$$ (g \circ f)(x) = \frac{1}{3}(3x - 2) - \frac{2}{3} $$

$$ (g \circ f)(x) = x - \frac{2}{3} + \frac{2}{3} $$

$$ (g \circ f)(x) = x $$

So, as we’ve seen from this last example it is possible to get the same answer
from both compositions on occasion. In fact when the answer from both
composition is $x$, as it is in this case, we know that these two functions are
very special functions. In fact, they are so special that we’re going to devote
the whole next section to these kinds of functions. So, let’s move onto the next
section.

---

## Practice Problems

**1.**

Given $f(x) = 6x + 2$ and $g(x) = 10 - 7x$ compute each of the following.

**(a)**

$$ (f - g)(2) $$

$$ (f - g)(2) = (6(2) + 2) - (10 - 7(2))$$

$$ (f - g)(2) = (12 + 2) - (10 - 14) $$

$$ (f - g)(2) = 12 + 2 - 10 + 14 $$

$$ (f - g)(2) = 18 $$

**(b)**

$$ (g - f)(2) $$

$$ (g - f)(2) = (10 - 7(2)) - (6(2) + 2) $$

$$ (g - f)(2) = (10 - 14) - (12 + 2) $$

$$ (g - f)(2) = 10 - 14 - 12 - 2 $$

$$ (g - f)(2) = -18 $$

**(c\)**

Given $f(x) = 6x + 2$ and $g(x) = 10 - 7x$ compute each of the following.

$$ fg $$

$$ fg = (6x + 2)(10 - 7x) $$

$$ fg = 60x + 20 - 32x^2 - 14x $$

$$ fg = -42x^2 + 46x + 20 $$

**(d)**

Given $f(x) = 6x + 2$ and $g(x) = 10 - 7x$ compute each of the following.

$$ \left(\frac{f}{g}\right)(x) $$

$$ \left(\frac{f}{g}\right)(x) = \frac{6x + 2}{10 - 7x} $$

**2.**

Given $P(t) = 4t^2 + 3t - 1$ and $A(t) = 2 - t^2$ compute each of the following.

**(a)**

$$ (P + A)(t) $$

$$ (P + A)(t) = (4t^2 + 3t - 1) + (2 - t^2) $$

$$ (P + A)(t) = 3t^2 + 3t + 1 $$

**(b)**

$$ A - P $$

$$ A - P = (2 - t^2) - (4t^2 + 3t - 1) $$

$$ A - P = 2 - t^2 - 4t^2 - 3t + 1 $$

$$ A - P = -5t^2 - 3t + 3 $$

**(c\)**

$$ (PA)(t) $$

$$ (PA)(t) = (4t^2 + 3t - 1)(2 - t^2) $$

$$ (PA)(t) = 4t^2(2 - t^2) + 3t(2 - t^2) - 1(2 - t^2) $$

$$ (PA)(t) = 8t^2 - 4t^4 + 6t - 3t^3 - 2 + t^2 $$

$$ (PA)(t) = -4t^4 - 3t^3 + 9t^2 + 6t - 2 $$

**(d)**

$$ \left(\frac{P}{A}\right)(-2) $$

$$ \left(\frac{P}{A}\right)(-2) = \frac{4(-2)^2 + 3(-2) - 1}{2 - (-2)^2} $$

$$ \left(\frac{P}{A}\right)(-2) = \frac{4(4) + 3(-2) - 1}{2 - (4)} $$

$$ \left(\frac{P}{A}\right)(-2) = \frac{16 - 6 - 1}{2 - 4} $$

$$ \left(\frac{P}{A}\right)(-2) = \frac{9}{-2} $$

$$ \left(\frac{P}{A}\right)(-2) = -\frac{9}{2} $$

**3.**

Given $h(z) = 7z + 6$ and $f(z) = 4 - z$ compute each of the following.

**(a)**

$$ (fh)(z) $$

$$ (fh)(z) = (4 - z)(7z + 6) $$

$$ (fh)(z) = 28z - 7z^2 + 24 - 6z $$

$$ (fh)(z) = -7z^2 + 22z + 24 $$

**(b)**

$$ (f \circ h)(z) $$

$$ (f \circ h)(z) = f[h(z)] = f[7z + 6] $$

$$ (f \circ h)(z) =  4 - (7z + 6) $$

$$ (f \circ h)(z) =  4 - 7z - 6 $$

$$ (f \circ h)(z) =  -7z - 2 $$

**(c\)**

$$ (h \circ f)(z) $$

$$ (h \circ f)(z) = h[f(z)] = h[4 - z] $$

$$ (h \circ f)(z) = 7(4 - z) + 6 $$

$$ (h \circ f)(z) = 28 - 7z + 6 $$

$$ (h \circ f)(z) = -7z + 34 $$

**(d)**

Given $h(z) = 7z + 6$ and $f(z) = 4 - z$ compute each of the following.

$$ (h \circ h)(z) $$

$$ (h \circ h)(z) =  h[h(z)] = h[7z + 6] $$

$$ (h \circ h)(z) = 7(7z + 6) + 6 $$

$$ (h \circ h)(z) = 49z + 42 + 6 $$

$$ (h \circ h)(z) = 49z + 48 $$

**4.**

Given $f(x) = 6x^2$ and $g(x) = x^2 + 3x - 1$ compute each of the following.

**(a)**

$$ (gf)(x) $$

$$ (gf)(x) = (x^2 + 3x - 1)(6x^2) $$

$$ (gf)(x) = x^2(6x^2) + 3x(6x^2) - 1(6x^2) $$

$$ (gf)(x) = 6x^4 + 18x^3 - 6x^2 $$

**(b)**

$$ (f \circ g)(x) $$

$$ (f \circ g)(x) = f[g(x)] = f[x^2 + 3x - 1] $$

$$ (f \circ g)(x) = 6(x^2 + 3x - 1)^2 $$

$$ (f \circ g)(x) = 6(x^2 + 3x - 1)(x^2 + 3x - 1) $$

$$ (f \circ g)(x) = 6(x^2(x^2 + 3x -1) + 3x(x^2 + 3x - 1) - 1(x^2 + 3x - 1)) $$

$$ (f \circ g)(x) = 6(x^4 + 3x^3 - x^2 + 3x^3 + 9x^2 - 3x - x^2 - 3x + 1) $$

$$ (f \circ g)(x) = 6x^4 + 18x^3 - 6x^2 + 18x^3 + 54x^2 - 18x - 6x^2 - 18x + 6 $$

$$ (f \circ g)(x) = 6x^4 + 36x^3 + 42x^2 - 36x + 6 $$

**(c\)**

$$ (g \circ f)(x) $$

$$ (g \circ f)(x) = g[f(x)] = g[6x^2] $$

$$ (g \circ f)(x) = (6x^2)^2 + 3(6x^2) - 1 $$

$$ (g \circ f)(x) = 36x^4 + 18x^2 - 1 $$

**(d)**

$$ (f \circ f)(x) $$

$$ (f \circ f)(x) = f[f(x)] = f[6x^2] $$

$$ (f \circ f)(x) = 6(6x^2)^2 $$

$$ (f \circ f)(x) = 6(6x^2)(6x^2) $$

$$ (f \circ f)(x) = 6(36x^4) $$

$$ (f \circ f)(x) = 216x^4 $$

**5.**

Given $R(t) = \sqrt{t} - 2$ and $A(t) = (t + 2)^2$, $t \geq 0$ compute each of
the following.

**(a)**

$$ (R \circ A)(t) = R[A(t)] = R[(t + 2)^2] $$

$$ (R \circ A)(t) = \sqrt{(t + 2)^2} - 2$$

$$ (R \circ A)(t) = t + 2 - 2 $$

$$ (R \circ A)(t) = t $$

**(b)**

$$ (A \circ R)(t) $$

$$ (A \circ R)(t) = A[R(t)] = A[\sqrt{t} - 2] $$

$$ (A \circ R)(t) = ((\sqrt{t} - 2) + 2)^2 $$

$$ (A \circ R)(t) = (\sqrt{t} - 2 + 2)^2 $$

$$ (A \circ R)(t) = (\sqrt{t})^2 $$

$$ (A \circ R)(t) = t $$

---

## Assignment Problems

**1.**

Given $f(x) = x + 12$ and $g(x) = 9 + 4x$ compute each of the following.

**(a)**

$$ f + g $$

$$ f + g = (x + 12) + (9 + 4x) $$

$$ f + g = x + 12 + 9 + 4x $$

$$ f + g = 5x + 21 $$

**(b)**

$$ (f - g)(1) $$

$$ (f - g)(1) = (1 + 12) - (9 + 4(1)) $$

$$ (f - g)(1) = 1 + 12 - 9 - 4 $$

$$ (f - g)(1) = 0 $$

**(c\)**

$$ (fg)(x) $$

$$ (fg)(x) = (x + 12)(9 + 4x) $$

$$ (fg)(x) = 9x + 108 + 4x^2 + 48x $$

$$ (fg)(x) = 4x^2 + 57x + 108 $$

**(d)**

$$ \frac{f}{g} $$

$$ \frac{f}{g} = \frac{x + 12}{9 + 4x} $$

**2.**

Given $h(w) = w^2 - 4w$ and $f(w) = 2 + w^2$ compute each of the following.

**(a)**

$$ (h - f)(w) $$

$$ (h - f)(w) = (w^2 - 4w) - (2 + w^2) $$

$$ (h - f)(w) = w^2 - 4w - 2 - w^2 $$

$$ (h - f)(w) = -4w - 2 $$

**(b)**

$$ (f + h)(-4) $$

$$ (f + h)(-4) = (2 + (-4)^2) + ((-4)^2 - 4(-4)) $$

$$ (f + h)(-4) = (2 + 16) + (16 - 4(-4)) $$

$$ (f + h)(-4) = (18) + (16 + 16) $$

$$ (f + h)(-4) = 18 + 32 $$

$$ (f + h)(-4) = 50 $$

**(c\)**

$$ fh $$

$$ fh = (2 + w^2)(w^2 - 4w) $$

$$ fh = 2w^2 + w^4 - 8w - 4w^3  $$

$$ fh = w^4 - 4w^3 + 2w^2 - 8w $$

**(d)**

$$ \left(\frac{h}{f}\right)(w) $$

$$ \left(\frac{h}{f}\right)(w) = \frac{w^2 - 4w}{2 + w^2} $$

**3.**

Given $A(x) = 6x - 1$ and $P(x) = \dfrac{1}{4 - x}$ compute each of the
following.

**(a)**

$$ (A + P)(0) $$

$$ (A + P)(0) = (6(0) - 1) + \left(\frac{1}{4 - (0)}\right) $$

$$ (A + P)(0) = -1 + \frac{1}{4} $$

$$ (A + P)(0) = -\frac{3}{4} $$

**(b)**

$$ (P - A)(-2) $$

$$ (P - A)(-2) = \left(\frac{1}{4 - (-2)}\right) - (6(-2) - 1) $$

$$ (P - A)(-2) = \left(\frac{1}{6}\right) - (-12 - 1) $$

$$ (P - A)(-2) = \frac{1}{6} - (-13) $$

$$ (P - A)(-2) = \frac{1}{6} + 13 $$

$$ (P - A)(-2) = \frac{79}{6} $$

**(c\)**

$$ AP $$

$$ AP = (6x - 1)\left(\frac{1}{4 - x}\right) $$

$$ AP = \frac{6x - 1}{4 - x} $$

**(d)**

$$ \left(\frac{A}{P}\right)(x) $$

$$ \left(\frac{A}{P}\right)(x) = \frac{6x - 1}{\dfrac{1}{4 - x}} $$

$$ \left(\frac{A}{P}\right)(x) = (6x - 1)(4 - x) $$

$$ \left(\frac{A}{P}\right)(x) = 24x - 4 - 6x^2 + x $$

$$ \left(\frac{A}{P}\right)(x) = -6x^2 + 25x - 4 $$

**4.**

Given $f(t) = 2t + 9$ and $g(t) = 2t - 1$ compute each of the following.

**(a)**

$$ (fg)(t) $$

$$ (fg)(t) = (2t + 9)(2t - 1) $$

$$ (fg)(t) = 4t^2 + 18t - 2t - 9 $$

$$ (fg)(t) = 4t^2 + 16t - 9 $$

**(b)**

$$ (f \circ g)(t) $$

$$ (f \circ g)(t) = f[g(t)] = f[2t - 1] $$

$$ (f \circ g)(t) = 2(2t - 1) + 9 $$

$$ (f \circ g)(t) = 4t - 2 + 9 $$

$$ (f \circ g)(t) = 4t + 7 $$

**(c\)**

$$ (g \circ f)(t) $$

$$ (g \circ f)(t) = g[f(t)] = g[2t + 9] $$

$$ (g \circ f)(t) =  2(2t + 9) - 1 $$

$$ (g \circ f)(t) =  4t + 18 - 1 $$

$$ (g \circ f)(t) =  4t + 17 $$

**(d)**

$$ (g \circ g)(t) $$

$$ (g \circ g)(t) =  g[g(t)] = g[2t - 1] $$

$$ (g \circ g)(t) = 2(2t - 1) - 1 $$

$$ (g \circ g)(t) = 4t - 2 - 1 $$

$$ (g \circ g)(t) = 4t - 3 $$

**5.**

Given $h(x) = x^2 + 1$ and $g(x) = 6 - 4x$ compute each of the following.

**(a)**

$$ (gh)(x) $$

$$ (gh)(x) = (6 - 4x)(x^2 + 1) $$

$$ (gh)(x) = 6x^2 - 4x^3 + 6 - 4x $$

$$ (gh)(x) = -4x^3 + 6x^2 - 4x + 6 $$

**(b)**

$$ (g \circ h)(x) $$

$$ (g \circ h)(x) = g[h(x)] = g[x^2 + 1] $$

$$ (g \circ h)(x) = 6 - 4(x^2 + 1) $$

$$ (g \circ h)(x) = 6 - 4x^2 - 4 $$

$$ (g \circ h)(x) = -4x^2 + 2 $$

**(c\)**

$$ (h \circ g)(x) $$

$$ (h \circ g)(x) = h[g(x)] = h[6 - 4x] $$

$$ (h \circ g)(x) = (6 - 4x)^2 + 1 $$

$$ (h \circ g)(x) = (6 - 4x)(6 - 4x) + 1 $$

$$ (h \circ g)(x) = (36 - 24x - 24x + 16x^2) + 1 $$

$$ (h \circ g)(x) = 36 - 48x + 16x^2 + 1 $$

$$ (h \circ g)(x) = 37 - 48x + 16x^2 $$

$$ (h \circ g)(x) = 16x^2 - 48x + 37 $$

**(d)**

$$ (h \circ h)(x) $$

$$ (h \circ h)(x) = h[h(x)] = h[x^2 + 1] $$

$$ (h \circ h)(x) = (x^2 + 1)^2 + 1 $$

$$ (h \circ h)(x) = (x^2 + 1)(x^2 + 1) + 1 $$

$$ (h \circ h)(x) = x^4 + 2x^2 + 1 + 1 $$

$$ (h \circ h)(x) = x^4 + 2x^2 + 2 $$

**6.**

Given $A(w) = 2w^2 + 9$ and $R(w) = 1 - 2w - w^2$ copute each of the following.

**(a)**

$$ (AR)(w) $$

$$ (AR)(w) = (2w^2 + 9)(1 - 2w - w^2) $$

$$ (AR)(w) = 2w^2(1 - 2w - w^2) + 9(1 - 2w - w^2) $$

$$ (AR)(w) = 2w^2 - 4w^3 - 2w^4 + 9 - 18w - 9w^2 $$

$$ (AR)(w) = -2w^4 - 4w^3 - 7w^2 - 18w + 9 $$

**(b)**

$$ (A \circ R)(w) $$

$$ (A \circ R)(w) = A[R(w)] = A[1 - 2w - w^2] $$

$$ (A \circ R)(w) = 2(1 - 2w - w^2)^2 + 9 $$

$$ (A \circ R)(w) = 2(1 - 2w - w^2)(1 - 2w - w^2) + 9 $$

$$ (A \circ R)(w) = 2(1(1 - 2w - w^2) - 2w(1 - 2w - w^2) - w^2(1 - 2w - w^2)) + 9 $$

$$ (A \circ R)(w) = 2(1 - 2w - w^2 - 2w + 4w^2 + 2w^3 - w^2 + 2w^3 + w^4) + 9 $$

$$ (A \circ R)(w) = 2 - 4w - 2w^2 - 4w + 8w^2 + 4w^3 - 2w^2 + 4w^3 + 2w^4 + 9 $$

$$ (A \circ R)(w) = 2w^4 + 4w^3 + 4w^3 - 2w^2 + 8w^2 - 2w^2 - 4w - 4w + 2 + 9 $$

$$ (A \circ R)(w) = 2w^4 + 8w^3 + 4w^2 - 8w + 11 $$

**(c\)**

$$ (R \circ A)(w) $$

$$ (R \circ A)(w) = R[A(w)] = R[2w^2 + 9] $$

$$ (R \circ A)(w) = 1 - 2(2w^2 + 9) - (2w^2 + 9)^2 $$

$$ (R \circ A)(w) = 1 - 4w^2 - 18 - (2w^2 + 9)(2w^2 + 9) $$

$$ (R \circ A)(w) = 1 - 4w^2 - 18 - (4w^4 + 36w^2 + 81) $$

$$ (R \circ A)(w) = 1 - 4w^2 - 18 - 4w^4 - 36w^2 - 81 $$

$$ (R \circ A)(w) = -4w^4 - 4w^2 - 36w^2 + 1 - 18 - 81 $$

$$ (R \circ A)(w) = -4w^4 - 40w^2 - 98 $$

**(d)**

$$ (A \circ A)(w) $$

$$ (A \circ A)(w) = A[A(w)] = A[2w^2 + 9] $$

$$ (A \circ A)(w) = 2(2w^2 + 9)^2 + 9 $$

$$ (A \circ A)(w) = 2(2w^2 + 9)(2w^2 + 9) + 9 $$

$$ (A \circ A)(w) = 2(4w^4 + 36w^2 + 81) + 9 $$

$$ (A \circ A)(w) = 8w^4 + 72w^2 + 162 + 9 $$

$$ (A \circ A)(w) = 8w^4 + 72w^2 + 171 $$

**7.**

Given $f(x) = 9x^2 + 10x + 12$ and $g(x) = 2$ compute each of the following.

**(a)**

$$ (fg)(x) $$

$$ (fg)(x) = (9x^2 + 10x + 12)(2) $$

$$ (fg)(x) = 18x^2 + 20x + 24 $$

**(b)**

$$ (g \circ f)(x) $$

$$ (g \circ f)(x) = g[f(x)] = g[9x^2 + 10x + 12] $$

$$ (g \circ f)(x) = 2 $$

**(c\)**

$$ (f \circ g)(x) $$

$$ (f \circ g)(x) = f[g(x)] = f[2] $$

$$ (f \circ g)(x) = 9(2)^2 + 10(2) + 12 $$

$$ (f \circ g)(x) = 9(4) + 20 + 12 $$

$$ (f \circ g)(x) = 36 + 20 + 12 $$

$$ (f \circ g)(x) = 68 $$

**(d)**

$$ (g \circ g)(x) $$

$$ (g \circ g)(x) = g[g(x)] = g[2] $$

$$ (g \circ g)(x) = 2 $$

**8.**

Given $g(t) = t + 1$ and $h(t) = \dfrac{2}{t - 3}$ compute each of the
following.

**(a)**

$$ (gh)(t) $$

$$ (gh)(t) = (t + 1)\left(\frac{2}{t - 3}\right) $$

$$ (gh)(t) = \frac{2(t + 1)}{t - 3} $$

$$ (gh)(t) = \frac{2t + 2}{t - 3} $$

**(b)**

$$ (g \circ h)(t) $$

$$ (g \circ h)(t) = g[h(t)] = g\left[\frac{2}{t - 3}\right] $$

$$ (g \circ h)(t) = \left(\frac{2}{t - 3}\right) + 1 $$

$$ (g \circ h)(t) = \frac{2 + (t - 3)}{t - 3} $$

$$ (g \circ h)(t) = \frac{t - 1}{t - 3} $$

**(c\)**

$$ (h \circ g)(t) $$

$$ (h \circ g)(t) = h[g(t)] = h[t + 1] $$

$$ (h \circ g)(t) = \frac{2}{(t + 1) - 3} $$

$$ (h \circ g)(t) = \frac{2}{t - 2}$$

**(d)**

$$ (h \circ h)(t) $$

$$ (h \circ h)(t) = h[h(t)] = h\left[\frac{2}{t - 3}\right] $$

$$ (h \circ h)(t) = \frac{2}{\left(\dfrac{2}{t - 3}\right) - 3} $$

$$ (h \circ h)(t) = \frac{2}{\dfrac{2 - 3(t - 3)}{t - 3}} $$

$$ (h \circ h)(t) = \frac{2}{\dfrac{-3t + 11}{t - 3}} $$

$$ (h \circ h)(t) = 2\left(\frac{t - 3}{-3t + 11}\right) $$

$$ (h \circ h)(t) = \frac{2(t - 3)}{-3t + 11} $$

$$ (h \circ h)(t) = \frac{2t - 6}{-3t + 11} $$

**9.**

Given $f(x) = \dfrac{1}{2}x - 3$ and $g(x) = 2x + 6$, $t \geq 0$ compute each of
the following.

**(a)**

$$ (f \circ g)(x) $$

$$ (f \circ g)(x) = f[g(x)] = f[2x + 6] $$

$$ (f \circ g)(x) = \frac{1}{2}(2x + 6) - 3 $$

$$ (f \circ g)(x) = x + 3 - 3 $$

$$ (f \circ g)(x) = x $$

**(b)**

$$ (g \circ f)(x) $$

$$ (g \circ f)(x) = g[f(x)] = g\left[\frac{1}{2}x - 3\right] $$

$$ (g \circ f)(x) = 2\left(\frac{1}{2}x - 3\right) + 6$$

$$ (g \circ f)(x) = x - 6 + 6 $$

$$ (g \circ f)(x) = x $$

**10.**

Given $h(w) = \dfrac{1}{w - 3}$ and $f(w) = \dfrac{1 + 3w}{w}$ compute each of
the following.

**(a)**

$$ (h \circ f)(w) $$

$$ (h \circ f)(w) = h[f(w)] = h\left[\frac{1 + 3w}{w}\right] $$

$$ (h \circ f)(w) = \frac{1}{\left(\dfrac{1 + 3w}{w}\right) - 3} $$

$$ (h \circ f)(w) = \frac{1}{\dfrac{1 + 3w - 3w}{w}} $$

$$ (h \circ f)(w) = \frac{1}{\dfrac{1}{w}} $$

$$ (h \circ f)(w) = 1\left(\frac{w}{1}\right) $$

$$ (h \circ f)(w) = w $$

**(b)**

$$ (f \circ h)(w) $$

$$ (f \circ h)(w) = f[h(w)] = f\left[\frac{1}{w - 3}\right] $$

$$ (f \circ h)(w) = \frac{1 + 3\left(\dfrac{1}{w - 3}\right)}{\left(\dfrac{1}{w - 3}\right)} $$

$$ (f \circ h)(w) = \frac{1 + \dfrac{3}{w - 3}}{\left(\dfrac{1}{w - 3}\right)} $$

$$ (f \circ h)(w) = \frac{\dfrac{(w - 3) + 3}{w - 3}}{\left(\dfrac{1}{w - 3}\right)} $$

$$ (f \circ h)(w) = \frac{\dfrac{w}{w - 3}}{\left(\dfrac{1}{w - 3}\right)} $$

$$ (f \circ h)(w) = \left(\frac{w}{w - 3}\right)\left(\frac{w - 3}{1}\right) $$

$$ (f \circ h)(w) = w $$
