# 2.10 Equations With Radicals

---

**Example 1**

Solve $x = \sqrt{x + 6}$

$$ x = \sqrt{x + 6} $$

$$ x^2 = (\sqrt{x + 6})^2 $$

$$ x^2 = x + 6 $$

$$ x^2 - x - 6 = 0 $$

$$ (x - 3)(x + 2) = 0 $$

$$ x = 3 $$

$$ (3) = \sqrt{(3) + 6} $$

$$ 3 = \sqrt{9} $$

$$ 3 = 3 $$

$$ x = -2 $$

$$ (-2) = \sqrt{(-2) + 6} $$

$$ -2 = \sqrt{4} $$

$$ -2 \neq 2 $$

$$ x = \{3\} $$

---

**Example 2**

Solve each of the following equations.

**(a)**

$$ y + \sqrt{y - 4} = 4 $$

$$ \sqrt{y - 4} = 4 - y $$

$$ (\sqrt{y - 4})^2 = (4 - y)^2 $$

$$ y - 4 = (4 - y)(4 - y) $$

$$ y - 4 = 16 - 4y - 4y + y^2 $$

$$ 16 - 4y - 4y + y^2 = y - 4 $$

$$ y^2 - 8y + 16 = y - 4  $$

$$ y^2 - 9y + 20 = 0 $$

$$ (y - 5)(y - 4) = 0 $$

$$ y = 5 $$

$$ (5) + \sqrt{(5) - 4} = 4 $$

$$ 5 + \sqrt{1} = 4 $$

$$ 5 + 1 = 4 $$

$$ 6 \neq 4 $$

$$ y = 4 $$

$$ (4) + \sqrt{(4) - 4} = 4 $$

$$ 4 + \sqrt{0} = 4 $$

$$ 4 + 0 = 4 $$

$$ 4 = 4 $$

$$ y = \{4\} $$

**(b)**

$$ 1 = t + \sqrt{2t - 3} $$

$$ 1 - t = \sqrt{2t - 3} $$

$$ (1 - t)^2 = (\sqrt{2t - 3})^2 $$

$$ (1 - t)(1 - t) = 2t - 3 $$

$$ 1 - t - t + t^2 = 2t - 3 $$

$$ t^2 - 2t + 1 = 2t - 3 $$

$$ t^2 - 4t + 4 = 0 $$

$$ (t - 2)(t - 2) = 0 $$

$$ t = 2 $$

$$ 1 = (2) + \sqrt{2(2) - 3} $$

$$ 1 = 2 + \sqrt{4 - 3} $$

$$ 1 = 2 + \sqrt{1} $$

$$ 2 = 2 + 1 $$

$$ 2 \neq 3 $$

$$ \emptyset $$

**(c\)**

$$ \sqrt{5z + 6} - 2 = z $$

$$ \sqrt{5z + 6} = z + 2 $$

$$ (\sqrt{5z + 6})^2 = (z + 2)^2 $$

$$ 5z + 6 = (z + 2)(z + 2) $$

$$ 5z + 6 = z^2 + 2z + 2z + 4 $$

$$ 5z + 6 = z^2 + 4z + 4 $$

$$ 0 = z^2 - z - 2 $$

$$ 0 = (z - 2)(z + 1) $$

$$ z = 2 $$

$$ \sqrt{5(2) + 6} - 2 = (2) $$

$$ \sqrt{10 + 6} - 2 = 2 $$

$$ \sqrt{16} - 2 = 2 $$

$$ 4 - 2 = 2 $$

$$ 2 = 2 $$

$$ z = -1 $$

$$ \sqrt{5(-1) + 6} - 2 = (-1) $$

$$ \sqrt{-5 + 6} - 2 = -1 $$

$$ \sqrt{1} - 2 = -1 $$

$$ 1 - 2 = -1 $$

$$ -1 = -1 $$

$$ z = \{2, -1\} $$

---

**Example 3**

Solve each of the following equations.

**(a)**

$$ \sqrt{2x - 1} - \sqrt{x - 4} = 2 $$

$$ \sqrt{2x - 1} = 2 + \sqrt{x - 4} $$

$$ (\sqrt{2x - 1})^2 = (2 + \sqrt{x - 4})^2 $$

$$ 2x - 1 = (2 + \sqrt{x - 4})(2 + \sqrt{x - 4}) $$

$$ 2x - 1 = 4 + 2\sqrt{x - 4} + 2\sqrt{x - 4} + (x - 4) $$

$$ 2x - 1 = 4 + 4\sqrt{x - 4} + x - 4 $$

$$ 2x - 1 = 4\sqrt{x - 4} + x $$

$$ x - 1 = 4\sqrt{x - 4} $$

$$ (x - 1)^2 = (4\sqrt{x - 4})^2 $$

$$ (x - 1)(x - 1) = 16(x - 4) $$

$$ x^2 - 2x + 1 = 16x - 64 $$

$$ x^2 - 18x + 65 = 0 $$

$$ (x - 13)(x - 5) = 0 $$

$$ x = 13 $$

$$ \sqrt{2(13) - 1} - \sqrt{(13) - 4} = 2 $$

$$ \sqrt{26 - 1} - \sqrt{9} = 2 $$

$$ \sqrt{25} - \sqrt{9} = 2 $$

$$ 5 - 3 = 2 $$

$$ 2 = 2 $$

$$ x = 5 $$

$$ \sqrt{2(5) - 1} - \sqrt{(5) - 4} = 2 $$

$$ \sqrt{10 - 1} - \sqrt{1} = 2 $$

$$ \sqrt{9} - \sqrt{1} = 2 $$

$$ 3 - 1 = 2 $$

$$ x = \{13, 5\} $$

**(b)**

$$ \sqrt{t + 7} + 2 = \sqrt{3 - t} $$

$$ \sqrt{t + 7} = \sqrt{3 - t} - 2 $$

$$ (\sqrt{t + 7})^2 = (\sqrt{3 - t} - 2)^2 $$

$$ t + 7 = (\sqrt{3 - t} - 2)(\sqrt{3 - t} - 2) $$

$$ t + 7 = (3 - t) - 4(\sqrt{3 - t}) + 4 $$

$$ t + 7 = 3 - t - 4(\sqrt{3 - t}) + 4 $$

$$ t + 7 = 7 - t - 4(\sqrt{3 - t}) $$

$$ t = -t -4(\sqrt{3 - t}) $$

$$ 2t = -4(\sqrt{3 - t}) $$

$$ (2t)^2 = (-4(\sqrt{3 - t}))^2 $$

$$ 4t^2 = 16(3 - t) $$

$$ 4t^2 = 48 - 16t $$

$$ 4t^2 + 16t - 48 = 0 $$

$$ (2t - 4)(2t + 12) = 0 $$

$$ 2t - 4 = 0 $$

$$ 2t = 4 $$

$$ t = 2 $$

$$ \sqrt{(2) + 7} + 2 = \sqrt{3 - (2)} $$

$$ \sqrt{9} + 2 = \sqrt{1} $$

$$ 3 + 2 = 1 $$

$$ 5 \neq 1 $$

$$ 2t + 12 = 0 $$

$$ 2t = -12 $$

$$ t = -6 $$

$$ \sqrt{(-6) + 7} + 2 = \sqrt{3 - (-6)} $$

$$ \sqrt{1} + 2 = \sqrt{9} $$

$$ 1 + 2 = 3 $$

$$ 3 = 3 $$

$$ t = \{-6\} $$

---

## Practice Problems

**1.**

$$ 2x = \sqrt{x + 3} $$

$$ (2x)^2 = \left(\sqrt{x + 3}\right)^2 $$

$$ 4x^2 = x + 3 $$

$$ 4x^2 - x - 3 = 0 $$

$$ (4x + 3)(x - 1) = 0 $$

$$ 4x + 3 = 0 $$

$$ 4x = -3 $$

$$ x = -\frac{3}{4} $$

$$ 2\left(-\frac{3}{4}\right) = \sqrt{\left(-\frac{3}{4}\right) + 3} $$

$$ -\frac{3}{2} = \sqrt{\left(-\frac{3}{4}\right) + 3} $$

$$ -\frac{3}{2} = \sqrt{\frac{9}{4}} $$

$$ -\frac{3}{2} \neq \frac{3}{2} $$

$$ x = \left\{1\right\} $$

**2.**

$$ \sqrt{33 - 2x} = x + 1 $$

$$ (\sqrt{33 - 2x})^2 = (x + 1)^2 $$

$$ 33 - 2x = (x + 1)(x + 1) $$

$$ 33 - 2x = x^2 + 2x + 1 $$

$$ 0 = x^2 + 4x - 32 $$

$$ 0 = (x + 8)(x - 4) $$

$$ x = -8 $$

$$ \sqrt{33 - 2(-8)} = (-8) + 1 $$

$$ \sqrt{33 + 16} = -7 $$

$$ \sqrt{49} = -7 $$

$$ 7 \neq -7 $$

$$ x = 4 $$

$$ \sqrt{33 - 2(4)} = (4) + 1 $$

$$ \sqrt{33 - 8} = 5 $$

$$ \sqrt{25} = 5 $$

$$ 5 = 5 $$

$$ x = \{4\} $$

**3.**

$$ 7 = \sqrt{39 + 3x} - x $$

$$ 7 + x = \sqrt{39 + 3x} $$

$$ (7 + x)^2 = (\sqrt{39 + 3x})^2 $$

$$ (7 + x)(7 + x) = 39 + 3x $$

$$ 49 + 14x + x^2 = 39 + 3x $$

$$ x^2 + 11x + 10 = 0 $$

$$ (x + 10)(x + 1) = 0 $$

$$ x = -10 $$

$$ 7 = \sqrt{39 + 3(-10)} - (-10) $$

$$ 7 = \sqrt{39 - 30} + 10 $$

$$ 7 = \sqrt{9} + 10 $$

$$ 7 = 3 + 10 $$

$$ 7 \neq 13 $$

$$ x = -1 $$

$$ 7 = \sqrt{39 + 3(-1)} - (-1) $$

$$ 7 = \sqrt{39 - 3} + 1 $$

$$ 7 = \sqrt{36} + 1 $$

$$ 7 = 6 + 1 $$

$$ 7 = 7 $$

$$ x = \{-1\} $$

**4.**

$$ x = 1 + \sqrt{2x - 2} $$

$$ x - 1 = \sqrt{2x - 2} $$

$$ (x - 1)^2 = (\sqrt{2x - 2})^2 $$

$$ (x - 1)(x - 1) = 2x - 2 $$

$$ x^2 - 2x + 1 = 2x - 2 $$

$$ x^2 - 4x + 3 = 0 $$

$$ (x - 3)(x - 1) = 0 $$

$$ x = 3 $$

$$ (3) = 1 + \sqrt{2(3) - 2} $$

$$ 3 = 1 + \sqrt{6 - 2} $$

$$ 3 = 1 + \sqrt{4} $$

$$ 3 = 1 + 2 $$

$$ 3 = 3 $$

$$ x = 1 $$

$$ (1) = 1 + \sqrt{2(1) - 2} $$

$$ 1 = 1 + \sqrt{2 - 2} $$

$$ 1 = 1 + \sqrt{0} $$

$$ 1 = 1 + 0 $$

$$ 1 = 1 $$

$$ x = \{3, 1\} $$

**5.**

$$ 1 + \sqrt{1 - x} = \sqrt{2x + 4} $$

$$ (1 + \sqrt{1 - x})^2 = (\sqrt{2x + 4})^2 $$

$$ (1 + \sqrt{1 - x})(1 + \sqrt{1 - x}) = 2x + 4 $$

$$ 1 + 2\sqrt{1 - x} + (1 - x) = 2x + 4 $$

$$ 2\sqrt{1 - x} + 2 - x = 2x +4 $$

$$ 2\sqrt{1 - x} = 3x + 2 $$

$$ (2\sqrt{1 - x})^2 = (3x + 2)^2 $$

$$ 4(1 - x) = (3x + 2)(3x + 2) $$

$$ 4 - 4x = 9x^2 + 12x + 4 $$

$$ 0 = 9x^2 + 16x $$

$$ 0 = x(9x + 16) $$

$$ x = 0 $$

$$ 1 + \sqrt{1 - (0)} = \sqrt{2(0) + 4} $$

$$ 1 + \sqrt{1} = \sqrt{4} $$

$$ 1 + 1 = 2 $$

$$ 2 = 2 $$

$$ 9x + 16 = 0 $$

$$ 9x = -16 $$

$$ x = -\frac{16}{9} $$

$$ 1 + \sqrt{1 - \left(-\frac{16}{9}\right)} = \sqrt{2\left(-\frac{16}{9}\right) + 4} $$

$$ 1 + \sqrt{\frac{25}{9}} = \sqrt{\frac{4}{9}} $$

$$ 1 + \frac{5}{3} = \frac{2}{3} $$

$$ \frac{8}{3} \neq \frac{2}{3} $$

$$ x = \{0\} $$

---

## Assignment Problems

Solve each of the following equations.

**1.**

$$ x = \sqrt{4x - 3} $$

$$ x^2 = 4x - 3 $$

$$ x^2 - 4x + 3 = 0 $$

$$ (x - 3)(x - 1) = 0 $$

$$ x = 3 $$

$$ (3) = \sqrt{4(3) - 3} $$

$$ 3 = \sqrt{12 - 3} $$

$$ 3 = \sqrt{9} $$

$$ 3 = 3 $$

$$ x = 1 $$

$$ (1) = \sqrt{4(1) - 3} $$

$$ 1 = \sqrt{1} $$

$$ 1 = 1 $$

$$ x = \{3, 1\} $$

**2.**

$$ 2x = -\sqrt{3 - x} $$

$$ -2x = \sqrt{3 - x} $$

$$ (-2x)^2 = (\sqrt{3 - x})^2 $$

$$ 4x^2 = 3 - x $$

$$ 4x^2 + x - 3 = 0 $$

$$ (4x - 3)(x + 1) $$

$$ 4x - 3 = 0 $$

$$ 4x = 3 $$

$$ x = \frac{3}{4} $$

$$ 2\left(\frac{3}{4}\right) = -\sqrt{3 - \left(\frac{3}{4}\right)} $$

$$ \frac{3}{2} = -1\left(\sqrt{\frac{9}{4}}\right) $$

$$ \frac{3}{2} = -1\left(\frac{3}{2}\right) $$

$$ \frac{3}{2} \neq -\frac{3}{2} $$

$$ x + 1 = 0 $$

$$ x = -1 $$

$$ 2(-1) = -\sqrt{3 - (-1)} $$

$$ -2 = -1(\sqrt{4}) $$

$$ -2 = -1(2) $$

$$ -2 = -2 $$

$$ x = \{-1\} $$

**3.**

$$ 4 - \sqrt{x + 6} = -x $$

$$ -\sqrt{x + 6} = -x - 4 $$

$$ \sqrt{x + 6} = x + 4 $$

$$ (\sqrt{x + 6})^2 = (x + 4)^2 $$

$$ x + 6 = (x + 4)(x + 4) $$

$$ x + 6 = x^2 + 8x + 16 $$

$$ 0 = x^2 + 7x + 10 $$

$$ 0 = (x + 5)(x + 2) $$

$$ x = -5 $$

$$ 4 - \sqrt{(-5) + 6} = -(-5) $$

$$ 4 - \sqrt{1} = 5 $$

$$ 4 - 1 = 5 $$

$$ 3 \neq 5 $$

$$ x = -2 $$

$$ 4 - \sqrt{(-2) + 6} = -(-2) $$

$$ 4 - \sqrt{4} = 2 $$

$$ 4 - 2 = 2 $$

$$ 2 = 2 $$

$$ x = \{-2\} $$

**4.**

$$ x + 3 = \sqrt{11(x + 3)} $$

$$ (x + 3)^2 = (\sqrt{11(x + 3)})^2 $$

$$ (x + 3)(x + 3) = 11(x + 3) $$

$$ (x + 3)\cancel{(x + 3)} = 11\cancel{(x + 3)} $$

$$ x + 3 = 11 $$

$$ x = 8 $$

$$ (8) + 3 = \sqrt{11((8) + 3)} $$

$$ 11 = \sqrt{11(11)} $$

$$ 11 = \sqrt{121} $$

$$ 11 = 11 $$

$$ x = \{8\} $$

**5.**

$$ x = 8 + \sqrt{22 - 3x} $$

$$ x - 8 = \sqrt{22 - 3x} $$

$$ (x - 8)^2 = (\sqrt{22 - 3x})^2 $$

$$ (x - 8)(x - 8) = 22 - 3x $$

$$ x^2 - 16x + 64 = 22 - 3x $$

$$ x^2 - 13x + 42 = 0  $$

$$ (x - 6)(x - 7) = 0 $$

$$ x = 6 $$

$$ (6) = 8 + \sqrt{22 - 3(6)} $$

$$ 6 = 8 + \sqrt{22 - 18} $$

$$ 6 = 8 + \sqrt{4} $$

$$ 6 = 8 + 2 $$

$$ 6 \neq 10 $$

$$ x = 7 $$

$$ (7) = 8 + \sqrt{22 - 3(7)} $$

$$ 7 = 8 + \sqrt{22 - 21} $$

$$ 7 = 8 + \sqrt{1} $$

$$ 7 = 8 + 1 $$

$$ 7 \neq 9 $$

$$ \emptyset $$

**6.**

$$ 2 - x = \sqrt{8 - 7x} $$

$$ (2 - x)^2 = (\sqrt{8 - 7x})^2 $$

$$ (2 - x)(2 - x) = 8 - 7x $$

$$ 4 - 4x + x^2 = 8 - 7x $$

$$ x^2 - 4x + 4 = 8 - 7x $$

$$ x^2 + 3x - 4 = 0 $$

$$ (x + 4)(x - 1) = 0 $$

$$ x = -4 $$

$$ 2 - (-4) = \sqrt{8 - 7(-4)} $$

$$ 6 = \sqrt{36} $$

$$ 6 = 6 $$

$$ x = 1 $$

$$ 2 - (1) = \sqrt{8 - 7(1)} $$

$$ 1 = \sqrt{1} $$

$$ 1 = 1 $$

$$ x = \{-4,1\} $$

**7.**

$$ \sqrt{1 + 3x} = 4 + \sqrt{5 - x} $$

$$ (\sqrt{1 + 3x})^2 = (4 + \sqrt{5 - x})^2 $$

$$ 1 + 3x = (4 + \sqrt{5 - x})(4 + \sqrt{5 - x}) $$

$$ 1 + 3x = 16 + 2\sqrt{5 - x} + (5 - x) $$

$$ 1 + 3x = 21 + 2\sqrt{5 - x} - x $$

$$ -20 + 4x = 2\sqrt{5 - x} $$

$$ (-20 + 4x)^2 = (2\sqrt{5 - x})^2 $$

$$ (-20 + 4x)(-20 + 4x) = 4(5 - x) $$

$$ 400 - 160x + 16x^2 = 20 - 4x $$

$$ 16x^2 - 160x + 400 = 20 - 4x $$

$$ 16x^2 -156x + 380 = 0 $$

$$ x = \frac{-(-156) \pm \sqrt{(-156)^2 - 4(16)(380)}}{2(16)} $$

$$ x = \frac{156 \pm 4}{32} $$

$$ x = \frac{156 + 4}{32} $$

$$ x = 5 $$

$$ \sqrt{1 + 3(5)} = 4 + \sqrt{5 - (5)} $$

$$ \sqrt{1 + 15} = 4 + \sqrt{0} $$

$$ \sqrt{16} = 4 + 0 $$

$$ 4 = 4 $$

$$ x = \frac{156 - 4}{32} $$

$$ x = \frac{19}{4} $$

$$ \sqrt{1 + 3\left(\frac{19}{4}\right)} = 4 + \sqrt{5 - \left(\frac{19}{4}\right)} $$

$$ \sqrt{1 + \frac{57}{4}} = 4 + \sqrt{\frac{1}{4}} $$

$$ \sqrt{\frac{61}{4}} = \frac{9}{2} $$

$$ \frac{\sqrt{61}}{2} \neq \frac{9}{2} $$

$$ x = \{5\} $$

**8.**

$$ \sqrt{x - 3} + \sqrt{x + 1} = 2 $$

$$ \sqrt{x - 3} = 2 - \sqrt{x + 1} $$

$$ (\sqrt{x - 3})^2 = (2 - \sqrt{x + 1})^2 $$

$$ x - 3 = (2 - \sqrt{x + 1})(2 - \sqrt{x + 1}) $$

$$ x - 3 = 4 - 4\sqrt{x + 1} + (x + 1) $$

$$ x - 3 = 5 + x - 4\sqrt{x + 1} $$

$$ \cancel{x} - 3 = 5 + \cancel{x} - 4\sqrt{x + 1} $$

$$ -8 = -4\sqrt{x + 1} $$

$$ 2 = \sqrt{x + 1} $$

$$ (2)^2 = (\sqrt{x + 1})^2 $$

$$ 4 = x + 1 $$

$$ 3 = x $$

$$ \sqrt{(3) - 3} + \sqrt{(3) + 1} = 2 $$

$$ \sqrt{0} + \sqrt{4} = 2 $$

$$ 0 + 2 = 2 $$

$$ 2 = 2 $$

$$ x = \{3\} $$
