# 2.11 Linear Inequalities

**Interval Notation**

| Inequality        | Interval Notation |
| ----------------- | ----------------- |
| $a \leq x \leq b$ | $[a, b]$          |
| $a < x < b$       | $(a, b)$          |
| $a \leq x < b$    | $[a, b)$          |
| $a < x \leq b$    | $(a, b]$          |
| $x > a$           | $(a, \infty)$     |
| $x \geq a$        | $[a, \infty)$     |
| $x < b$           | $(-\infty, b)$    |
| $x \leq b$        | $(-\infty, b]$    |

**Solving For Inequalities**

1. If $a < b$ then $a + c < b + c$ and $a - c < b - c$ for any number $c$. In
   other words, we can add or subtract a number to both sides of the inequality
   and we don't change the inequality itself.

2. If $a < b$ and $c > 0$ then $ac < bc$ and $\frac{a}{c} < \frac{b}{c}$. So,
   provided $c$ is a positive number we can multiply or divide both sides of an
   inequality by the number without changing the inequality.

3. If $a < b$ and $c < 0$ then $ac > bc$ and $\frac{a}{c} > \frac{b}{c}$. In
   this case, unlike the previous fact, if $c$ is negative we need to flip the
   direction of the inequality when we multiply or divide both sides by the
   inequality by $c$.

---

**Example 1**

Solve the following inequalities. Give both inequality and interval notation
forms of the solution.

**(a)**

$$ -2(m - 3) < 5(m + 1) - 12 $$

$$ -2m + 6 < 5m + 5 - 12 $$

$$ -2m + 6 < 5m - 7 $$

$$ 13 < 7m $$

$$ \frac{13}{7} < m $$

$$ \left(\frac{13}{7}, \infty\right) $$

**(b)**

$$ 2(1 - x) + 5 \leq 3(2x - 1) $$

$$ 2 - 2x + 5 \leq 6x - 3 $$

$$ 7 - 2x \leq 6x - 3 $$

$$ -8x \leq -10 $$

$$ x \geq \frac{5}{4} $$

$$ \left[\frac{5}{4}, \infty\right) $$

---

**Example 2**

Solve each of the following Inequalities. Give both inequality and interval
notation forms for the solution.

**(a)**

$$ -6 \leq 2(x - 5) < 7 $$

$$ -6 \leq 2x - 10 < 17 $$

$$ 4 \leq 2x < 17 $$

$$ 2 \leq x < \frac{17}{2} $$

$$ \left[2, \frac{17}{2}\right) $$

**(b)**

$$ -3 < \frac{3}{2}(2 - x) \leq 5 $$

$$ -2 < 2 - x \leq \frac{10}{3} $$

$$ -4 < -x \leq \frac{4}{3} $$

$$ 4 > x \geq -\frac{4}{3} $$

$$ \left[-\frac{4}{3}, 4\right) $$

**(c\)**

$$ -14 < -7(3x + 2) < 1 $$

$$ 2 > 3x + 2 > -\frac{1}{7} $$

$$ 0 > 3x > -\frac{15}{7} $$

$$ 0 > x > -\frac{5}{7} $$

$$ \left(-\frac{5}{7}, 0\right) $$

---

**Example 3**

If $-1 < x < 4$ then determine $a$ and $b$ in $a < 2x + 3 < b$.

This is easier than it may appear at first. All we are really going to do is
start with the given inequality aand then manipulate the middle term to look
like the second inequality. Again, we'll need to remember that whatever we do to
the middle term we'll also need to do to the two outer terms.

So first we'll multiply everything by 2.

$$ -2 < 2x < 8 $$

Now add 3 to everything.

$$ 1 < 2x + 3 < 11 $$

We've now got the middle term identical to the second inequality in the problems
statement and so all we need to do is pick off $a$ and $b$. From this
ineqeuality we can see that $a = 1$ and $b = 11$.

---

## Practice Problems

For problems 1 – 6 solve each of the following inequalities. Give the solution
in both inequality and interval notations.

**1.**

$$ 4(z + 2) - 1 > 5 - 7(4 - z) $$

$$ 4z + 8 - 1 > 5 - 28 + 7z $$

$$ 4z + 7 > 7z - 23 $$

$$ -3z > -30 $$

$$ z < 10 $$

$$ (-\infty, 10) $$

**2.**

$$ \frac{1}{2}(3 + 4t) \leq 6\left(\frac{1}{3} - \frac{1}{2}t\right) - \frac{1}{4}(2 + 10t) $$

$$ \frac{3}{2} + 2t \leq 2 - 3t - \frac{1}{2} - \frac{5}{2}t $$

$$ \frac{3}{2} + 2t \leq -\frac{11}{2}t + \frac{3}{2} $$

$$ 2t + \frac{11}{2}t \leq 0 $$

$$ \frac{15}{2}t \leq 0 $$

$$ 15t \leq 0 \times 2 $$

$$ t \leq 0 \div 15 $$

$$ t \leq 0 $$

$$ (-\infty, 0] $$

**3.**

$$ -1 < 4x + 2 < 10 $$

$$ -3 < 4x < 8 $$

$$ -\frac{3}{4} < x < 2 $$

$$ \left(-\frac{3}{4}, 2\right) $$

**4.**

$$ 8 \leq 3 - 5z < 12 $$

$$ 5 \leq -5z < 9 $$

$$ -1 \geq z > -\frac{9}{5} $$

$$ \left(-\frac{9}{5}, -1\right] $$

**5.**

$$ 0 \leq 10w - 15 \leq 23 $$

$$ 15 \leq 10w \leq 38 $$

$$ \frac{3}{2} \leq w \leq \frac{19}{5} $$

$$ \left[\frac{3}{2}, \frac{19}{5}\right] $$

**6.**

$$ 2 < \frac{1}{6} - \frac{1}{2}x \leq 4 $$

**7.**

If $0 \leq x < 3$ determine a and b for the inequality: $a \leq 4x + 1 < b$

$$ 0 \leq 4x < 12 $$

$$ 1 \leq 4x + 1 \leq 13 $$

$$ a = 1 $$

$$ b = 13 $$

---

## Assignment Problems

For problems 1 – 10 solve each of the following inequalities. Give the solution
in both inequality and interval notations.

**1.**

$$ 7x + 2(4 - x) < 12 - 3(5 + 6x) $$

$$ 7x + 8 - 2x < 12 - 15 - 18x $$

$$ 5x + 8 < -3 - 18x $$

$$ 23x < -11 $$

$$ x < -\frac{11}{23} $$

$$ \left(-\infty, -\frac{11}{23}\right) $$

**2.**

$$ 10(3 + w) \geq 9(2 - 4w) $$

$$ 30 + 10w \geq 18 - 36w $$

$$ 46w \geq -12 $$

$$ w \geq -\frac{12}{46} $$

$$ w \geq -\frac{6}{23} $$

$$ \left[-\frac{6}{23}, \infty\right) $$

**3.**

$$ 2(4 + 5y) \leq 12y - 6(1 - 3y) $$

$$ 8 + 10y \leq 12y - 6 + 18y $$

$$ 8 + 10y \leq 30y - 6 $$

$$ 14 \leq 20y $$

$$ \frac{14}{20} \leq y $$

$$ \frac{7}{10} \leq y $$

$$ \left[\frac{7}{10},\infty\right) $$

**4.**

$$ 2\left(\frac{1}{3} - \frac{1}{6}z\right) > \frac{1}{9}z + 4\left(2 - \frac{7}{18}z\right) $$

$$ \frac{2}{3} - \frac{2}{6}z > \frac{1}{9}z + 8 - \frac{28}{18}z $$

$$ \frac{2}{3} - \frac{1}{3}z > \frac{1}{9}z + 8 - \frac{14}{9}z $$

$$ \frac{2}{3} - \frac{3}{9}z > -\frac{13}{9}z + \frac{24}{3} $$

$$ \frac{10}{9}z > \frac{22}{3} $$

$$ z > \left(\frac{22}{3}\right)\left(\frac{9}{10}\right) $$

$$ z > \left(\frac{198}{30}\right) $$

$$ z > \frac{33}{5} $$

$$ \left(\frac{33}{5},\infty\right) $$

**5.**

$$ 2 \leq 2 + 4(3 - x) \leq 6 $$

$$ 2 \leq 2 + 12 - 4x \leq 6 $$

$$ 2 \leq 14 - 4x \leq 6 $$

$$ -12 \leq -4x \leq -8 $$

$$ 3 \geq x \geq 2 $$

$$ [2, 3] $$

**6.**

$$ -4 < 7x + 8 \leq 1 $$

$$ -12 < 7x \leq -7 $$

$$ -\frac{12}{7} < x \leq -\frac{7}{7} $$

$$ -\frac{12}{7} < x \leq -1 $$

$$ \left(-\frac{12}{7}, -1\right] $$

**7.**

$$ \frac{1}{2} < 2\left(\frac{1}{4} + \frac{1}{8}t\right) < \frac{3}{4} $$

$$ \frac{1}{2} < \frac{1}{2} + \frac{1}{4}t < \frac{3}{4} $$

$$ 0 < \frac{1}{4}t < \frac{1}{4} $$

$$ 0 < t < 1 $$

$$ (0, 1) $$

**8.**

$$ -12 \leq 4 - 11m \leq 3 $$

$$ -16 \leq -11m \leq -1 $$

$$ \frac{16}{11} \geq m \geq \frac{1}{11} $$

$$ \left[\frac{1}{11}, \frac{16}{11}\right] $$

**9.**

$$ 0 \leq \frac{3}{7} - \frac{5}{14}x < \frac{1}{2} $$

$$ -\frac{3}{7} \leq -\frac{5}{14}x < \frac{1}{14} $$

$$ 6 \geq 5x > -1 $$

$$ \frac{6}{5} \geq x > -\frac{1}{5} $$

$$ \left(-\frac{1}{5}, \frac{6}{5}\right] $$

**10.**

$$ -8 < 2(3 + 4x) - 4(1 + 3x) \leq 3 $$

$$ -8 < 6 + 8x - 4 - 12x \leq 3 $$

$$ -8 < 2 - 4x \leq 4 $$

$$ -10 < -4x \leq 2 $$

$$ \frac{5}{2} > x \geq -\frac{1}{2} $$

$$ \left[-\frac{1}{2}, \frac{5}{2}\right) $$

**11.**

If $-7 < x \leq 6$ determine a and b for inequality: $a < 3x + 8 \leq b$

$$ -21 < 3x \leq 18 $$

$$ -13 < 3x + 8 \leq 26 $$

$$ a = -13 $$

$$ b = 26 $$

**12.**

If $-3 \leq x \leq -1$ determine a and b for inequality: $a \leq 6 - 2x \leq b$

$$ a < -2x + 6 \leq b $$

$$ 6 \geq -2x \geq 2 $$

$$ 6 + 6 \geq 6 - 2x \geq 2 + 6 $$

$$ 12 \geq 6 - 2x \geq 8 $$

$$ 8 \leq 6 - 2x \leq 12 $$

$$ a = 8 $$

$$ b = 12 $$
