# 2.2 Linear Equations

---

**Example 1**

**(a)**

$$ 3(x + 5) = 2(-6 - x) - 2x $$

$$ 3x + 15 = 2(-6) - 2(x) - 2x $$

$$ 3x + 15 = -12 - 2x - 2x $$

$$ 3x + 15 = -12 - 4x $$

$$ 7x = -27 $$

$$ \frac{7x}{7} = \frac{-27}{7} $$

$$ x = -\frac{27}{7} $$

$$ 3((-\frac{27}{7}) + 5) = 2(-6 - (-\frac{27}{7})) - 2(-\frac{27}{7}) $$

$$ 3(-\frac{135}{35} + \frac{175}{35}) = 2(-\frac{252}{42} + \frac{162}{42}) + \frac{54}{7} $$

$$ 3(\frac{40}{35}) = 2(-\frac{90}{42}) + \frac{54}{7} $$

$$ 3(\frac{8}{7}) = 2(-\frac{15}{7}) + \frac{54}{7} $$

$$ \frac{24}{7} = -\frac{30}{7} + \frac{54}{7} $$

$$ \frac{24}{7} = \frac{24}{7} $$

$$ x = \{-\frac{27}{7}\}$$

**(b)**

$$ \frac{m - 2}{3} + 1 = \frac{2m}{7} $$

$$ \frac{m - 2}{3} + \frac{3}{3} = \frac{2m}{7} $$

$$ \frac{m - 2 + 3}{3} = \frac{2m}{7} $$

$$ (\frac{m - 2 + 3}{3})(\frac{3}{1}) = (\frac{2m}{7})(\frac{3}{1}) $$

$$ m - 2 + 3 = \frac{6m}{7} $$

$$ (m - 2 + 3)(\frac{7}{1}) = (\frac{6m}{7})(\frac{7}{1}) $$

$$ 7m - 14 + 21 = 6m $$

$$ m - 14 + 21 = 0 $$

$$ m = 14 - 21 $$

$$ m = -7 $$

$$ \frac{(-7) - 2}{3} + 1 = \frac{2(-7)}{7} $$

$$ \frac{-7 - 2}{3} + 1 = \frac{-14}{7} $$

$$ \frac{-9}{3} + 1 = -2 $$

$$ -3 + 1 = -2 $$

$$ -2 = -2 $$

$$ m = \{-7\} $$

**(c\)**

$$ \frac{5}{2y - 6} = \frac{10 - y}{y^2 - 6y + 9} $$

$$ \frac{5}{2(y - 3)} = \frac{10 - y}{(y - 3)(y - 3)} $$

$$ LCD = 2(y - 3)^2 $$

$$ (\frac{5}{2(y - 3)})(\frac{2(y - 3)^2}{1}) = (\frac{10 - y}{(y - 3)(y - 3)})(\frac{2(y - 3)^2}{1}) $$

$$ 5(y - 3) = 2(10 - y) $$

$$ 5y - 15 = 20 - 2y $$

$$ 7y = 35 $$

$$ \frac{7y}{7} = \frac{35}{7} $$

$$ y = 5 $$

$$ \frac{5}{2(5) - 6} = \frac{10 - (5)}{(5)^2 - 6(5) + 9} $$

$$ \frac{5}{4} = \frac{5}{25 - 30 + 9} $$

$$ \frac{5}{4} = \frac{5}{4} $$

$$ y = \{5\} $$

$$  $$

**(d)**

$$ \frac{2z}{z + 3} = \frac{3}{z - 10} + 2 $$

$$ LCD = (z + 3)(z - 10) $$

$$ (z + 3)(z - 10)(\frac{2z}{z + 3}) = (\frac{3}{z - 10} + 2)(z + 3)(z - 10) $$

$$ 2z(z - 10) = 3(z + 3)+ 2(z + 3)(z - 10) $$

$$ 2z^2 - 20z = 3z + 9 + 2(z^2 - 7z - 30) $$

$$ 2z^2 - 20z = 3z + 9 + 2z^2 - 14z - 60 $$

$$ \cancel{2z^2} - 20z = 3z + 9 + \cancel{2z^2} - 14z - 60 $$

$$ -20z = -11z - 51 $$

$$ 51 = 9z $$

$$ \frac{51}{9} = z $$

$$ \frac{17}{3} = z $$

$$ \dfrac{2(\dfrac{17}{3})}{(\dfrac{17}{3}) + 3} \stackrel{?}{=} \dfrac{3}{(\dfrac{17}{3}) - 10} + 2 $$

$$ \frac{\dfrac{34}{3}}{\dfrac{26}{3}} \stackrel{?}{=} \frac{3}{-\dfrac{13}{3}} + 2 $$

$$ \frac{17}{3} = \frac{17}{3} $$

$$ z = \{\frac{17}{3}\} $$

---

**Example 2**

Solve each of the following equations.

**(a)**

$$ \frac{2}{x + 2} = \frac{-x}{x^2 + 5x + 6} $$

$$ \frac{2}{x + 2} = \frac{-x}{(x + 3)(x + 2)} $$

$$ LCD = (x + 2)(x + 3) $$

$$ (x + 2)(x + 3)(\frac{2}{x + 2}) = \frac{-x}{(x + 3)(x + 2)}(x + 3)(x + 2) $$

$$ 2(x + 3) = -x $$

$$ 2x + 6 = -x $$

$$ 3x = -6 $$

$$ x = -\frac{6}{3} $$

$$ x = -2 $$

$$ \frac{2}{(-2) + 2} = \frac{-(-2)}{(-2)^2 + 5(-2) + 6} $$

$$ \frac{2}{0} = \frac{-(-2)}{(-2)^2 + 5(-2) + 6} $$

$$ \text{NO SOLUTION SET - CANNOT DIVIDE BY ZERO} $$

$$ \emptyset $$

**(b)**

$$ \frac{2}{x + 1} = 4 - \frac{2x}{x + 1} $$

$$ LCD = (x + 1) $$

$$ (x + 1)(\frac{2}{x + 1}) = (4 - \frac{2x}{x + 1})(x + 1) $$

$$ 2 = 4(x + 1) - 2x $$

$$ 2 = 4x + 4 - 2x $$

$$ 2 = 2x + 4 $$

$$ -2 = 2x $$

$$ -1 = x $$

$$ \frac{2}{(-1) + 1} = 4 - \frac{2(-1)}{(-1) + 1} $$

$$ \frac{2}{0} = 4 - \frac{2(-1)}{0} $$

$$ \text{NO SOLUTION SET - CANNOT DIVIDE BY ZERO} $$

$$ \emptyset $$

---

## Practice Problems

Solve each of the following equations and check your answer.

**1.**

$$ 4x - 7(2 - x) = 3x + 2 $$

$$ 4x - 14 + 7x = 3x + 2 $$

$$ 11x - 14 = 3x + 2 $$

$$ 8x = 16 $$

$$ \frac{8x}{8} = \frac{16}{8} $$

$$ x = 2 $$

$$ 4(2) - 7(2 - (2)) = 3(2) + 2 $$

$$ 8 - 7(0) = 6 + 2 $$

$$ 8 = 8 $$

$$ x = \{2\} $$

**2.**

$$ 2(w + 3) - 10 = 6(32 - 3w) $$

$$ 2w + 6 - 10 = 192 - 18w $$

$$ 2w - 4 = 192 - 18w $$

$$ 20w = 192 + 4 $$

$$ 20w = 196 $$

$$ \frac{20w}{20} = \frac{196}{20} $$

$$ w = \frac{49}{5} $$

$$ 2((\frac{49}{5}) + 3) - 10 = 6(32 - 3(\frac{49}{5})) $$

$$ 2(\frac{49}{5} + \frac{15}{5}) - 10 = 6(\frac{160}{5} - \frac{147}{5}) $$

$$ 2(\frac{64}{5}) - 10 = 6(\frac{13}{5}) $$

$$ \frac{128}{5} - 10 = \frac{78}{5} $$

$$ \frac{128}{5} - \frac{50}{5} = \frac{78}{5} $$

$$ \frac{78}{5} = \frac{78}{5} $$

$$ w = \{\frac{49}{5}\} $$

**3.**

$$ \frac{4 - 2z}{3} = \frac{3}{4} - \frac{5z}{6} $$

$$ LCD = 3(4) = 12 $$

$$ (3)(4)(\frac{4 - 2z}{3}) = (\frac{3}{2(2)} - \frac{5z}{3(2)})(3)(2)(2) $$

$$ 4(4 - 2z) = 3(3) - 5z(2) $$

$$ 16 - 8z = 9 - 10z $$

$$ 2z = -7 $$

$$ z = -\frac{7}{2} $$

$$ \frac{4 - 2(-\frac{7}{2})}{3} \stackrel{?}{=} \frac{3}{4} - \frac{5(-\frac{7}{2})}{6} $$

$$ \frac{4 - (-\frac{14}{2})}{3} \stackrel{?}{=} \frac{3}{4} - \frac{(-\frac{35}{2})}{6} $$

$$ \frac{4 + 7}{3} \stackrel{?}{=} \frac{3}{4} + \frac{35}{12} $$

$$ \frac{11}{3} \stackrel{?}{=} \frac{9}{12} + \frac{35}{12} $$

$$ \frac{11}{3} \stackrel{?}{=} \frac{44}{12} $$

$$ \frac{11}{3} = \frac{11}{3} $$

$$ z = \{-\frac{7}{2}\} $$

**4.**

$$ \frac{4t}{t^2 - 25} = \frac{1}{5 - t} $$

$$ \frac{4t}{(t - 5)(t + 5)} = \frac{1}{-1(t - 5)} $$

$$ \frac{4t}{(t - 5)(t + 5)} = -\frac{1}{t - 5} $$

$$ LCD = (t - 5)(t + 5) $$

$$ (t - 5)(t + 5)(\frac{4t}{(t - 5)(t + 5)}) = (-\frac{1}{t - 5})(t - 5)(t + 5) $$

$$ 4t = -1(t + 5) $$

$$ 4t = -t - 5 $$

$$ 5t = -5 $$

$$ t = -1 $$

$$ \frac{4(-1)}{(-1)^2 - 25} \stackrel{?}{=} \frac{1}{5 - (-1)} $$

$$ \frac{-4}{1 - 25} \stackrel{?}{=} \frac{1}{5 + 1} $$

$$ \frac{-4}{-24} \stackrel{?}{=} \frac{1}{6} $$

$$ \frac{1}{6} = \frac{1}{6} $$

$$ t = \{-1\} $$

$$  $$

**5.**

$$ \frac{3y + 4}{y - 1} = 2 + \frac{7}{y - 1} $$

$$ LCD = y - 1 $$

$$ (y - 1)(\frac{3y + 4}{y - 1}) = (2 + \frac{7y}{y - 1})(y - 1) $$

$$ 3y + 4 = 2(y - 1) + 7y $$

$$ 3y + 4 = 2y - 2 + 7y $$

$$ 3y + 4 = 9y - 2 $$

$$ 6 = 6y $$

$$ 1 = y $$

$$ \frac{3(1) + 4}{(1) - 1} = 2 + \frac{7}{(1) - 1} $$

$$ \frac{3 + 4}{1 - 1} = 2 + \frac{7}{1 - 1} $$

$$ \frac{3 + 4}{0} = 2 + \frac{7}{0} $$

$$ \text{NO SOLUTION - CANNOT DIVIDE BY ZERO} $$

$$ \emptyset $$

**6.**

$$  \frac{5x}{3x - 3} + \frac{6}{x + 2} = \frac{5}{3} $$

$$  \frac{5x}{3(x - 1)} + \frac{6}{x + 2} = \frac{5}{3} $$

$$ LCD = 3(x - 1)(x + 2) $$

$$ (3)(x - 1)(x + 2)(\frac{5x}{3(x - 1)} + \frac{6}{x + 2}) = (\frac{5}{3})(3)(x - 1)(x + 2) $$

$$ 5x(x + 2) + 6(3)(x - 1) = 5(x - 1)(x + 2) $$

$$ 5x^2 + 10x + 18x - 18 = 5(x^2 + x - 2) $$

$$ 5x^2 + 28x - 18 = 5x^2 + 5x - 10 $$

$$ \cancel{5x^2} + 28x - 18 = \cancel{5x^2} + 5x - 10 $$

$$ 28x - 18 = 5x - 10 $$

$$ 23x = 8 $$

$$ x = \frac{8}{23} $$

$$  \frac{5(\frac{8}{23})}{3(\frac{8}{23}) - 3} + \frac{6}{(\frac{8}{23}) + 2} \stackrel{?}{=} \frac{5}{3} $$

$$ \frac{\frac{40}{23}}{-\frac{45}{23}} + \frac{6}{\frac{54}{23}} \stackrel{?}{=} \frac{5}{3} $$

$$ -\frac{8}{9} + \frac{23}{9} \stackrel{?}{=} \frac{5}{3} $$

$$ \frac{5}{3} = \frac{5}{3} $$

$$ x = \{\frac{8}{23}\} $$

---

## Assignment Problems

Solve each of the following equations and check your answer.

**1.**

$$ 13 + 2(1 - u) = 8u - 5(u + 7) $$

$$ 13 + 2 - 2u = 8u - 5u - 35 $$

$$ 15 - 2u = 3u - 35 $$

$$ 5u = 50 $$

$$ u = 10 $$

$$ 13 + 2(1 - (10)) \stackrel{?}{=} 8(10) - 5((10) + 7) $$

$$ 13 - 18 \stackrel{?}{=} 80 - 85 $$

$$ -5 \stackrel{?}{=} -5 $$

$$ u = \{10\} $$

**2.**

$$ 8(2 + 3z) + 1 = z - 10(z + 1) $$

$$ 16 + 24z + 1 = z - 10z - 10 $$

$$ 24z + 17 = -9z - 10 $$

$$ 33z = -27 $$

$$ z = -\frac{27}{33} $$

$$ z = -\frac{9}{11} $$

$$ 8(2 + 3(-\frac{9}{11})) + 1 \stackrel{?}{=} (-\frac{9}{11}) - 10((-\frac{9}{11}) + 1) $$

$$ 8(-\frac{5}{11}) + 1 \stackrel{?}{=} -\frac{9}{11} - 10(\frac{2}{11}) $$

$$ -\frac{40}{11} + 1 \stackrel{?}{=} -\frac{9}{11} - \frac{20}{11} $$

$$ -\frac{29}{11} \stackrel{?}{=} -\frac{29}{11} $$

$$ z = \{-\frac{9}{11}\} $$

**3.**

$$ 8 - (4 - 12t) + 2 = 3t + 2(7 - 3t) $$

$$ 8 - 4 + 12t + 2 = 3t + 14 - 6t $$

$$ 6 + 12t = -3t + 14 $$

$$ 15t = 8 $$

$$ t = \frac{8}{15} $$

$$ 8 - (4 - 12(\frac{8}{15})) + 2 \stackrel{?}{=} 3(\frac{8}{15}) + 2(7 - 3(\frac{8}{15})) $$

$$ 8 - (4 - \frac{96}{15}) + 2 \stackrel{?}{=} \frac{24}{15} + 2(7 - \frac{24}{15}) $$

$$ 8 - (-\frac{12}{5}) + 2 \stackrel{?}{=} \frac{8}{5} + 2(\frac{27}{5}) $$

$$ 10 + \frac{12}{5} \stackrel{?}{=} \frac{8}{5} + \frac{54}{5} $$

$$ \frac{50}{5} + \frac{12}{5} \stackrel{?}{=} \frac{8}{5} + \frac{54}{5} $$

$$ \frac{62}{5} = \frac{62}{5} $$

$$ t = \{\frac{8}{15}\} $$

**4.**

$$ 2x(6x - 1) + 21 = 8x - x(3 - 12x) $$

$$ 12x^2 - 2x + 21 = 8x - 3x + 12x^2 $$

$$ \cancel{12x^2} - 2x + 21 = 8x - 3x + \cancel{12x^2} $$

$$ -2x + 21 = 8x - 3x $$

$$ -2x + 21 = 5x $$

$$ 21 = 7x $$

$$ 3 = x $$

$$ 2(3)(6(3) - 1) + 21 \stackrel{?}{=} 8(3) - (3)(3 - 12(3)) $$

$$ 6(18 - 1) + 21 \stackrel{?}{=} 24 - (3)(3 - 36) $$

a$ 108 - 6 + 21 \stackrel{?}{=} 24 + 99 $$

$$ 108 - 6 + 21 \stackrel{?}{=} 24 + 99 $$

$$ 123 = 123 $$

$$ x = \{3\}$$

**5.**

$$ \frac{3w - 1}{5} + 2 = \frac{7w + 2}{15} $$

$$ LCD = (5)(3) = 15 $$

$$ (3)(5)(\frac{3w - 1}{5} + 2) = (\frac{7w + 2}{(5)(3)})(3)(5) $$

$$ (3)(3w - 1) + 2(5)(3) = 7w + 2 $$

$$ 9w - 3 + 30 = 7w + 2 $$

$$ 9w + 27 = 7w + 2 $$

$$ 2w = -25 $$

$$ w = -\frac{25}{2} $$

$$ \frac{3(-\frac{25}{2}) - 1}{5} + 2 \stackrel{?}{=} \frac{7(-\frac{25}{2}) + 2}{15} $$

$$ \frac{-\frac{77}{2}}{5} + 2 \stackrel{?}{=} \frac{-\frac{171}{2}}{15} $$

$$ -\frac{77}{10}+ 2 \stackrel{?}{=} -\frac{171}{30} $$

$$ -\frac{57}{10} = -\frac{57}{10} $$

$$ w = \{-\frac{25}{2}\} $$

**6.**

$$ \frac{10y}{9} + \frac{1}{3} = \frac{2y - 1}{9} $$

$$ LCD = (3)(3) = 9 $$

$$ (3)(3)(\frac{10y}{(3)(3)} + \frac{1}{3}) = (\frac{2y - 1}{(3)(3)})(3)(3) $$

$$ 10y + (1)(3) = 2y - 1 $$

$$ 10y + 3 = 2y - 1 $$

$$ 8y = -4 $$

$$ y = -\frac{1}{2} $$

$$ \frac{10(-\frac{1}{2})}{9} + \frac{1}{3} \stackrel{?}{=} \frac{2(-\frac{1}{2}) - 1}{9} $$

$$ \frac{-5}{9} + \frac{1}{3} \stackrel{?}{=} \frac{-1 - 1}{9} $$

$$ \frac{-5}{9} + \frac{3}{9} \stackrel{?}{=} \frac{-2}{9} $$

$$ \frac{-2}{9} = \frac{-2}{9} $$

$$ y = \{-\frac{1}{2}\} $$

**7.**

$$ 2(3 - \frac{x}{4}) = \frac{2x + 5}{3} - \frac{1}{3} $$

$$ \frac{6}{1} - \frac{x}{2} = \frac{2x + 5}{3} - \frac{1}{3} $$

$$ LCD = 3(2) = 6 $$

$$ (3)(2)(\frac{6}{1} - \frac{x}{2}) = (\frac{2x + 5}{3} - \frac{1}{3})(3)(2) $$

$$ 6(2)(3) - 3x = 2(2x + 5) - 2 $$

$$ 36 - 3x = 4x + 8 $$

$$ 28 = 7x $$

$$ 4 = x $$

$$ 2(3 - \frac{(4)}{4}) \stackrel{?}{=} \frac{2(4) + 5}{3} - \frac{1}{3} $$

$$ 2(3 - 1) \stackrel{?}{=} \frac{8 + 5}{3} - \frac{1}{3} $$

$$ 6 - 2 \stackrel{?}{=} \frac{8 + 5 - 1}{3} $$

$$ 4 \stackrel{?}{=} \frac{12}{3} $$

$$ 4 = 4 $$

$$ x = \{4\} $$

**8.**

$$ \frac{6x + 24}{x + 4} = 5 $$

$$ (x + 4)(\frac{6x + 24}{x + 4}) = (5)(x + 4) $$

$$ 6x + 24 = 5x + 20 $$

$$ x = -4 $$

$$ \frac{6(-4) + 24}{(-4) + 4} \stackrel{?}{=} 5 $$

$$ \frac{-24 + 24}{-4 + 4} \stackrel{?}{=} 5 $$

$$ \frac{0}{0} \stackrel{?}{=} 5 $$

$$ \text{EMPTY SOLUTION SET - CANNOT DIVIDE BY ZERO} $$

$$ \emptyset $$

**9.**

$$ \frac{3}{v + 7} - \frac{2 - 7v}{v^2 + 5v - 14} = \frac{4}{v - 2} $$

$$ \frac{3}{v + 7} - \frac{2 - 7v}{(v + 7)(v - 2)} = \frac{4}{v - 2} $$

$$ LCD = (v + 7)(v - 2) $$

$$ (v + 7)(v - 2)(\frac{3}{v + 7} - \frac{2 - 7v}{(v + 7)(v - 2)}) = (\frac{4}{v - 2})(v + 7)(v - 2) $$

$$ 3(v - 2) - (2 - 7v) = 4(v + 7) $$

$$ 3v - 6 - 2 + 7v = 4v + 28 $$

$$ 10v - 8 = 4v + 28 $$

$$ 6v = 36 $$

$$ v = 6 $$

$$ \frac{3}{(6) + 7} - \frac{2 - 7(6)}{(6)^2 + 5(6) - 14} \stackrel{?}{=} \frac{4}{(6) - 2} $$

$$ \frac{3}{6 + 7} - \frac{2 - 42}{36 + 30 - 14} \stackrel{?}{=} \frac{4}{6 - 2} $$

$$ \frac{3}{13} - \frac{-40}{52} \stackrel{?}{=} \frac{4}{4} $$

$$ 1 = 1 $$

$$ v = \{6\} $$

**10.**

$$ \frac{6t - 1}{t^2 + 5t + 4} = -\frac{19}{t + 1} $$

$$ \frac{6t - 1}{(t + 4)(t + 1)} = -\frac{19}{t + 1} $$

$$ LCD = (t + 4)(t + 1) $$

$$ (t + 4)(t + 1)(\frac{6t - 1}{(t + 4)(t + 1)}) = (-\frac{19}{t + 1})(t + 4)(t + 1) $$

$$ 6t - 1 = (-19)(t + 4) $$

$$ 6t - 1 = -19t - 76 $$

$$ 25t = -75 $$

$$ t = -3 $$

$$ \frac{6(-3) - 1}{(-3)^2 + 5(-3) + 4} \stackrel{?}{=} -\frac{19}{(-3) + 1} $$

$$ \frac{-18 - 1}{9 - 15 + 4} \stackrel{?}{=} -\frac{19}{-2} $$

$$ \frac{-19}{-2} = -\frac{19}{-2} $$

$$ \frac{19}{2} = \frac{19}{2} $$

$$ t = \{-3\} $$

**11.**

$$ \frac{8 - 4z}{3z - 2} = 2 - \frac{10z}{3z - 2} $$

$$ LCD = 3z - 2 $$

$$ (3z - 2)(\frac{8 - 4z}{3z - 2}) = (2 - \frac{10z}{3z - 2})(3z - 2) $$

$$ 8 - 4z = 2(3z - 2) - 10z $$

$$ 8 - 4z = 6z - 4 - 10z $$

$$ 8 - 4z = -4z - 4 $$

$$ 8 \neq -4 $$

$$ \text{NO REAL SOLUTION} $$

$$ \emptyset $$

**12.**

$$ \frac{4w - 1}{w - 2} + \frac{8w}{w^2 - 6w + 8} = \frac{4w + 3}{w - 4} $$

$$ \frac{4w - 1}{w - 2} + \frac{8w}{(w - 4)(w - 2)} = \frac{4w + 3}{w - 4} $$

$$ LCD = (w - 4)(w - 2) $$

$$ (w - 4)(w - 2)(\frac{4w - 1}{w - 2} + \frac{8w}{(w - 4)(w - 2)}) = (\frac{4w + 3}{w - 4})(w - 4)(w - 2) $$

$$ (4w - 1)(w - 4) + 8w = (4w + 3)(w - 2) $$

$$ (4w)(w) + (-1)(w) +(4w)(-4) + (-1)(-4) + 8w = (4w)(w) + (3)(w) +(4w)(-2) + (3)(-2) $$

$$ 4w^2 - w - 16w + 4 + 8w = 4w^2 + 3w - 8w - 6 $$

$$ \cancel{4w^2} - w - 16w + 4 + 8w = \cancel{4w^2} + 3w - 8w - 6 $$

$$ -w - 16w + 4 + 8w = 3w - 8w - 6 $$

$$ -9w + 4 = -5w - 6 $$

$$ 10 = 4w $$

$$ \frac{10}{4} = w $$

$$ \frac{5}{2} = w $$

$$ \frac{4(\frac{5}{2}) - 1}{(\frac{5}{2}) - 2} + \frac{8(\frac{5}{2})}{(\frac{5}{2})^2 - 6(\frac{5}{2}) + 8} \stackrel{?}{=} \frac{4(\frac{5}{2}) + 3}{(\frac{5}{2}) - 4} $$

$$ \frac{\frac{20}{2} - 1}{\frac{5}{2} - 2} + \frac{\frac{40}{2}}{\frac{25}{4} - \frac{30}{2} + 8} \stackrel{?}{=} \frac{\frac{20}{2} + 3}{\frac{5}{2} - 4} $$

$$ \frac{9}{\frac{1}{2}} + \frac{20}{-\frac{3}{4}} \stackrel{?}{=} \frac{13}{-\frac{3}{2}} $$

$$ 18 - \frac{80}{3} \stackrel{?}{=} -\frac{26}{3} $$

$$ -\frac{26}{3} = -\frac{26}{3} $$

$$ w = \{\frac{5}{2}\} $$
