# 2.4 Equations With More Than One Variable

---

**Example 1**

Solve $A = P(1 + rt)$ for $r$.

$$ A = P(1 + rt) $$

$$ A = P + Prt $$

$$ A - P = Prt $$

$$ \frac{A - P}{Pt} = r \Rightarrow r = \frac{A - P}{Pt} $$

---

**Example 2**

Solve $V = m\left(\dfrac{1}{b} - \dfrac{5aR}{m}\right)$ for $R$.

$$ V = m\left(\dfrac{1}{b} - \frac{5aR}{m} \right) $$

$$ V = \frac{m}{b} - 5aR $$

$$ (V)(b) = (\frac{m}{b})(b) - (5aR)(b) $$

$$ Vb = m - 5abR $$

$$ Vb - m = -5abR $$

$$ \frac{Vb - m}{-5ab} = R $$

$$ \frac{(-1)(Vb - m)}{(-1)-5ab} = R $$

$$ \frac{-Vb + m}{5ab} = R $$

$$ \frac{m - Vb}{5ab} = R $$

$$ R = \frac{m - Vb}{5ab} $$

---

**Example 3**

Solve $V = m\left(\dfrac{1}{b} - \dfrac{5aR}{m}\right)$ for $b$.

$$ V = m\left(\dfrac{1}{b} - \dfrac{5aR}{m}\right) $$

$$ V = \frac{m}{b} - 5aR $$

$$ V + 5aR = \frac{m}{b} $$

$$ b(V + 5aR) = m $$

$$ b = \frac{m}{V + 5aR} $$

---

**Example 4.**

Solve $\dfrac{1}{a} = \dfrac{1}{b} + \dfrac{1}{c}$ for $c$.

$$ \dfrac{1}{a} = \dfrac{1}{b} + \dfrac{1}{c} $$

$$ LCD = abc $$

$$ (abc)(\dfrac{1}{a}) = (\dfrac{1}{b})(abc) + (\dfrac{1}{c})(abc) $$

$$ bc = ac + ab $$

$$ bc - ac = ab $$

$$ c(b - a) = ab $$

$$ c = \frac{ab}{b - a} $$

---

**Example 5**

Solve $y = \dfrac{4}{5x - 9}$ for $x$.

$$ y = \frac{4}{5x - 9} $$

$$ y(5x - 9) = 4 $$

$$ 5xy - 9y = 4 $$

$$ 5xy = 9y + 4 $$

$$ x = \frac{9y + 4}{5y} $$

---

**Example 6**

Solve $y = \dfrac{4 - 3x}{1 + 8x}$ for $x$.

$$ y = \frac{4 - 3x}{1 + 8x} $$

$$ y(1 + 8x) = 4 - 3x $$

$$ y + 8xy = 4 - 3x $$

$$ 8xy + 3x = 4 - y $$

$$ x(8y + 3) = 4 - y $$

$$ x = \frac{4 - y}{8y + 3} $$

---

## Practice Problems

**1.**

Solve $E = 3v\left(4 - \dfrac{2}{r}\right)$ for $r$.

$$ E = 3v\left(4 - \frac{2}{r}\right) $$

$$ E = 12v - \frac{6v}{r} $$

$$ Er = 12vr - 6v $$

$$ Er - 12vr = -6v $$

$$ r(E - 12v) = -6v $$

$$ r = \frac{-6v}{E - 12v} $$

$$  $$

**2.**

Solve $Q = \dfrac{6h}{7s} + 4(1 - h)$ for $s$.

$$ Q = \dfrac{6h}{7s} + 4(1 - h) $$

$$ 7sQ = 6h + 28s(1 - h) $$

$$ 7sQ - 28s(1 - h) = 6h $$

$$ s(7Q - 28(1 - h)) = 6h $$

$$ s = \frac{6h}{7Q - 28(1 - h)} $$

**3.**

Solve $Q = \dfrac{6h}{7s} + 4(1 - h)$ for $h$.

$$ Q = \dfrac{6h}{7s} + 4(1 - h) $$

$$ 7sQ = 6h + 28s(1 - h) $$

$$ 7sQ = 6h + 28s - 28sh $$

$$ 7sQ - 28s = 6h -28sh $$

$$ 7sQ - 28s = h(6 - 28s) $$

$$ \frac{7sQ - 28s}{6 - 28s} = h $$

$$ h = \frac{7sQ - 28s}{6 - 28s} $$

**4.**

Solve $A - \dfrac{1 - 2t}{4p} = \dfrac{4 + 3t}{5p}$ for $t$.

$$ A - \frac{1 - 2t}{4p} = \frac{4 + 3t}{5p} $$

$$ LCD = (5)(4)p = 20p $$

$$ (5)(4p)\left(A - \frac{1 - 2t}{4p}\right) = (5p)(4)\left(\frac{4 + 3t}{5p}\right) $$

$$ 20Ap - 5(1 - 2t) = 4(4 + 3t)$$

$$ 20Ap - 5 + 10t = 16 + 12t $$

$$ 20Ap - 5 - 16 = -10t + 12t $$

$$ 20Ap - 21 = 2t $$

$$ \frac{20Ap - 21}{2} = t $$

$$ t = \frac{20Ap - 21}{2} $$

**5.**

Solve $y = \dfrac{10}{3 - 7x}$ for $x$.

$$ y = \frac{10}{3 - 7x} $$

$$ y(3 - 7x) = 10 $$

$$ 3y - 7xy = 10 $$

$$ -7xy = 10 - 3y $$

$$ x = \frac{10 - 3y}{-7y} $$

$$ x = \left(\frac{10 - 3y}{-7y}\right)\left(\frac{-1}{-1}\right) $$

$$ x = \frac{3y - 10}{7y} $$

**6.**

Solve $y = \dfrac{3 + x}{12 - 9x}$ for $x$.

$$ y = \frac{3 + x}{12 - 9x} $$

$$ y(12 - 9x) = 3 + x $$

$$ y(12 - 9x) - 3 = x $$

$$ 12y - 9xy - 3 = x  $$

$$ 12y - 3 = x + 9xy $$

$$ 12y - 3 = x(1 + 9y) $$

$$ \frac{12y - 3}{1 + 9y} = x $$

$$ x = \frac{12y - 3}{1 + 9y} $$

---

## Assignment Problems

**1.**

Solve $A = 3p(4 - 2r)$ for $p$.

$$ A = 3p(4 - 2r) $$

$$ A = 12p - 6rp $$

$$ A = p(12 - 6r) $$

$$ \frac{A}{12 - 6r} = p $$

$$ p = \frac{A}{12 - 6r} $$

**2.**

Solve $A = 3p(4 - 2r)$ for $r$.

$$ A = 3p(4 - 2r) $$

$$ A = 12p - 6rp $$

$$ A - 12p - -6rp $$

$$ \frac{A - 12p}{-6p} = r $$

$$ \left(\frac{-1}{-1}\right)\left(\frac{A - 12p}{-6p}\right) = r $$

$$ \frac{12p - A}{6p} = r $$

$$ r = \frac{12p - A}{6p} $$

**3.**

Solve $T = \dfrac{c}{3}\left(6p + \dfrac{3q}{c}\right) - 7p$ for $p$.

$$ T = \frac{c}{3}\left(6p + \frac{3q}{c}\right) - 7p $$

$$ (3)(T) = \left(\frac{c}{3}\left(6p + \frac{3q}{c}\right) - 7p\right)(3) $$

$$ 3T = c\left(6p + \frac{3q}{c}\right) - 21p$$

$$ 3T = 6pc + 3q - 21p $$

$$ 3T - 3q = 6pc - 21p $$

$$ 3T - 3q = p(6c - 21) $$

$$ \frac{3T - 3q}{6c - 21} = p $$

$$ \frac{T - q}{2c - 7} = p $$

$$ p = \frac{T - q}{2c - 7} $$

**4.**

Solve $T = \dfrac{c}{3}\left(6p + \dfrac{3q}{c}\right) - 7p$ for $c$.

$$ T = \frac{c}{3}\left(6p + \frac{3q}{c}\right) - 7p $$

$$ (3)(T) = \left(\frac{c}{3}\left(6p + \frac{3q}{c}\right) - 7p\right)(3) $$

$$ 3T = c\left(6p + \frac{3q}{c}\right) - 21p$$

$$ 3T = 6pc + 3q - 21p $$

$$ 3T - 3q + 21p = 6pc $$

$$ \frac{3T - 3q + 21p}{6p} = c $$

$$ \frac{T - q + 7p}{2p} = c $$

$$ c = \frac{T - q + 7p}{2p} $$

**5.**

Solve $\dfrac{1}{n} = \dfrac{2}{m} - \dfrac{3}{q}$ for $n$.

$$ \frac{1}{n} = \frac{2}{m} - \frac{3}{q} $$

$$ LCD = nmq $$

$$ (nmq)\left(\frac{1}{n}\right) = \left(\frac{2}{m} - \frac{3}{q}\right)(nmq) $$

$$ mq = 2nq - 3mn $$

$$ mq = n(2q - 3m) $$

$$ \frac{mq}{2q - 3m} = n $$

$$ n = \frac{mq}{2q - 3m} $$

**6.**

Solve $\dfrac{1}{n} = \dfrac{2}{m} - \dfrac{3}{q}$ for $q$.

$$ \frac{1}{n} = \frac{2}{m} - \frac{3}{q} $$

$$ LCD = nmq $$

$$ (nmq)\left(\frac{1}{n}\right) = \left(\frac{2}{m} - \frac{3}{q}\right)(nmq) $$

$$ mq = 2nq - 3mn $$

$$ mq - 2nq = -3mn $$

$$ q(m - 2n) = -3m $$

$$ q = \frac{-3m}{m - 2n} $$

$$ q = \left(\frac{-3m}{m - 2n}\right)\left(\frac{-1}{-1}\right) $$

$$ q = \frac{3m}{2n - m} $$

**7.**

Solve $3A + 6C = 4A(B - 7C)$ for $C$.

$$ 3A + 6C = 4A(B - 7C) $$

$$ 3A + 6C = 4AB - 28AC $$

$$ 3A - 4AB = -6C - 28AC $$

$$ 3A - 4AB = C(-6 - 28A) $$

$$ \frac{3A - 4AB}{-6 - 28A} = C $$

$$ \left(\frac{-1}{-1}\right)\left(\frac{3A - 4AB}{-6 - 28A}\right) = C $$

$$ \frac{4AB - 3A}{28A + 6} = C $$

$$ C = \frac{4AB - 3A}{28A + 6} $$

**8.**

Solve $3A + 6C = 4A(B - 7C)$ for $A$.

$$ 3A + 6C = 4A(B - 7C) $$

$$ 3A + 6C = 4AB - 28AC $$

$$ 6C = 4AB - 28AC - 3A $$

$$ 6C = A(4B - 28C -3) $$

$$ \frac{6C}{4B - 28C - 3} = A $$

$$ A = \frac{6C}{4B - 28C - 3} $$

**9.**

Solve $y = \dfrac{4 - 9x}{3}$ for $x$.

$$ y = \frac{4 - 9x}{3} $$

$$ 3y = 4 - 9x $$

$$ 3y - 4 = -9x $$

$$ \frac{3y - 4}{-9} = x $$

$$ \left(\frac{-1}{-1}\right)\left(\frac{3y - 4}{-9}\right) = x $$

$$ \frac{4 - 3y}{9} = x $$

$$ x = \frac{4 - 3y}{9} $$

**10.**

Solve $y = \dfrac{12}{1 - x}$ for $x$.

$$ y = \frac{12}{1 - x} $$

$$ y(1 - x) = 12 $$

$$ y - xy = 12 $$

$$ -xy = 12 - y $$

$$ xy = y - 12 $$

$$ x = \frac{y - 12}{y} $$

**11.**

Solve $y = \dfrac{7}{10x + 9}$ for $x$.

$$ y = \frac{7}{10x + 9} $$

$$ y(10x + 9) = 7 $$

$$ 10xy + 9y = 7 $$

$$ 10xy = 7 - 9y $$

$$ x = \frac{7 - 9y}{10y} $$

**12.**

Solve $y = \dfrac{8 - 5x}{9 - 7x}$ for $x$.

$$ y = \frac{8 - 5x}{9 - 7x} $$

$$ y(9 - 7x) = 8 - 5x $$

$$ 9y - 7xy = 8 - 5x $$

$$ 9y - 8 = 7xy - 5x $$

$$ 9y - 8 = x(7y - 5) $$

$$ \frac{9y - 8}{7y - 5} = x $$

$$ x = \frac{9y - 8}{7y - 5} $$

**13.**

Solve $y = \dfrac{2 + 11x}{1 + 4x}$ for $x$.

$$ y = \frac{2 + 11x}{1 + 4x} $$

$$ y(1 + 4x) = 2 + 11x $$

$$ y + 4xy = 2 + 11x $$

$$ y - 2 = 11x - 4xy $$

$$ y - 2 = x(11 - 4y) $$

$$ \frac{y - 2}{11 - 4y} = x $$

$$ x = \frac{y - 2}{11 - 4y} $$

**14.**

Solve $y = \dfrac{9 + 2x}{4 - x}$ for $x$.

$$ y = \frac{9 + 2x}{4 - x} $$

$$ y(4 - x) = 9  + 2x $$

$$ 4y - xy = 9 + 2x $$

$$ 4y - 9 = xy + 2x $$

$$ 4y - 9 = x(y + 2) $$

$$ \frac{4y - 9}{y + 2} = x $$

$$ x = \frac{4y - 9}{y + 2} $$
