# 2.5 Quadratic Equations - Part I

---

**Standard Form**

$$ ax^2 + bx + c = 0 \text{ } a \neq 0 $$

---

**Solving by Factoring**

_zero factor property_:

$$ \text{If } ab = 0 \text{ then either } a = 0 \text{ and/or } b = 0 $$

---

**Example 1**

Solve each of the following equations by factoring.

**(a)**

$$ x^2 - x = 12 $$

$$ x^2 - x - 12 = 0 $$

$$ (x - 4)(x + 3) = 0 $$

$$ x = 4 $$

$$ (4)^2 - (4) = 12 $$

$$ 16 - 4 = 12 $$

$$ 12 = 12 $$

$$ x = -3 $$

$$ (-3)^2 - (-3) = 12 $$

$$ 9 + 3 = 12 $$

$$ 12 = 12 $$

$$ x = \{4, -3\} $$

**(b)**

$$ x^2 + 40 = -14x $$

$$ x^2 + 14x + 40 = 0 $$

$$ (x + 4)(x + 10) = 0 $$

$$ x = -4 $$

$$ (-4)^2 + 40 = -14(-4) $$

$$ 16 + 40 = 56 $$

$$ 56 = 56 $$

$$ x = -10 $$

$$ (-10)^2 + 40 = -14(-10) $$

$$ 100 + 40 = 140 $$

$$ 140 = 140 $$

$$ x = \{-4, -10\} $$

**(c\)**

$$ y^2 + 12y + 36 = 0 $$

$$ (y + 6)(y + 6) = 0 $$

$$ y = -6 $$

$$ (-6)^2 + 12(-6) + 36 = 0 $$

$$ 36 - 72 + 36 = 0 $$

$$ 72 - 72 = 0 $$

$$ 0 = 0 $$

$$ y = \{-6\} $$

**(d)**

$$ 4m^2 - 1 = 0 $$

$$ (2m + 1)(2m - 1) = 0 $$

$$ 2m + 1 = 0 $$

$$ 2m = -1 $$

$$ m = -\frac{1}{2} $$

$$ 4(-\frac{1}{2})^2 - 1 = 0 $$

$$ 4(\frac{1}{4}) - 1 = 0 $$

$$ 1 - 1 = 0 $$

$$ 0 = 0 $$

$$ 2m - 1 = 0 $$

$$ 2m = 1 $$

$$ m = \frac{1}{2} $$

$$ 4(\frac{1}{2})^2 - 1 = 0 $$

$$ 4(\frac{1}{4}) - 1 = 0 $$

$$ 1 - 1 = 0 $$

$$ 0 = 0 $$

$$ m = \left\{-\frac{1}{2}, \frac{1}{2}\right\} $$

**(e)**

$$ 3x^2 = 2x + 8 $$

$$ 3x^2 - 2x - 8 = 0 $$

$$ (3x + 4)(x - 2) = 0 $$

$$ 3x + 4 = 0 $$

$$ 3x = -4 $$

$$ x = -\frac{4}{3} $$

$$ 3\left(-\frac{4}{3}\right)^2 = 2\left(-\frac{4}{3}\right) + 8 $$

$$ 3\left(\frac{16}{9}\right) = -\frac{8}{3} + 8 $$

$$ \frac{16}{3} = \frac{16}{3} $$

$$ x - 2 = 0 $$

$$ x = 2 $$

$$ 3(2)^2 = 2(2) + 8 $$

$$ 3(4) = 4 + 8 $$

$$ 12 = 12 $$

$$ x = \left\{-\frac{4}{3}, 2\right\} $$

**(f)**

$$ 10z^2 + 19z + 6 = 0 $$

$$ (5z + 2)(2z + 3) = 0 $$

$$ 5z + 2 = 0 $$

$$ 5z = -2 $$

$$ z = -\frac{2}{5} $$

$$ 10\left(-\frac{2}{5}\right)^2 + 19\left(-\frac{2}{5}\right) + 6 = 0 $$

$$ 10\left(\frac{4}{25}\right) - \frac{38}{5} + 6 = 0 $$

$$ \frac{8}{5} - \frac{38}{5} + \frac{30}{5} = 0 $$

$$ -\frac{30}{5} + \frac{30}{5} = 0 $$

$$ 0 = 0 $$

$$ 2z + 3 = 0 $$

$$ 2z = -3 $$

$$ z = -\frac{3}{2} $$

$$ 10\left(-\frac{3}{2}\right)^2 + 19\left(-\frac{3}{2}\right) + 6 = 0 $$

$$ 10\left(\frac{9}{4}\right) - \frac{57}{2} + 6 = 0 $$

$$ \frac{45}{2} - \frac{57}{2} + \frac{12}{2} = 0 $$

$$ -\frac{12}{2} + \frac{12}{2} = 0 $$

$$ 0 = 0 $$

$$ z = \left\{-\frac{2}{5}, -\frac{3}{2}\right\} $$

**(g)**

$$ 5x^2 = 2x $$

$$ 5x^2 - 2x = 0 $$

$$ x(5x - 2) = 0 $$

$$ x = 0 $$

$$ 5(0)^2 = 2(0) $$

$$ 5(0) = 2(0) $$

$$ 0 = 0 $$

$$ 5x - 2 = 0 $$

$$ 5x = 2 $$

$$ x = \frac{2}{5} $$

$$ 5\left(\frac{2}{5}\right)^2 = 2\left(\frac{2}{5}\right) $$

$$ 5\left(\frac{4}{25}\right) = \frac{4}{5} $$

$$ \frac{4}{5} = \frac{4}{5} $$

$$ x = \left\{0, \frac{2}{5}\right\} $$

---

**Example 2**

Solve each of the following equations.

**(a)**

$$ \frac{1}{x + 1} = 1 - \frac{5}{2x - 4} $$

$$ LCD = (x + 1)(2x - 4) $$

$$ (x + 1)(2x - 4)\left(\frac{1}{x + 1}\right) = \left(1 - \frac{5}{2x - 4}\right)(x + 1)(2x - 4) $$

$$ 2x - 4 = (x + 1)(2x - 4) - 5(x + 1) $$

$$ 2x - 4 = 2x^2 + 2x - 4x - 4 - 5x - 5 $$

$$ 0 = 2x^2 - 9x - 5 $$

$$ 0 = (2x + 1)(x - 5) $$

$$ 2x + 1 = 0 $$

$$ 2x = -1 $$

$$ x = -\frac{1}{2} $$

$$ \frac{1}{\left(-\dfrac{1}{2}\right) + 1} = 1 - \frac{5}{2\left(-\dfrac{1}{2}\right) - 4} $$

$$ \frac{1}{\dfrac{1}{2}} = 1 - \frac{5}{-1 - 4} $$

$$ 2 = 1 - \frac{5}{-5} $$

$$ 2 = 1 - (-1) $$

$$ 2 = 1 + 1 $$

$$ 2 = 2 $$

$$ x - 5 = 0 $$

$$ x = 5 $$

$$ \frac{1}{(5) + 1} = 1 - \frac{5}{2(5) - 4} $$

$$ \frac{1}{6} = 1 - \frac{5}{10 - 4} $$

$$ \frac{1}{6} = \frac{6}{6} - \frac{5}{6} $$

$$ \frac{1}{6} = \frac{1}{6} $$

$$ x = \left\{-\frac{1}{2}, \frac{1}{6}\right\} $$

**(b)**

$$ x + 3 + \frac{3}{x - 1} = \frac{4 - x}{x - 1} $$

$$ x + 3 = \frac{4 - x}{x - 1} - \frac{3}{x - 1} $$

$$ x + 3 = \frac{4 - x - 3}{x - 1} $$

$$ (x - 1)(x + 3) = \left(\frac{4 - x - 3}{x - 1}\right)(x - 1) $$

$$ x^2 - x + 3x - 3 = 1 - x  $$

$$ x^2 + 3x - 3 = 1 $$

$$ x^2 + 3x - 4 = 0 $$

$$ (x + 4)(x - 1) = 0 $$

$$ x + 4 = 0 $$

$$ x = -4 $$

$$ (-4) + 3 + \frac{3}{(-4) - 1} = \frac{4 - (-4)}{(-4) - 1} $$

$$ -1 + \frac{3}{-5} = \frac{8}{-5} $$

$$ -\frac{8}{5} = -\frac{8}{5} $$

$$ x - 1 = 0 $$

$$ x = 1 $$

$$ (1) + 3 + \frac{3}{(1) - 1} = \frac{4 - (1)}{(1) - 1} $$

$$ 4 + \frac{3}{0} = \frac{3}{0} $$

$$ \text{NO DIVISION BY ZERO} $$

$$ x = \{-4\} $$

---

**Example 3**

Solve $5x^3 - 5x^2 - 10x = 0$

$$ 5x^3 - 5x^2 - 10x = 0 $$

$$ x(5x^2 - 5x - 10) = 0 $$

$$ x(5x + 5)(x - 2)= 0 $$

$$ x = 0 $$

$$ 5(0)^3 - 5(0)^2 - 10(0) = 0 $$

$$ 5(0) - 5(0) - 0 = 0 $$

$$ 0 - 0 - 0 = 0 $$

$$ 0 = 0 $$

$$ 5x + 5 = 0 $$

$$ 5x = -5 $$

$$ x = -1 $$

$$ 5(-1)^3 - 5(-1)^2 - 10(-1) = 0 $$

$$ 5(-1) - 5(1) + 10 = 0 $$

$$ -5 - 5 + 10 = 0 $$

$$ -10 + 10 = 0 $$

$$ 0 = 0 $$

$$ x - 2 = 0 $$

$$ x = 2 $$

$$ 5(2)^3 - 5(2)^2 - 10(2) = 0 $$

$$ 5(8) - 5(4) - 20 = 0 $$

$$ 40 - 20 - 20 = 0 $$

$$ 20 - 20 = 0 $$

$$ 0 = 0 $$

$$ x = \{0, -1, 2\} $$

---

_square root property_:

$$ \text{If } p^2 = d \text{ then } p = \pm\sqrt{d} $$

---

**Example 4**

**(a)**

$$ x^2 - 100 = 0 $$

$$ x^2 = 100 $$

$$ x = \pm\sqrt{100} $$

$$ x = \pm 10 $$

**(b)**

$$ 25y^2 - 3 = 0 $$

$$ 25y^2 = 3 $$

$$ y^2 = \frac{3}{25} $$

$$ y = \pm \sqrt{\frac{3}{25}} $$

$$ y = \pm \frac{\sqrt{3}}{5} $$

**(c\)**

$$ 4z^2 + 49 = 0 $$

$$ 4z^2 = -49 $$

$$ z^2 = \frac{-49}{4} $$

$$ z = \pm \sqrt{\frac{-49}{4}} $$

$$ z = \pm \sqrt{\frac{49(-1)}{4}} $$

$$ z = \pm \sqrt{\frac{49}{4}}i $$

$$ z = \pm \frac{7}{2}i $$

**(d)**

$$ (2t - 9)^2 = 5 $$

$$ 2t - 9 = \pm \sqrt{5} $$

$$ 2t = 9 \pm \sqrt{5} $$

$$ t = \frac{9 \pm \sqrt{5}}{2} $$

$$ t = \frac{9}{2} \pm \frac{\sqrt{5}}{2} $$

**(e)**

$$ (3x + 10)^2 + 81 = 0 $$

$$ (3x + 10)^2 = -81 $$

$$ 3x + 10 = \pm \sqrt{-81} $$

$$ 3x + 10 = \pm \sqrt{-1(81)} $$

$$ 3x + 10 = \pm \sqrt{81}i $$

$$ 3x + 10 = \pm 9i $$

$$ 3x = -10 \pm 9i $$

$$ x = \frac{-10 \pm 9i}{3} $$

$$ x = \frac{-10}{3} \pm \frac{9i}{3} $$

$$ x = -\frac{10}{3} \pm 3i $$

---

## Practice Problems

---

For problems 1 - 7 solve the quadratic equation by factoring.

**1.**

$$ u^2 - 5u - 14 = 0 $$

$$ (u - 7)(u + 2) = 0 $$

$$ u - 7 = 0 $$

$$ u = 7 $$

$$ (7)^2 - 5(7) - 14 = 0 $$

$$ 49 - 35 - 14 = 0 $$

$$ 0 = 0 $$

$$ u + 2 = 0 $$

$$ u = -2 $$

$$ (-2)^2 - 5(-2) - 14 = 0 $$

$$ 4 - (-10) - 14 = 0 $$

$$ 4 + 10 - 14 = 0 $$

$$ 14 - 14 = 0 $$

$$ 0 = 0 $$

$$ u = \{7, -2\} $$

**2.**

$$ x^2 + 15x = -50 $$

$$ x^2 + 15x + 50 = 0 $$

$$ (x + 5)(x + 10) = 0 $$

$$ x + 5 = 0 $$

$$ x = -5 $$

$$ (-5)^2 + 15(-5) = -50 $$

$$ 25 - 75 = -50 $$

$$ -50 = -50 $$

$$ x + 10 = 0 $$

$$ x = -10 $$

$$ (-10)^2 + 15(-10) = -50 $$

$$ 100 - 150 = -50 $$

$$ -50 = -50 $$

$$ x = \{-5, -10\} $$

**3.**

$$ y^2 = 11y - 28 $$

$$ y^2 - 11y + 28 = 0 $$

$$ (y - 7)(y - 4) = 0 $$

$$ y - 7 = 0 $$

$$ y = 7 $$

$$ (7)^2 = 11(7) - 28 $$

$$ 49 = 77 - 28 $$

$$ 49 = 49 $$

$$ y - 4 = 0 $$

$$ y = 4 $$

$$ (4)^2 = 11(4) - 28 $$

$$ 16 = 44 - 28 $$

$$ 16 = 16 $$

$$ y = \{7, 4\} $$

**4.**

$$ 19x = 7 - 6x^2 $$

$$ 6x^2 + 19x - 7 = 0 $$

$$ (3x - 1)(2x + 7) = 0 $$

$$ 3x - 1 = 0 $$

$$ 3x = 1 $$

$$ x = \frac{1}{3} $$

$$ 19\left(\frac{1}{3}\right) = 7 - 6\left(\frac{1}{3}\right)^2 $$

$$ \frac{19}{3} = 7 -6\left(\frac{1}{9}\right) $$

$$ \frac{19}{3} = 7 - \frac{6}{9} $$

$$ \frac{19}{3} = \frac{21}{3} - \frac{2}{3} $$

$$ \frac{19}{3} = \frac{19}{3} $$

$$  $$

$$ 2x + 7 = 0 $$

$$ 2x = -7 $$

$$ x = -\frac{7}{2} $$

$$ 19\left(-\frac{7}{2}\right) = 7 - 6\left(-\frac{7}{2}\right)^2 $$

$$ -\frac{133}{2} = 7 - 6\left(\frac{49}{4}\right) $$

$$ -\frac{133}{2} = 7 - \frac{147}{2} $$

$$ -\frac{133}{2} = \frac{14}{2} - \frac{147}{2} $$

$$ -\frac{133}{2} = -\frac{133}{2} $$

$$ x = \left\{\frac{1}{3}, -\frac{7}{2}\right\} $$

**5.**

$$ 6w^2 - w = 5 $$

$$ 6w^2 - w - 5 = 0 $$

$$ (6w + 5)(w - 1) = 0 $$

$$ 6w + 5 = 0 $$

$$ 6w = -5 $$

$$ w = -\frac{5}{6} $$

$$ 6\left(-\frac{5}{6}\right)^2 - \left(-\frac{5}{6}\right) = 5 $$

$$ 6\left(\frac{25}{36}\right) + \frac{5}{6} = 5 $$

$$ \frac{25}{6} + \frac{5}{6} = 5 $$

$$ \frac{30}{6} = 5 $$

$$ 5 = 5 $$

$$ w - 1 = 0 $$

$$ w = 1 $$

$$ 6(1)^2 - (1) = 5 $$

$$ 6(1) - 1 = 5 $$

$$ 6 - 1 = 5 $$

$$ 5 = 5 $$

$$ w = \left\{-\frac{5}{6}, 1\right\} $$

**6.**

$$ z^2 - 16z + 61 = 2z - 20 $$

$$ z^2 -16z - 2z +  61 + 20 =0 $$

$$ z^2 - 18z + 81 = 0 $$

$$ (z - 9)(z - 9) = 0 $$

$$ z - 9 = 0 $$

$$ z = 9 $$

$$ (9)^2 - 16(9) + 61 = 2(9) - 20 $$

$$ 81 - 144 + 61 = 18 - 20 $$

$$ -2 = -a $$

$$ z = \{9\} $$

**7.**

$$ 12x^2 = 25x $$

$$ 12x^2 - 25x = 0 $$

$$ x(12x - 25) = 0 $$

$$ x = 0 $$

$$ 12(0)^2 = 25(0) $$

$$ 12(0) = 0 $$

$$ 0 = 0 $$

$$ 12x - 25 = 0 $$

$$ 12x = 25 $$

$$ x = \frac{25}{12} $$

$$ 12\left(\frac{25}{12}\right)^2 = 25\left(\frac{25}{12}\right) $$

$$ 12\left(\frac{625}{144}\right) = \frac{625}{12} $$

$$ \frac{625}{12}= \frac{625}{12} $$

$$ x = \left\{0, \frac{25}{12}\right\} $$

---

For problems 8 & 9 use factoring to solve the equation.

**8.**

$$ x^4 - 2x^3 -3x^2 = 0 $$

$$ x^2(x^2 - 2x - 3) = 0 $$

$$ x^2(x - 3)(x + 1) = 0  $$

$$ x^2 = 0 $$

$$ x = \sqrt{0} $$

$$ x = 0 $$

$$ (0)^4 - 2(0)^3 -3(0)^2 = 0 $$

$$ 0 - 2(0) - 3(0) = 0 $$

$$ 0 = 0 $$

$$ x - 3 = 0 $$

$$ x = 3 $$

$$ (3)^4 - 2(3)^3 -3(3)^2 = 0 $$

$$ 81 - 2(27) - 3(9) = 0 $$

$$ 81 - 54 - 27 = 0 $$

$$ 0 = 0 $$

$$ x + 1 = 0 $$

$$ x = -1 $$

$$ (-1)^4 - 2(-1)^3 -3(-1)^2 = 0 $$

$$ 1 - 2(-1) - 3(1) = 0 $$

$$ 1 + 2 - 3 = 0 $$

$$ 0 = 0 $$

$$ x = \{0,3,-1\} $$

**9.**

$$ t^5 = 9t^3 $$

$$ t^5 - 9t^3 = 0 $$

$$ t^3(t^2 - 9) = 0 $$

$$ t^3(t + 3)(t - 3) = 0 $$

$$ t^3 = 0 $$

$$ t = \sqrt[3]{0} $$

$$ t = 0 $$

$$ (0)^5 = 9(0)^3 $$

$$ 0 = 9(0) $$

$$ 0 = 0 $$

$$ t + 3 = 0 $$

$$ t = -3 $$

$$ (-3)^5 = 9(-3)^3 $$

$$ -243 = 9(-27) $$

$$ -243 = -243 $$

$$ t - 3 = 0 $$

$$ t = 3 $$

$$ (3)^5 = 9(3)^3 $$

$$ 243 = 9(27) $$

$$ 243 = 243 $$

$$ t = \{0,3,-3\} $$

---

For problems 10 - 12 use factoring to solve the equation.

**10.**

$$ \frac{w^2 - 10}{w + 2} + w - 4 = w - 3 $$

$$ \frac{w^2 - 10}{w + 2} \cancel{+ w} - 4 = \cancel{w} - 3 $$

$$ \frac{w^2 - 10}{w + 2} = -3 + 4 $$

$$ \frac{w^2 - 10}{w + 2} = 1 $$

$$ (w + 2)\left(\frac{w^2 - 10}{w + 2}\right) = (1)(w + 2) $$

$$ w^2 - 10 = w + 2 $$

$$ w^2 - w - 12 = 0$$

$$ (w - 4)(w + 3) = 0 $$

$$ w - 4 = 0 $$

$$ w = 4 $$

$$ \frac{(4)^2 - 10}{(4) + 2} + (4) - 4 = (4) - 3 $$

$$ \frac{16 - 10}{6} + 0 = 1 $$

$$ \frac{6}{6} = 1 $$

$$ 1 = 1 $$

$$ w + 3 = 0 $$

$$ w = -3 $$

$$ \frac{(-3)^2 - 10}{(-3) + 2} + (-3) - 4 = (-3) - 3 $$

$$ \frac{9 - 10}{-1} - 7 = -6 $$

$$ \frac{-1}{-1} - 7 = -6 $$

$$ 1 - 7 = -6 $$

$$ -6 = -6 $$

$$ w =\{4,-3\} $$

**11.**

$$ \frac{4z}{z + 1} + \frac{5}{z} = \frac{6z + 5}{z^2 + z} $$

$$ LCD=(z+1)(z)(z^2 +z) $$

$$ (z + 1)(z)(z^2 + z)\left(\frac{4z}{z + 1} + \frac{5}{z}\right) = \left(\frac{6z + 5}{z^2 + z}\right)(z + 1)(z)(z^2 + z) $$

$$ 4z(z)(z^2 + z) + 5(z + 1)(z^2 + z) = (6z + 5)(z + 1)(z) $$

$$ 4z(z^3 + z^2) + 5(z^3 + z^2 + z^2 + z) = (6z^2 + 5z +6z + 5)(z) $$

$$ 4z^4 + 4z^3 + 5z^3 + 5z^2 + 5z^2 + 5z = 6z^3 + 5z^2 + 6z^2 + 5z $$

$$ 4z^4 + 9z^3 + 10z^2 + 5z = 6z^3 + 11z^2 + 5z $$

$$ 4z^4 + 3z^3 - z^2 = 0 $$

$$ z^2(4z^2 + 3z - 1) = 0 $$

$$ z^2(4z - 1)(z + 1) = 0 $$

$$ z^2 = 0 $$

$$ z = \sqrt{0} $$

$$ z = 0 $$

$$ \frac{4(0)}{(0) + 1} + \frac{5}{(0)} = \frac{6(0) + 5}{(0)^2 + (0)} $$

$$ \text{NO DIVISION BY ZERO} $$

$$ z \neq 0 $$

$$ 4z - 1 = 0 $$

$$ 4z = 1 $$

$$ z = \frac{1}{4} $$

$$ \frac{4\left(\dfrac{1}{4}\right)}{\left(\dfrac{1}{4}\right) + 1} + \frac{5}{\left(\dfrac{1}{4}\right)} = \frac{6\left(\dfrac{1}{4}\right) + 5}{\left(\dfrac{1}{4}\right)^2 + \left(\dfrac{1}{4}\right)} $$

$$ \frac{4}{5} + 20 = \frac{104}{5} $$

$$ \frac{104}{5} = \frac{104}{5} $$

$$ z + 1 = 0 $$

$$ z = -1 $$

$$ \frac{4(-1)}{(-1) + 1} + \frac{5}{(-1)} = \frac{6(-1) + 5}{(-1)^2 + (-1)} $$

$$ \frac{-4}{0} + \frac{5}{-1} = \frac{-6 + 5}{0} $$

$$ \text{NO DIVISION BY ZERO} $$

$$ z \neq -1 $$

$$ z = \left\{\frac{1}{4}\right\} $$

**12.**

$$ x + 1 = \frac{2x - 7}{x + 5} - \frac{5x + 8}{x + 5} $$

$$ LCD = (x + 5) $$

$$ (x + 5)(x + 1) = \left(\frac{2x - 7}{x + 5} - \frac{5x + 8}{x + 5}\right)(x + 5) $$

$$ x^2 + 5x + x + 5 = (2x - 7) - (5x + 8)$$

$$ x^2 + 6x + 5 = 2x - 7 - 5x - 8 $$

$$ x^2 + 6x + 5 = -3x - 15 $$

$$ x^2 + 6x + 3x + 5 + 15 = 0 $$

$$ x^2 + 9x + 20 = 0 $$

$$ (x + 5)(x + 4) = 0 $$

$$ x + 5 = 0 $$

$$ x = -5 $$

$$ (-5) + 1 = \frac{2(-5) - 7}{(-5) + 5} - \frac{5(-5) + 8}{(-5) + 5} $$

$$ -4 = \frac{-10 - 7}{0} - \frac{-25 + 8}{0} $$

$$ \text{NO DIVISION BY ZERO} $$

$$ x \neq -5 $$

$$ x + 4 = 0 $$

$$ x = -4 $$

$$ (-4) + 1 = \frac{2(-4) - 7}{(-4) + 5} - \frac{5(-4) + 8}{(-4) + 5} $$

$$ -3 = \frac{-8 - 7}{1} - \frac{-20 + 8}{1} $$

$$ -3 = -15 - (-12) $$

$$ -3 = -15 + 12 $$

$$ -3 = -3 $$

$$ x = \{-4\} $$

---

For problems 13 - 16 use the Square Root Property to solve the equation.

**13.**

$$ 9u^2 - 16 = 0 $$

$$ 9u^2 = 16 $$

$$ u^2 = \frac{16}{9} $$

$$ u = \pm \sqrt{\frac{16}{9}} $$

$$ u = \pm \frac{4}{3} $$

$$ u = \frac{4}{3} $$

$$ 9\left(\frac{4}{3}\right)^2 - 16 = 0 $$

$$ 9\left(\frac{16}{9}\right) - 16 = 0 $$

$$ 16 - 16 = 0 $$

$$ 0 = 0 $$

$$ u = -\frac{4}{3} $$

$$ 9\left(-\frac{4}{3}\right)^2 - 16 = 0 $$

$$ 9\left(\frac{16}{9}\right) - 16 = 0 $$

$$ 16 - 16 = 0 $$

$$ 0 = 0 $$

$$ u = \left\{\frac{4}{3}, -\frac{4}{3}\right\} $$

**14.**

$$ x^2 + 15 = 0 $$

$$ x^2 = - 15 $$

$$ x = \pm \sqrt{-15} $$

$$ x = \pm \sqrt{-1(15)} $$

$$ x = \pm \sqrt{15}i $$

**15.**

$$ (z - 2)^2 - 36 = 0 $$

$$ (z - 2)^2 = 36 $$

$$ z - 2 = \pm \sqrt{36} $$

$$ z = 2 \pm \sqrt{36} $$

$$ z = 2 \pm 6 $$

$$ z = 2 + 6 $$

$$ z = 8 $$

$$ ((8) - 2)^2 - 36 = 0 $$

$$ 6^2 - 36 = 0 $$

$$ 36 - 36 = 0 $$

$$ 0 = 0 $$

$$ z = 2 - 6 $$

$$ z = -4 $$

$$ ((-4) - 2)^2 - 36 = 0 $$

$$ (-6)^2 - 36 = 0 $$

$$ 36 - 36 = 0 $$

$$ 0 = 0 $$

$$ z = \{8, -4\} $$

**16.**

$$ (6t + 1)^2 + 3 = 0 $$

$$ (6t + 1)^2 = -3 $$

$$ 6t + 1 = \pm \sqrt{-3} $$

$$ 6t + 1 = \pm \sqrt{-1(3)} $$

$$ 6t + 1 = \pm \sqrt{3}i $$

$$ 6t = -1 \pm \sqrt{3}i $$

$$ t = \frac{-1 \pm \sqrt{3}i}{6} $$

$$ t = \frac{-1}{6} \pm \frac{\sqrt{3}i}{6} $$

---

## Assignment Problems

For probmes 1 - 15 solve the quadratic equation by factoring.

**1.**

$$ z^2 - 11z + 24 = 0 $$

**2.**

$$ w^2 + 13w + 12 = 0 $$

**3.**

$$ x^2 + 32 = 12x $$

**4.**

$$ y^2 = 6y + 27 $$

**5.**

$$ u^2 - 4u - 20 = 3u + 24 $$

**6.**

$$ z^2 - 36 = 0 $$

**7.**

$$ 144x^2 - 25 = 0 $$

**8.**

$$ 7x^2 + 19x = 6 $$

**9.**

$$ 4y^2 + 15y + 6 = 4y $$

**10.**

$$ 6z^2 - 11z + 15 = 12z - 5 $$

**11.**

$$ 20v^2 + 3v = 5v^2 + 5v + 1 $$

**12.**

$$ x^2 - 4x + 16 = 4x $$

**13.**

$$ 9y^2 + 17y + 20 = 4 - 7y $$

**14.**

$$ 7u^2 + 9u = 0 $$

**15.**

$$ 14x = 3x^2 $$

---

For problems 16 - 18 use factoring to solve the equation.

**16.**

$$ 3v^3 - 19v^2 + 14v = 0 $$

**17.**

$$ y^6 + y^5 = 20y^4 $$

**18.**

$$ z^4 + 2z^3 + z^2 = 0 $$

---

For problems 19 - 22 use factoring to solve the equation.

**19.**

$$ 1 + \frac{1}{x + 2} = \frac{12 - x}{x^2 + x - 6} $$

**20.**

$$ \frac{t + 1}{t + 2} = \frac{4(t - 5)}{t^2 + 2t} + \frac{4}{t} $$

**21.**

$$ \frac{w^2 - 1}{w + 6} = \frac{5 - 5w}{w + 6} - w $$

**22.**

$$ \frac{y - 2}{y - 9} + \frac{y^2 - 19y + 34}{y^2 - 10y + 9} = \frac{y - 3}{y - 1} $$

---

For problems 23 - 31 use the Square Root Property to solve the equation.

**23.**

$$ v^2 - 144 = 0 $$

**24.**

$$ 81x^2 - 25 = 0 $$

**25.**

$$ 4t^2 + 1 = 0 $$

**26.**

$$ 7y^2 - 3 = 0 $$

**27.**

$$ 14 + 2x^2 = 0 $$

**28.**

$$ (3t - 8)^2 - 16 = 0 $$

**29.**

$$ (u + 11)^2 + 6 = 0 $$

**30.**

$$ 4(2x - 1)^2 - 36 = 0 $$

**31.**

$$ (4 - z)^2 - 121 = 0 $$
