# 2.6 Quadratic Equations - Part II

---

$$ ax^2 + bx + c = 0 \text{ } a \neq 0 $$

---

**Completing the Square**

$$ x^2 + bx $$

$$ x^2 + bx + \left(\frac{b}{2}\right)^2 = \left(x + \frac{b}{2}\right)^2 $$

---

**Example 1**

Complete the square on each of the following.

**(a)**

$$ x^2 - 16x $$

$$ \left(\frac{-16}{2}\right)^2 = (\textcolor{blue}{-8})^2 = 64 $$

$$ x^2 - 16x \textcolor{red}{+ 64} = (x \textcolor{blue}{- 8})^2 $$

**(b)**

$$ y^2 + 7y $$

$$ \left(\textcolor{blue}{\frac{7}{2}}\right)^2 = \frac{49}{4} $$

$$ y^2 + 7y \textcolor{red}{+ \frac{49}{4}} = \left(y \textcolor{blue}{+ \frac{7}{2}}\right)^2  $$

---

**Example 2**

Use completing the square to solve each of the following quadratic equations.

$$ x^2 + bx + \left(\frac{b}{2}\right)^2 = \left(x + \frac{b}{2}\right)^2 $$

**(a)**

$$ x^2 - 6x + 1 = 0 $$

$$ x^2 - 6x = -1 $$

$$ \left(\frac{-6}{2}\right)^2 = (-3)^2 = 9 $$

$$ x^2 - 6x \textcolor{red}{+ 9} = -1 \textcolor{red}{+ 9} $$

$$ x^2 - 6x + 9 = 8 $$

$$ (x - 3)(x - 3) = 8 $$

$$ (x - 3)^2 = 8 $$

$$ \sqrt{(x - 3)^2} = \pm \sqrt{8} $$

$$ x - 3 = \pm \sqrt{8} $$

$$ x = 3 \pm \sqrt{8} $$

**(b)**

$$ 2x^2 + 6x + 7 = 0 $$

$$ 2x^2 + 6x = -7 $$

$$ x^2 + 3x = -\frac{7}{2} $$

$$ \left(\frac{3}{2}\right)^2 = \frac{9}{4} $$

$$ x^2 + 3x + \frac{9}{4} = -\frac{7}{2} + \frac{9}{4} $$

$$ x^2 + 3x + \frac{9}{4} = -\frac{14}{4} + \frac{9}{4} $$

$$ \left(x + \frac{3}{2}\right)^2 = -\frac{5}{4} $$

$$ \sqrt{\left(x + \frac{3}{2}\right)^2} = \pm \sqrt{-\frac{5}{4}} $$

$$ x + \frac{3}{2} = \pm \sqrt{-\frac{5}{4}} $$

$$ x = -\frac{3}{2} \pm \sqrt{\frac{5}{4}}i $$

**(c\)**

$$ 3x^2 - 2x - 1 = 0 $$

$$ x^2 - \frac{2}{3}x - \frac{1}{3} = 0 $$

$$ x^2 - \frac{2}{3}x = \frac{1}{3} $$

$$ \left(\frac{-\dfrac{2}{3}}{2}\right)^2 = \left(-\frac{1}{3}\right)^2 = \frac{1}{9} $$

$$ x^2 - \frac{2}{3}x + \frac{1}{9} = \frac{1}{3} + \frac{1}{9} $$

$$ \left(x - \frac{1}{3}\right)^2 = \frac{4}{9} $$

$$ \sqrt{\left(x - \frac{1}{3}\right)^2} = \pm \sqrt{\frac{4}{9}} $$

$$ x - \frac{1}{3} = \pm \sqrt{\frac{4}{9}} $$

$$ x = \frac{1}{3} \pm \sqrt{\frac{4}{9}} $$

$$ x = \frac{1}{3} \pm \frac{2}{3} $$

$$ x = \frac{1}{3} + \frac{2}{3} $$

$$ x = 1 $$

$$ 3(1)^2 - 2(1) - 1 = 0 $$

$$ 3(1) - 2 - 1 = 0 $$

$$ 3 - 2 - 1 = 0 $$

$$ 0 = 0 $$

$$ x = \frac{1}{3} - \frac{2}{3} $$

$$ x = -\frac{1}{3} $$

$$ 3\left(-\frac{1}{3}\right)^2 - 2\left(-\frac{1}{3}\right) - 1 = 0 $$

$$ 3\left(\frac{1}{9}\right) + \frac{2}{3} - 1 = 0 $$

$$ \frac{3}{9} + \frac{2}{3} - 1 = 0 $$

$$ \frac{1}{3} + \frac{2}{3} - 1 = 0 $$

$$ \frac{3}{3} - 1 = 0 $$

$$ 1 - 1 = 0 $$

$$ 0 = 0 $$

$$ x = \left\{1, -\frac{1}{3}\right\} $$

---

**Quadratic Formula**

The following demonstrates how a standard form quadratic equation can be broken
down to show the quadratic formula, which grants us the ability to always solve
for $x$.

$$ ax^2 + bx + c = 0 $$

$$ x^2 + \left(\frac{b}{a}\right)x + \frac{c}{a} = 0 $$

Finding the number to complete the square:

$$ \left(\frac{b}{2a}\right)^2 = \frac{b^2}{4a^2} $$

$$ x^2 + \left(\frac{b}{a}\right)x + \frac{b^2}{4a^2} = \frac{b^2}{4a^2} - \frac{c}{a} $$

$$ \left(x + \frac{b}{2a}\right)^2 = \frac{b^2 - 4ac}{4a^2} $$

$$ x + \frac{b}{2a} = \pm \sqrt{\frac{b^2 - 4ac}{4a^2}} $$

$$ x = -\frac{b}{2a} \pm \sqrt{\frac{b^2 - 4ac}{4a^2}} $$

$$ x = \frac{-b \pm \sqrt{b^2 - 4ac}}{2a} $$

---

**Example 3**

Use the quadratic formula to solve each of the following equations.

**(a)**

$$ x^2 + 2x = 7 $$

$$ x^2 + 2x - 7 = 0 $$

$$ a = 1 $$

$$ b = 2 $$

$$ c = -7 $$

$$ x = \frac{-b \pm \sqrt{b^2 - 4ac}}{2a} $$

$$ x = \frac{-(2) \pm \sqrt{(2)^2 - 4(1)(-7)}}{2(1)} $$

$$ x = \frac{-2 \pm \sqrt{16(2)}}{2} $$

$$ x = \frac{-2 \pm 4\sqrt{2}}{2} $$

$$ x = -1 \pm 2\sqrt{2} $$

$$  $$

**(b)**

$$ 3q^2 + 11 = 5q $$

$$ 3q^2 - 5q + 11 = 0 $$

$$ a = 3 $$

$$ b = -5 $$

$$ c = 11 $$

$$ x = \frac{-b \pm \sqrt{b^2 - 4ac}}{2a} $$

$$ q = \frac{-(-5) \pm \sqrt{(-5)^2 - 4(3)(11)}}{2(3)} $$

$$ q = \frac{5 \pm \sqrt{-107}}{6} $$

$$ q = \frac{5 \pm \sqrt{107}i}{6} $$

$$  $$

**(c\)**

$$ 7t^2 = 6 - 19t $$

$$ 7t^2 + 19t - 6 = 0 $$

$$ a = 7 $$

$$ b = 19 $$

$$ c = -6 $$

$$ x = \frac{-b \pm \sqrt{b^2 - 4ac}}{2a} $$

$$ t = \frac{-(19) \pm \sqrt{(19)^2 - 4(7)(-6)}}{2(7)} $$

$$ t = \frac{-19 \pm \sqrt{529}}{14} $$

$$ t = \frac{-19 \pm 23}{14} $$

$$ t = \frac{-19 + 23}{14} $$

$$ t = \frac{4}{14} = \frac{2}{7} $$

$$ t = \frac{-19 - 23}{14} $$

$$ t = \frac{-42}{14} = -3 $$

$$ t = \left\{\frac{2}{7}, -3\right\} $$

**(d)**

$$ \frac{3}{y - 2} = \frac{1}{y} + 1 $$

$$ LCD = (y)(y - 2) $$

$$ (y)(y - 2)\left(\frac{3}{y - 2}\right) = \left(\frac{1}{y} + 1\right)(y)(y - 2) $$

$$ 3y = (y - 2) + (y)(y - 2) $$

$$ 3y = y - 2 + y^2 - 2y $$

$$ 3y = y^2 - y - 2 $$

$$ 0 = y^2 - 4y - 2 $$

$$ y^2 - 4y - 2 = 0 $$

$$ a = 1 $$

$$ b = -4 $$

$$ c = -2 $$

$$ x = \frac{-b \pm \sqrt{b^2 - 4ac}}{2a} $$

$$ y = \frac{-(-4) \pm \sqrt{(-4)^2 - 4(1)(-2)}}{2(1)} $$

$$ y = \frac{4 \pm \sqrt{4(6)}}{2} $$

$$ y = \frac{4 \pm 2\sqrt{6}}{2} $$

$$ y = \frac{4}{2} \pm \frac{2}{2}\sqrt{6} $$

$$ y = 2 \pm \sqrt{6} $$

**(e)**

$$ 16x - x^2 = 0 $$

$$ 0 = x^2 - 16x $$

$$ x^2 - 16x = 0 $$

$$ a = 1 $$

$$ b = -16 $$

$$ c = 0 $$

$$ x = \frac{-b \pm \sqrt{b^2 - 4ac}}{2a} $$

$$ x = \frac{-(-16) \pm \sqrt{(-16)^2 - 4(1)(0)}}{2(1)} $$

$$ x = \frac{16 \pm \sqrt{256}}{2} $$

$$ x = \frac{16 \pm 16}{2} $$

$$ x = \frac{16}{2} \pm \frac{16}{2} $$

$$ x = 8 \pm 8 $$

$$ x = 8 + 8 $$

$$ x = 16 $$

$$ 16(16) - (16)^2 = 0 $$

$$ 256 - 256 = 0 $$

$$ 0 = 0 $$

$$ x = 8 - 8 $$

$$ x = 0 $$

$$ 16(0) - (0)^2 = 0 $$

$$ 0 - 0 = 0 $$

$$ 0 = 0 $$

$$ x = \{16, 0\} $$

---

**Example 4**

Solve each of the following equations.

**(a)**

$$ \frac{1}{2}x^2 + x - \frac{1}{10} = 0 $$

$$ a = \frac{1}{2} $$

$$ b = 1 $$

$$ c = -\frac{1}{10} $$

$$ x = \frac{-b \pm \sqrt{b^2 - 4ac}}{2a} $$

$$ x = \frac{-(1) \pm \sqrt{(1)^2 - 4\left(\dfrac{1}{2}\right)\left(-\dfrac{1}{10}\right)}}{2\left(\dfrac{1}{2}\right)} $$

$$ x = \frac{-1 \pm \sqrt{1 + \dfrac{1}{5}}}{1} $$

$$ x = -1 \pm \sqrt{\frac{6}{5}} $$

$$ x = -1 \pm \frac{\sqrt{30}}{5} $$

**(b)**

$$ 0.04x^2 - 0.23x + 0.09 = 0 $$

$$ x = \frac{-b \pm \sqrt{b^2 - 4ac}}{2a} $$

$$ a = 0.04 $$

$$ b = -0.23 $$

$$ c = 0.09 $$

$$ x = \frac{-b \pm \sqrt{b^2 - 4ac}}{2a} $$

$$ x = \frac{-(-0.23) \pm \sqrt{(-0.23)^2 - 4(0.04)(0.09)}}{2(0.04)} $$

$$ x = \frac{0.23 \pm \sqrt{0.0385}}{0.08} $$

$$ x = \frac{0.23 \pm 0.19621}{0.08} $$

$$ x = \frac{0.23 + 0.19621}{0.08} $$

$$ x = 5.327625 $$

$$ x = \frac{0.23 - 0.19621}{0.08} $$

$$ x = 0.422375 $$

---

## Practice Problems

---

For problems 1 - 3 complete the square.

$$ x^2 + bx $$

$$ x^2 + bx + \left(\frac{b}{2}\right)^2 = \left(x + \frac{b}{2}\right)^2 $$

**1.**

$$ x^2 + 8x $$

$$ \left(\frac{8}{2}\right)^2 = (4)^2 = 16 $$

$$ x^2 + 8x + 16 = (x + 4)^2 $$

**2.**

$$ u^2 - 11u $$

$$ \left(-\frac{11}{2}\right)^2 $$

$$ u^2 - 11u + \left(-\frac{11}{2}\right)^2 = \left(u - \frac{11}{2}\right)^2 $$

$$ u^2 - 11u + \frac{121}{4} = \left(u - \frac{11}{2}\right)^2 $$

**3.**

$$ 2z^2 - 12z $$

$$ 2(z^2 - 6z) $$

$$ \left(-\frac{6}{2}\right)^2 = (-3)^2 = 9 $$

$$ 2z^2 - 12z = 2(z^2 - 6z + 9) = 2(z - 3)^2 $$

---

For problems 4 – 8 solve the quadratic equation by completing the square.

**4.**

$$ t^2 - 10t + 34 = 0 $$

$$ t^2 - 10t = -34 $$

$$ \left(-\frac{10}{2}\right)^2 = (-5)^2 = 25 $$

$$ t^2 - 10t + 25 = -34 + 25 $$

$$ (t - 5)^2 = -9 $$

$$ \sqrt{(t - 5)^2} = \pm \sqrt{-9} $$

$$ t - 5 =  \pm 3i $$

$$ t = 5 \pm 3i $$

$$ t = \{5 + 3i, 5 - 3i\} $$

**5.**

$$ v^2 + 8v - 9 = 0 $$

$$ v^2 + 8v = 9 $$

$$ \left(\frac{8}{2}\right)^2 = (4)^2 = 16 $$

$$ v^2 + 8v + 16 = 9 + 16 $$

$$ (v + 4)^2 = 25 $$

$$ \sqrt{(v + 4)^2} = \pm \sqrt{25} $$

$$ v + 4 = \pm 5 $$

$$ v = -4 \pm 5 $$

$$ v = -4 + 5 $$

$$ v = 1 $$

$$ (1)^2 + 8(1) - 9 = 0 $$

$$ 1 + 8 - 9 = 0 $$

$$ 9 - 9 = 0 $$

$$ 0 = 0 $$

$$ v = -4 - 5 $$

$$ v = -9 $$

$$ (-9)^2 + 8(-9) - 9 = 0 $$

$$ 81 - 72 - 9 = 0 $$

$$ 9 - 9 = 0 $$

$$ 0 = 0 $$

$$ v = \{1, -9\} $$

**6.**

$$ x^2 + 9x + 16 = 0 $$

$$ x^2 + 9x = -16 $$

$$ \left(\frac{9}{2}\right)^2 = \frac{(9)^2}{(2)^2} = \frac{81}{4} $$

$$ x^2 + 9x + \frac{81}{4} = -16 + \frac{81}{4} $$

$$ \left(x + \frac{9}{2}\right)^2 = \frac{17}{4} $$

$$ \sqrt{\left(x + \frac{9}{2}\right)^2} = \pm \sqrt{\frac{17}{4}} $$

$$ x + \frac{9}{2} = \pm \frac{\sqrt{17}}{2}$$

$$ x = \frac{9}{2} \pm \frac{\sqrt{17}}{2}$$

$$ x = \frac{9 \pm \sqrt{17}}{2} $$

$$ x = \left\{\frac{9 + \sqrt{17}}{2}, \frac{9 - \sqrt{17}}{2}\right\} $$

**7.**

$$ 4u^2 - 8u + 5 = 0 $$

$$ u^2 - \frac{8}{4}u + \frac{5}{4} = 0 $$

$$ u^2 - 2u = -\frac{5}{4} $$

$$ \left(-\frac{2}{2}\right)^2 = (-1)^2 = 1 $$

$$ u^2 - 2u + 1 = -\frac{5}{4} + 1 $$

$$ (u - 1)^2 = -\frac{1}{4} $$

$$ \sqrt{(u - 1)^2} = \pm \sqrt{-\frac{1}{4}} $$

$$ u - 1 = \pm \frac{1}{2}i $$

$$ u = 1 \pm \frac{1}{2}i $$

$$ u = \left\{1 + \frac{1}{2}i, 1 - \frac{1}{2}i\right\} $$

**8.**

$$ 2x^2 + 5x + 3 = 0 $$

$$ x^2 + \frac{5}{2}x + \frac{3}{2} = 0 $$

$$ x^2 + \frac{5}{2}x = -\frac{3}{2} $$

$$ \left(\frac{\dfrac{5}{2}}{2}\right)^2 = \left(\frac{5}{4}\right)^2 = \frac{25}{16} $$

$$ x^2 + \frac{5}{2}x + \frac{25}{16} = -\frac{3}{2} + \frac{25}{16} $$

$$ \left(x + \frac{5}{4}\right)^2 = \frac{1}{16} $$

$$ \sqrt{\left(x + \frac{5}{4}\right)^2} = \pm \sqrt{\frac{1}{16}} $$

$$ x + \frac{5}{4} = \pm \frac{1}{4} $$

$$ x = -\frac{5}{4} \pm \frac{1}{4} $$

$$ x = -\frac{5}{4} + \frac{1}{4} $$

$$ x = -\frac{4}{4} $$

$$ x = -1 $$

$$ x = -\frac{5}{4} - \frac{1}{4} $$

$$ x = -\frac{6}{4} $$

$$ x = -\frac{3}{2} $$

$$ x = \left\{-1, -\frac{3}{2}\right\} $$

---

For problems 9 – 13 use the quadratic formula to solve the quadratic equation.

$$ x = \frac{-b \pm \sqrt{b^2 - 4ac}}{2a} $$

**9.**

$$ x^2 - 6x + 4 = 0 $$

$$ a = 1 $$

$$ b = -6 $$

$$ c = 4 $$

$$ x = \frac{-b \pm \sqrt{b^2 - 4ac}}{2a} $$

$$ x = \frac{-(-6) \pm \sqrt{(-6)^2 - 4(1)(4)}}{2(1)} $$

$$ x = \frac{6 \pm \sqrt{5(4)}}{2} $$

$$ x = \frac{6 \pm 2\sqrt{5}}{2} $$

$$ x = 3 \pm \sqrt{5} $$

$$ x = \{3 + \sqrt{5}, 3 - \sqrt{5}\} $$

**10.**

$$ 9w^2 - 6w = 101 $$

$$ 9w^2 - 6w - 101 = 0 $$

$$ a = 9 $$

$$ b = -6 $$

$$ c = -101 $$

$$ x = \frac{-b \pm \sqrt{b^2 - 4ac}}{2a} $$

$$ w = \frac{-(-6) \pm \sqrt{(-6)^2 - 4(9)(-101)}}{2(9)} $$

$$ w = \frac{6 \pm \sqrt{36(102)}}{18} $$

$$ w = \frac{6 \pm 6\sqrt{102}}{18} $$

$$ w = \frac{1}{3} \pm \frac{1}{3}\sqrt{102} $$

$$ w = \left\{\frac{1}{3} + \frac{1}{3}\sqrt{102}, \frac{1}{3} - \frac{1}{3}\sqrt{102}\right\} $$

**11.**

$$ 8u^2 + 5u + 70 = 5 - 7u $$

$$ 8u^2 + 5u + 7u + 70 - 5 = 0 $$

$$ 8u^2 + 12u + 65 = 0 $$

$$ a = 8 $$

$$ b = 12 $$

$$ c = 65 $$

$$ x = \frac{-b \pm \sqrt{b^2 - 4ac}}{2a} $$

$$ u = \frac{-(12) \pm \sqrt{(12)^2 - 4(8)(65)}}{2(8)} $$

$$ u = \frac{-12 \pm \sqrt{1936}i}{16} $$

$$ u = \frac{-12 \pm 44i}{16} $$

$$ u = -\frac{3}{4} \pm \frac{11}{4}i $$

$$ u = \left\{-\frac{3}{4} + \frac{11}{4}, -\frac{3}{4} - \frac{11}{4}i\right\} $$

**12.**

$$ 169 - 20t + 4t^2 = 0 $$

$$ 4t^2 - 20t + 169 = 0 $$

$$ a = 4 $$

$$ b = -20 $$

$$ c = 169 $$

$$ x = \frac{-b \pm \sqrt{b^2 - 4ac}}{2a} $$

$$ t = \frac{-(-20) \pm \sqrt{(-20)^2 - 4(4)(169)}}{2(4)} $$

$$ t = \frac{20 \pm \sqrt{2304}i}{8} $$

$$ t = \frac{20 \pm 48i}{8} $$

$$ t = \frac{5}{2} \pm 6i $$

$$ t = \left\{\frac{5}{2} + 6i, \frac{5}{2} - 6i\right\} $$

**13.**

$$ 2z^2 + z - 72 = z^2 - 2z + 58 $$

$$ 2z^2 - z^2 + z + 2z - 72 - 58 = 0 $$

$$ z^2 + 3z - 130 = 0 $$

$$ a = 1 $$

$$ b = 3 $$

$$ c = -130 $$

$$ x = \frac{-(b) \pm \sqrt{(b)^2 - 4(a)(c)}}{2(a)} $$

$$ z = \frac{-(3) \pm \sqrt{(3)^2 - 4(1)(-130)}}{2(1)} $$

$$ z = \frac{-3 \pm \sqrt{529}}{2} $$

$$ z = \frac{-3 \pm 23}{2} $$

$$ z = \frac{-3 + 23}{2} $$

$$ z = \frac{20}{2} $$

$$ z = 10 $$

$$ z = \frac{-3 - 23}{2} $$

$$ z = \frac{-26}{2} $$

$$ z = -13 $$

$$ z = \{10, 13\} $$

---

## Assignment Problems

---

For problems 1 – 6 complete the square.

**1.**

$$ w^2 + 3w $$

$$ \left(\frac{3}{2}\right)^2  = \frac{9}{4} $$

$$ w^2 + 3w + \frac{9}{4} = \left(w + \frac{3}{2}\right)^2 $$

**2.**

$$ x^2 - 10x $$

$$ \left(-\frac{10}{2}\right)^2 = (-5)^2 = 25 $$

$$ x^2 - 10x + 25 = (x - 5)^2 $$

**3.**

$$ y^2 + 14y $$

$$ \left(\frac{14}{2}\right)^2 = (7)^2 = 49 $$

$$ y^2 + 14y + 49 = (y + 7)^2 $$

**4.**

$$ 3u^2 - 36u $$

$$ 3(u^2 - 12u) $$

$$ \left(-\frac{12}{2}\right)^2 = (-6)^2 = 36 $$

$$ 3(u^2 - 12u + 36 - 36) $$

$$ 3((u - 6)^2 - 36) $$

$$ 3u^2 - 36u = 3(u - 6)^2 - 108 $$

**5.**

$$ 2t^2 - 9t $$

$$ 2\left(t^2 - \frac{9}{2}t\right) $$

$$ \left(\frac{-\dfrac{9}{2}}{2}\right)^2  = \left(-\frac{3}{2}\right)^2 = \frac{9}{4} $$

$$ 2\left(t^2 - \frac{9}{2}t + \frac{9}{4} - \frac{9}{4}\right) $$

$$ 2\left(\left(t - \frac{3}{2}\right)^2 - \frac{9}{4}\right) $$

$$ 2t^2 - 9t = 2\left(t - \frac{3}{2}\right)^2 - \frac{9}{2} $$

**6.**

$$ 18x - x^2 $$

$$ x^2 - 18x $$

$$ \left(-\frac{18}{2}\right)^2 = (-9)^2 = 81 $$

$$ x^2 - 18x + 81 = (x - 9)^2 $$

---

For problems 7 – 16 solve the quadratic equation by completing the square.

**7.**

$$ x^2 + 3x - 10 = 0 $$

$$ x^2 + 3x = 10 $$

$$ \left(\frac{3}{2}\right)^2 = \frac{9}{4} $$

$$ x^2 + 3x + \frac{9}{4} = 10 + \frac{9}{4} $$

$$ \left(x + \frac{3}{2}\right)^2 = \frac{49}{4} $$

$$ \sqrt{\left(x + \frac{3}{2}\right)^2} = \pm \sqrt{\frac{49}{4}} $$

$$ x + \frac{3}{2} = \pm \frac{7}{2} $$

$$ x = -\frac{3}{2} \pm \frac{7}{2} $$

$$ x = -\frac{3}{2} + \frac{7}{2} $$

$$ x = \frac{4}{2} $$

$$ x = 2 $$

$$ x = -\frac{3}{2} - \frac{7}{2} $$

$$ x = -\frac{10}{2} $$

$$ x = -5 $$

$$ x = \{2, -5\} $$

**8.**

$$ z^2 - 12z + 40 = 0 $$

$$ z^2 - 12z = -40 $$

$$ \left(-\frac{12}{2}\right)^2 = (-6)^2 = 36 $$

$$ z^2 - 12z + 36 = -40 + 36 $$

$$ (z - 6)^2 = -4 $$

$$ \sqrt{(z - 6)^2} = \pm \sqrt{-4} $$

$$ z - 6 = \pm \sqrt{4}i $$

$$ z = 6 \pm 2i $$

$$ z = \{6 + 2i, 6 - 2i\} $$

**9.**

$$ t^2 - 7t + 2 = 0 $$

$$ t^2 - 7t = -2 $$

$$ \left(-\frac{7}{2}\right)^2 = \frac{49}{4} $$

$$ t^2 - 7t + \frac{49}{4} = -2 + \frac{49}{4} $$

$$ \left(t - \frac{7}{2}\right)^2 = \frac{41}{4}  $$

$$ \sqrt{\left(t - \frac{7}{2}\right)^2} = \pm \sqrt{\frac{41}{4}} $$

$$ t - \frac{7}{2} = \pm \frac{\sqrt{41}}{2} $$

$$ t = \frac{7}{2}  \pm \frac{\sqrt{41}}{2} $$

$$ t = \left\{\frac{7}{2} + \frac{\sqrt{41}}{2}, \frac{7}{2} - \frac{\sqrt{41}}{2}\right\} $$

**10.**

$$ u^2 + 5u + 9 = 0 $$

$$ u^2 + 5u = -9 $$

$$ \left(\frac{5}{2}\right)^2 = \frac{25}{4} $$

$$ u^2 + 5u + \frac{25}{4} = -9 + \frac{25}{4} $$

$$ \left(u + \frac{5}{2}\right)^2 = -\frac{11}{4} $$

$$ \sqrt{\left(u + \frac{5}{2}\right)^2} = \pm \sqrt{-\frac{11}{4}} $$

$$ u + \frac{5}{2} = \pm \frac{\sqrt{11}}{2}i $$

$$ u = -\frac{5}{2} \pm \frac{\sqrt{11}}{2}i $$

$$ u = \left\{-\frac{5}{2} + \frac{\sqrt{11}}{2}i, -\frac{5}{2} - \frac{\sqrt{11}}{2}i\right\} $$

**11.**

$$ 4x^2 - 4x + 5 = 0 $$

$$ x^2 - x + \frac{5}{4} = 0 $$

$$ x^2 - x = -\frac{5}{4} $$

$$ \left(-\frac{1}{2}\right)^2 = \frac{1}{4} $$

$$ x^2 -x + \frac{1}{4} = -\frac{5}{4} + \frac{1}{4} $$

$$ \left(x - \frac{1}{2}\right)^2 = -1 $$

$$ \sqrt{\left(x - \frac{1}{2}\right)^2} = \pm \sqrt{-1} $$

$$ x - \frac{1}{2} = \pm i $$

$$ x = \frac{1}{2} \pm i $$

$$ x = \left\{\frac{1}{2} + i, \frac{1}{2} - i\right\} $$

**12.**

$$ 16w^2 + 8w + 1 = 0 $$

$$ w^2 + \frac{1}{2}w + \frac{1}{16} = 0 $$

$$ w^2 + \frac{1}{2}w = -\frac{1}{16} $$

$$ \left(\frac{\dfrac{1}{2}}{2}\right)^2 = \left(\frac{1}{4}\right)^2 = \frac{1}{16} $$

$$ w^2 + \frac{1}{2}w + \frac{1}{16} = -\frac{1}{16} + \frac{1}{16} $$

$$ \left(w + \frac{1}{4}\right)^2 = 0 $$

$$ \sqrt{\left(w + \frac{1}{4}\right)^2} = \pm \sqrt{0} $$

$$ w + \frac{1}{4} = 0 $$

$$ w = -\frac{1}{4} $$

$$ w = \left\{-\frac{1}{4}\right\} $$

**13.**

$$ 4y^2 - 24y + 29 = 0 $$

$$ y^2 - 6y + \frac{29}{4} = 0 $$

$$ y^2 - 6y = -\frac{29}{4} $$

$$ \left(-\frac{6}{2}\right)^2 = (-3)^2 = 9 $$

$$ y^2 - 6y + 9 = -\frac{29}{4} + 9 $$

$$ (y - 3)^2 = \frac{7}{4} $$

$$ \sqrt{(y - 3)^2} = \pm \sqrt{\frac{7}{4}} $$

$$ y - 3 = \pm \frac{\sqrt{7}}{2} $$

$$ y = 3 \pm \frac{\sqrt{7}}{2} $$

$$ y = \left\{3 + \frac{\sqrt{7}}{2}, 3 - \frac{\sqrt{7}}{2}\right\} $$

**14.**

$$ 81z^2 + 54z + 10 = 0 $$

$$ z^2 + \frac{54}{81}z + \frac{10}{81} = 0 $$

$$ z^2 + \frac{2}{3}z = -\frac{10}{81} $$

$$ \left(\frac{\dfrac{2}{3}}{2}\right)^2 = \left(\frac{1}{3}\right)^2 = \frac{1}{9} $$

$$ z^2 + \frac{2}{3}z + \frac{1}{9} = -\frac{10}{81} + \frac{1}{9} $$

$$ \left(z + \frac{1}{3}\right)^2 = -\frac{1}{81}  $$

$$ \sqrt{\left(z + \frac{1}{3}\right)^2 } = \pm \sqrt{-\frac{1}{81}} $$

$$ z + \frac{1}{3} = \pm \frac{1}{9}i $$

$$ z = -\frac{1}{3} \pm \frac{1}{9}i $$

$$ z = \left\{-\frac{1}{3} + \frac{1}{9}i, -\frac{1}{3} - \frac{1}{9}i\right\} $$

**15.**

$$ 9t^2 - 12t - 14 = 0 $$

$$ t^2 - \frac{4}{3}t - \frac{14}{9} = 0 $$

$$ t^2 - \frac{4}{3}t = \frac{14}{9} $$

$$ \left(-\frac{\dfrac{4}{3}}{2}\right)^2 = \left(-\frac{2}{3}\right)^2 = \frac{4}{9} $$

$$ t^2 - \frac{4}{3}t + \frac{4}{9} = \frac{14}{9} + \frac{4}{9} $$

$$ \left(t - \frac{2}{3}\right)^2 = 2 $$

$$ \sqrt{\left(t - \frac{2}{3}\right)^2} = \pm \sqrt{2} $$

$$ t - \frac{2}{3} = \pm \sqrt{2} $$

$$ t = \frac{2}{3} \pm \sqrt{2} $$

$$ t = \left\{\frac{2}{3} + \sqrt{2}, \frac{2}{3} - \sqrt{2}\right\} $$

**16.**

$$ 5v^2 - 14v + 11 = 0 $$

$$ v^2 - \frac{14}{5}v + \frac{11}{5} = 0 $$

$$ v^2 - \frac{14}{5}v = -\frac{11}{5} $$

$$ \left(-\frac{\dfrac{14}{5}}{2}\right)^2 = \left(-\frac{7}{5}\right)^2 = \frac{49}{25} $$

$$ v^2 - \frac{14}{5}v + \frac{49}{25} = -\frac{11}{5} + \frac{49}{25} $$

$$ \left(v - \frac{7}{5}\right)^2 = -\frac{6}{25} $$

$$ \sqrt{\left(v - \frac{7}{5}\right)^2} = \pm \sqrt{-\frac{6}{25}} $$

$$ v - \frac{7}{5} = \pm \frac{\sqrt{6}}{5}i $$

$$ v = \frac{7}{5} \pm \frac{\sqrt{6}}{5}i $$

$$ v = \left\{\frac{7}{5} + \frac{\sqrt{6}}{5}i, \frac{7}{5} - \frac{\sqrt{6}}{5}i\right\} $$

---

For problems 17 – 26 use the quadratic formula to solve the quadratic equation.

**17.**

$$ w^2 - 14w + 245 = 0 $$

$$ w = \frac{-(-14) \pm \sqrt{(-14)^2 - 4(1)(245)}}{2(1)} $$

$$ w = \frac{14 \pm \sqrt{-784}}{2} $$

$$ w = \frac{14 \pm 28i}{2} $$

$$ w = \frac{14}{2} \pm \frac{28}{2}i $$

$$ w = 7 \pm 14i $$

$$ w = \{7 + 14i, 7 - 14i\} $$

**18.**

$$ 3t^2 + 20t + 31 = 0 $$

$$ t = \frac{-(20) \pm \sqrt{(20)^2 - 4(3)(31)}}{2(3)} $$

$$ t = \frac{-20 \pm \sqrt{28}}{6} $$

$$ t = \frac{-20 \pm 2\sqrt{7}}{6} $$

$$ t = -\frac{10}{3} \pm \frac{\sqrt{7}}{3} $$

$$ t = \left\{-\frac{10}{3} + \frac{\sqrt{7}}{3}, -\frac{10}{3} - \frac{\sqrt{7}}{3}\right\} $$

**19.**

$$ 6x + 61 + 18x^2 = 0 $$

$$ 18x^2 + 6x + 61 = 0 $$

$$ x = \frac{-(6) \pm \sqrt{(6)^2 - 4(18)(61)}}{2(18)} $$

$$ x = \frac{-6 \pm \sqrt{-4356}}{36} $$

$$ x = \frac{-6 \pm 66i}{36} $$

$$ x = -\frac{1}{6} \pm \frac{11}{6}i $$

$$ x = \left\{-\frac{1}{6} + \frac{11}{6}i, -\frac{1}{6} - \frac{11}{6}i\right\} $$

**20.**

$$ x^2 = 4x - 23 $$

$$ x^2 - 4x + 23 = 0 $$

$$ x = \frac{-(-4) \pm \sqrt{(-4)^2 - 4(1)(23)}}{2(1)} $$

$$ x = \frac{4 \pm \sqrt{-76}}{2} $$

$$ x = \frac{4 \pm 2\sqrt{19}i}{2} $$

$$ x = 2 \pm \sqrt{19}i $$

$$ x = \{2 + \sqrt{19}i, 2 - \sqrt{19}i\} $$

**21.**

$$ y^2 + 20y = 4y - 64 $$

$$ y^2 + 20y - 4y - 64 = 0 $$

$$ y^2 + 16y - 64 = 0 $$

$$ y = \frac{-(16) \pm \sqrt{(16)^2 - 4(1)(-64)}}{2(1)} $$

$$ y = \frac{-16 \pm \sqrt{512}}{2} $$

$$ y = \frac{-16 \pm 16\sqrt{2}}{2} $$

$$ y = -8 \pm 8\sqrt{2} $$

$$ y = \{-8 + 8\sqrt{2}, -8 - 8\sqrt{2}\} $$

**22.**

$$ 33 = 8z + z^2 $$

$$ 0 = z^2 + 8z - 33 $$

$$ z^2 + 8z - 33 = 0 $$

$$ z = \frac{-(8) \pm \sqrt{(8)^2 - 4(1)(-33)}}{2(1)} $$

$$ z = \frac{-8 \pm \sqrt{196}}{2} $$

$$ z = \frac{-8 \pm 14}{2} $$

$$ z = -4 \pm 7 $$

$$ z = -4 + 7 $$

$$ z = 3 $$

$$ z = -4 - 7 $$

$$ z = -11 $$

$$ z = \{3, -11\} $$

**23.**

$$ 2t^2 + 49 = 32t - 2t^2 $$

$$ 2t^2 + 2t^2 - 32t +  49 = 0 $$

$$ 4t^2 - 32t + 49 = 0 $$

$$ t = \frac{-(-32) \pm \sqrt{(-32)^2 - 4(4)(49)}}{2(4)} $$

$$ t = \frac{32 \pm \sqrt{240}}{8} $$

$$ t = \frac{32 \pm 4\sqrt{15}}{8} $$

$$ t = 4 \pm \frac{\sqrt{15}}{2} $$

$$ t = \left\{4 + \frac{\sqrt{15}}{2}, 4 - \frac{\sqrt{15}}{2}\right\} $$

**24.**

$$ 40u + 25u^2 = 10u - 11 $$

$$ 25u^2 + 40u - 10u - 11 = 0 $$

$$ 25u^2 + 30u - 11 = 0 $$

$$ u = \frac{-(30) \pm \sqrt{(30)^2 - 4(25)(-11)}}{2(25)} $$

$$ u = \frac{-30 \pm \sqrt{2000}}{100} $$

$$ u = \frac{-30 \pm 20\sqrt{5}}{100} $$

$$ u = -\frac{3}{10} \pm \frac{2\sqrt{5}}{10} $$

$$ u = \left\{-\frac{3}{10} + \frac{2\sqrt{5}}{10}, -\frac{3}{10} - \frac{2\sqrt{5}}{10}\right\} $$

**25.**

$$ 10x^2 - 10x = 4x^2 - 3x + 10 $$

$$ 10x^2 - 4x^2 - 10x + 3x - 10 = 0 $$

$$ 6x^2 - 7x - 10 = 0 $$

$$ x = \frac{-(-7) \pm \sqrt{(-7)^2 - 4(6)(-10)}}{2(6)} $$

$$ x = \frac{7 \pm \sqrt{289}}{12} $$

$$ x = \frac{7 \pm 17}{12} $$

$$ x = \frac{7}{12} \pm \frac{17}{12} $$

$$ x = \frac{7}{12} + \frac{17}{12} $$

$$ x = \frac{24}{12} $$

$$ x = 2 $$

$$ x = \frac{7}{12} - \frac{17}{12} $$

$$ x = -\frac{10}{12} $$

$$ x = -\frac{5}{6} $$

$$ x = \left\{2, -\frac{5}{6}\right\} $$

**26.**

$$ 16z^2 + 4z - 40 = 140z + 19 $$

$$ 16z^2 + 4z - 140z - 40 - 19 = 0 $$

$$ 16z^2 - 136z - 59 = 0 $$

$$ z = \frac{-(-136) \pm \sqrt{(-136)^2 - 4(16)(-59)}}{2(16)} $$

$$ z = \frac{136 \pm \sqrt{22272}}{32} $$

$$ z = \frac{136 \pm 16\sqrt{87}}{32} $$

$$ z = \frac{17}{4} \pm \frac{\sqrt{87}}{2} $$

$$ z = \left\{\frac{17}{4} + \frac{\sqrt{87}}{2}, \frac{17}{4} - \frac{\sqrt{87}}{2}\right\} $$
