# 2.7 Quadratic Equations: A Summary

---

**How to determine which method to use when solving Quadratic Equations**

1. Is it cleary a square root property problem? In other words, does the
   equation consist ONLY of something squared and a constant. If this is true,
   then the square root property is probably the easiest method for use.

2. Does it factor? If so, that is probably the way to go. Note that you
   shouldn't spend a lot of time trying to determine if the quadratic equation
   factors. Look at the equation and if you can determine that it factors then
   go with that. If you can't quickly determine that it factors then don't worry
   about it.

3. If you've reached this point then you've determined that the equation is not
   in the correct form for the square root property and that it doesn't factor
   (or that you can't quickly see that it factors). So, at this point you're
   only real option is the quadratic formula.

---

Inspecting our quadratic formula, we find within the square root the
<b>discriminant</b> (i.e. $b^2 - 4ac$), which we can use to determine which
solution set we will get from our equation.

$$ x = \frac{-b \pm \sqrt{b^2 - 4ac}}{2a} $$

1. Two real distinct solutions. We will get this solution set if
   $b^2 - 4ac > 0$. In this case we will be taking the square root of a positive
   number and so the square root will be a real number. Therefore, the numerator
   in the quadratic formula will be $-b$ plus or minus a real number. This means
   that the numberator will be two different real numbers. Dividing either one
   by $2a$ won't change the fact that they are real, nor will it change the fact
   that they are different.

2. A double root. We will get this solution set if $b^2 - 4ac = 0$. Here we will
   be taking the square root of zero, which is zero. However, this means that
   the "plus or minus" part of the numerator will be zero and so the numerator
   in the quadratic formula will be $-b$. In other words, we will get a single
   real number out of the quadratic formula, which is what we get when we get a
   double root.

3. Two complex solutions. We will get this set if $b^2 - 4ac < 0$. If the
   discriminant is negative we will be taking the square root of negative
   numbers in the quadratic formula which means that we will get complex
   solutions. Also, we will get two since they have a "plus or minus" in front
   of the square root.

To summarize the above:

1. If $b^2 - 4ac > 0$ then we will get two real solutions to the quadratic
   equation.

2. If $b^2 - 4ac = 0$ then we will get a double root to the quadratic equation.

3. If $b^2 - 4ac < 0$ then we will get two complex solutions to the quadratic
   equation.

---

**Example 1**

Using the discriminant determine which solution set we get for each of the
following quadratic equations.

**(a)**

$$ 13x^2 + 1 = 5x $$

$$ 13x^2 - 5x + 1 = 0 $$

$$ a = 13 $$

$$ b = -5 $$

$$ c = 1 $$

$$ b^2 - 4ac $$

$$ (-5)^2 - 4(13)(1) $$

$$ 25 - 52 = -27 $$

$$ b^2 - 4ac < 0 $$

Therefore we will get <b>two complex solutions</b>.

**(b)**

$$ 6q^2 + 20q = 3 $$

$$ 6q^2 + 20q - 3 = 0 $$

$$ a = 6 $$

$$ b = 20 $$

$$ c = -3 $$

$$ b^2 - 4ac $$

$$ (20)^2 - 4(6)(-3) $$

$$ 400 + 72 = 472 $$

$$ b^2 - 4ac > 0 $$

Therefore we will get <b>two real solutions</b>

**(c\)**

$$ 49t^2 + 126t + 81 = 0 $$

$$ a = 49 $$

$$ b = 126 $$

$$ c = 81 $$

$$ b^2 - 4ac $$

$$ (126)^2 - 4(49)(81) $$

$$ 15876 - 15876 = 0 $$

$$ b^2 - 4ac = 0$$

There for we will get a <b>double root</b>.

---

## Practice Problems

For problems 1 – 4 use the discriminant to determine the type of roots for the
equation. Do not find any roots.

**1.**

$$ 169x^2 - 182x + 49 = 0 $$

$$ a = 169 $$

$$ b = -182 $$

$$ c = 49 $$

$$ b^2 - 4ac $$

$$ (-182)^2 - 4(169)(49) $$

$$ 33124 - 33124 = 0 $$

$$ b^2 - 4ac = 0 $$

Therefore we will get a <b>double root</b>.

**2.**

$$ x^2 + 28x + 61 = 0 $$

$$ a = 1 $$

$$ b = 28 $$

$$ c = 61 $$

$$ b^2 - 4ac $$

$$ (28)^2 - 4(1)(61) $$

$$ 784 - 244 = 540 $$

$$ b^2 - 4ac > 0 $$

Therefore we will get <b>two real solutions</b>.

**3.**

$$ 49x^2 - 126x + 102 = 0 $$

$$ a = 49 $$

$$ b = -126 $$

$$ c = 102 $$

$$ b^2 - 4ac $$

$$ (-126)^2 - 4(49)(102) $$

$$ 15876 - 19992 $$

$$ -4116 $$

$$ b^2 - 4ac < 0 $$

Therefore we will get <b>two complex solutions</b>.

**4.**

$$ 9x^2 + 151 = 0 $$

$$ 9x^2 + 0x + 151 = 0 $$

$$ a = 9 $$

$$ b = 0 $$

$$ c = 151 $$

$$ b^2 - 4ac $$

$$ (0)^2 - 4(9)(151) $$

$$ 0 - 5436 $$

$$ -5436 $$

$$ b^2 - 4ac < 0 $$

Therefore we will get <b>two complex solutions</b>.

---

## Assignment Problems

---

For problems 1 – 7 use the discriminant to determine the type of roots for the
equation. Do not find any roots.

**1.**

$$ 25x^2 - 120x + 619 = 0 $$

$$ a = 25 $$

$$ b = -120 $$

$$ c = 619 $$

$$ b^2 - 4ac $$

$$ (-120)^2 - 4(25)(619) $$

$$ -47500 $$

$$ b^2 - 4ac < 0 $$

Therefore we will get <b>two complex solutions</b>.

**2.**

$$ 104x^2 - 75x - 14 = 0 $$

$$ a = 104 $$

$$ b = -75 $$

$$ c = -14 $$

$$ b^2 - 4ac $$

$$ (-75)^2 - 4(104)(-14) $$

$$ 11449 $$

$$ b^2 - 4ac > 0 $$

Therefore we will get <b>two real solutions</b>.

**3.**

$$ 2x^2 + 60x + 450 = 0 $$

$$ a = 2 $$

$$ b = 60 $$

$$ c = 450 $$

$$ b^2 - 4ac $$

$$ (60)^2 - 4(2)(450) $$

$$ 0 $$

$$ b^2 - 4ac = 0 $$

Therefore we will get a <b>double root</b>.

**4.**

$$ \frac{1}{6}x^2 - 43 = 0 $$

$$ a = \frac{1}{6} $$

$$ b = 0 $$

$$ c = -43 $$

$$ b^2 - 4ac $$

$$ (0)^2 - 4\left(\frac{1}{6}\right)(-43) $$

$$ \frac{86}{3} $$

$$ b^2 - 4ac > 0 $$

Therefore we will get <b>two real solutions</b>.

**5.**

$$ 97 + 136x + 289x^2 = 0 $$

$$ 289x^2 + 136x + 97 = 0 $$

$$ a = 289 $$

$$ b = 136 $$

$$ c = 97 $$

$$ b^2 - 4ac $$

$$ (136)^2 - 4(289)(97) $$

$$ -93636 $$

$$ b^2 - 4ac < 0 $$

Therefore we will get <b>two complex solutions</b>.

**6.**

$$ 10x^2 - 7x = 0 $$

$$ a = 10 $$

$$ b = -7 $$

$$ c = 0 $$

$$ b^2 - 4ac $$

$$ (-7)^2 - 4(10)(0) $$

$$ 49 $$

$$ b^2 - 4ac > 0 $$

Therefore we will get <b>two real solutions</b>.

**7.**

$$ \frac{49}{9}x^2 + \frac{14}{15}x + \frac{1}{25} = 0 $$

$$ a = \frac{49}{9} $$

$$ b = \frac{14}{15} $$

$$ c = \frac{1}{25} $$

$$ b^2 - 4ac $$

$$ \left(\frac{14}{15}\right)^2 - 4\left(\frac{49}{9}\right)\left(\frac{1}{25}\right) $$

$$ 0 $$

$$ b^2 - 4ac = 0 $$

Therefore we will get a <b>double root</b>.
