# 2.9 Equations Reducible to Quadratic in Form

---

**Example 1**

Solve $x^4 - 7x^2 + 12 = 0$

$$ x^4 = (x^2)^2 $$

$$ u = x^2 $$

$$ u^2 = (x^2)^2 $$

$$ x^2 - 7x^2 + 12 = 0 \Rightarrow u^2 - 7u + 12 = 0 $$

$$ u^2 - 7u - 12 = 0 = (u - 4)(u - 3) = 0 \Rightarrow u = \{3, 4\} $$

$$ u = x^2 $$

$$ u = 3\text{ : } 3 = x^2 \Rightarrow x = \pm \sqrt{3} $$

$$ u = 4\text{ : } 4 = x^2 \Rightarrow x = \pm \sqrt{4} = \pm 2 $$

$$ x = \{2, -2, \sqrt{3}, -\sqrt{3}\} $$

---

**Example 2**

Solve each of the following equations.

**(a)**

$$ x^{\frac{2}{3}} - 2x^{\frac{1}{3}} - 15 = 0 $$

$$ u = x^{\frac{1}{3}} $$

$$ u^2 = (x^{\frac{1}{3}})^2 = x^{\frac{2}{3}} $$

$$ u^2 - 2u - 15 = 0 $$

$$ (u + 3)(u - 5) = 0 $$

$$ u = \{-3, 5\} $$

$$ u = -3\text{ : } x^{\frac{1}{3}} = -3 \Rightarrow x = (-3)^3 = -27 $$

$$ u = 5\text{ : } x^{\frac{1}{3}} = 5 \Rightarrow x = (5)^3 = 125 $$

$$ x = \{-27, 125\} $$

**(b)**

$$ y^{-6} - 9y^{-3} + 8 = 0 $$

$$ u = y^{-3} $$

$$ u^2 = (y^{-3})^2 = y^{-6} $$

$$ u^2 - 9u + 8 = 0 $$

$$ (u - 8)(u - 1) = 0 $$

$$ u = \{8, 1\} $$

$$ u = 8\text{ : } y^{-3} = 8 \Rightarrow \frac{1}{y^3} = 8 \Rightarrow 1 = 8y^3
\Rightarrow \frac{1}{8} = y^3 = \sqrt[3]{\frac{1}{8}} = y \Rightarrow \frac{1}{2} = y $$

$$ u = 1\text{ : } y^{-3} = 1 \Rightarrow \frac{1}{y^3} = 1 \Rightarrow 1 = y^3
\Rightarrow 1 = 1$$

$$ y = \left\{\frac{1}{2}, 1\right\} $$

**(c\)**

$$ z - 9\sqrt{z} + 14 = 0 $$

$$ u = \sqrt{z} $$

$$ u^2 = (\sqrt{z})^2 = z $$

$$ u^2 - 9u + 14 = 0 $$

$$ (u - 2)(u - 7) = 0 $$

$$ u = \{2, 7\} $$

$$ u = 2\text{ : } \sqrt{z} = 2 \Rightarrow (\sqrt{z})^2 = 2^2 \Rightarrow z = 4 $$

$$ u = 7\text{ : } \sqrt{z} = 7 \Rightarrow (\sqrt{z})^2 = 7^2 \Rightarrow z =
49 $$

$$ z = \{4, 49\} $$

**(d)**

$$ t^4 - 4 = 0 $$

$$ u = t^2 $$

$$ u^2 = (t^2)^2 = t^4 $$

$$ u^2 - 4 = 0 $$

$$ (u + 2)(u - 2) = 0 $$

$$ u = \{-2, 2\} $$

$$ u = -2\text{ : } t^2 = -2 \Rightarrow \sqrt{t^2} = \pm \sqrt{-2} \Rightarrow
t = \pm \sqrt{2}i $$

$$ u = 2\text{ : } t^2 = -2 \Rightarrow \sqrt{t^2} = \pm \sqrt{2} $$

$$ u = \{\sqrt{2}i, -\sqrt{2}i, \sqrt{2}, -\sqrt{2}\} $$

---

**Example 3**

Solve $2x^{10} - x^5 - 4 = 0$.

$$ 2x^{10} - x^5 - 4 = 0 $$

$$ u = x^5 $$

$$ u^2 = (x^5)^2 = x^{10} $$

$$ 2u^2 - u - 4 = 0 $$

$$ u = \frac{-(-1) \pm \sqrt{(-1)^2 - 4(2)(-4)}}{2(2)} $$

$$ u = \frac{1 \pm \sqrt{33}}{4} $$

$$ u = \frac{1}{4} \pm \frac{\sqrt{33}}{4} $$

$$ u = \frac{1}{4} + \frac{\sqrt{33}}{4}\text{ : } x^5 = \frac{1}{4} + \frac{\sqrt{33}}{4} \Rightarrow \sqrt[5]{x^5} = \sqrt[5]{\frac{1}{4} + \frac{\sqrt{33}}{4}} \Rightarrow x = 1.1101 $$

$$ u = \frac{1}{4} - \frac{\sqrt{33}}{4}\text{ : } x^5 = \frac{1}{4} - \frac{\sqrt{33}}{4} \Rightarrow \sqrt[5]{x^5} = \sqrt[5]{\frac{1}{4} - \frac{\sqrt{33}}{4}} \Rightarrow x = -1.0347 $$

$$ x = \{1.1101, -1.0347\} $$

---

## Practice Problems

**1.**

$$ x^6 - 9x^3 + 8 = 0 $$

$$ u = x^3 $$

$$ u^2 = (x^3)^2 = x^6 $$

$$ u^2 - 9u + 8 = 0 $$

$$ (u - 1)(u - 8) = 0 $$

$$ u = \{1, 8\} $$

$$ u = 1\text{ : } x^3 = 1 \Rightarrow \sqrt[3]{x^3} = \sqrt[3]{1} \Rightarrow x = 1 $$

$$ u = 8\text{ : } x^3 = 8 \Rightarrow \sqrt[3]{x^3} = \sqrt[3]{8} \Rightarrow x = 2 $$

$$ x = \{1, 2\} $$

**2.**

$$ x^{-4} - 7x^{-2} - 18 = 0 $$

$$ u = x^{-2} $$

$$ u^2 = (x^{-2})^2 = x^{-4} $$

$$ u^2 - 7u - 18 = 0 $$

$$ (u - 9)(u + 2) = 0 $$

$$ u = \{9, -2\} $$

$$ u = 9\text{ : } x^{-2} = \frac{1}{x^2} = 9 \Rightarrow x^2 = -\frac{1}{2} \Rightarrow x = \pm \sqrt{-\frac{1}{2}} = \pm \frac{1}{2}i $$

$$ u = -2\text{ : } x^{-2} = \frac{1}{x^2} = -2 \Rightarrow x^2 = \frac{1}{9} \Rightarrow x = \pm \sqrt{\frac{1}{9}} = \pm \frac{1}{3} $$

$$ u = \left\{\frac{1}{2}i, -\frac{1}{2}i, \frac{1}{3}, -\frac{1}{3}\right\} $$

**3.**

$$ 4x^{\frac{2}{3}} + 21x^{\frac{1}{3}} + 27 = 0 $$

$$ u = x^{\frac{1}{3}} $$

$$ u^2 = (x^{\frac{1}{3}})^2 = x^{\frac{2}{3}} $$

$$ 4u^2 + 21u + 27 = 0 $$

$$ (4u + 9)(u + 3) = 0 $$

$$ 4u + 9 = 0 $$

$$ 4u = -9 $$

$$ u = -\frac{9}{4} $$

$$ u + 3 = 0 $$

$$ u = -3 $$

$$ u = \left\{-\frac{9}{4}, -3\right\} $$

$$ u = -\frac{9}{4}\text{ : } x^{\frac{1}{3}} = -\frac{9}{4} \Rightarrow x = (-\frac{9}{4})^3 \Rightarrow x = -\frac{729}{64} $$

$$ u = -3\text{ : } x^{\frac{1}{3}} = -3 \Rightarrow x = (-3)^3 \Rightarrow x = -27 $$

$$ x = \left\{-\frac{729}{64}, -27\right\} $$

**4.**

$$ x^8 - 6x^4 + 7 = 0 $$

$$ u = x^4 $$

$$ u^2 = (x^4)^2 = x^8 $$

$$ u^2 - 6u + 7 = 0 $$

$$ u = \frac{-(-6) \pm \sqrt{(-6)^2 - 4(1)(7)}}{2(1)} $$

$$ u = \frac{6 \pm 2\sqrt{2}}{2} $$

$$ u = 3 \pm \sqrt{2} $$

$$ u = \{3 + \sqrt{2}, 3 - \sqrt{2}\} $$

$$ u = 3 + \sqrt{2}\text{ : } x^4 = 3 + \sqrt{2} \Rightarrow x = (3 + \sqrt{2})^{\frac{1}{4}} = (4.4142)^{\frac{1}{4}} = 1.4495 $$

$$ u = 3 - \sqrt{2}\text{ : } x^3 = 3 - \sqrt{2} \Rightarrow x = (3 - \sqrt{2})^{\frac{1}{4}} = (1.5858)^{\frac{1}{4}} =  1.1222 $$

$$ u = \{1.4495, 1.1222\} $$

**5.**

$$ \frac{2}{x^2} + \frac{17}{x} + 21 = 0 $$

$$ u = \frac{1}{x} $$

$$ u^2 = \left(\frac{1}{x}\right)^2 = \frac{1^2}{x^2} = \frac{1}{x^2} $$

$$ 2u^2 + 17u + 21 = 0 $$

$$ (2u + 3)(u + 7) = 0 $$

$$ 2u + 3 = 0 $$

$$ 2u = -3 $$

$$ u = -\frac{3}{2} $$

$$ u + 7 = 0 $$

$$ u = -7 $$

$$ u = \left\{-\frac{3}{2}, -7\right\} $$

$$ u = -\frac{3}{2}\text{ : } \frac{1}{x} = -\frac{3}{2} \Rightarrow 1 = -\frac{3}{2}x \Rightarrow -\frac{2}{3} = x $$

$$ u = -7\text{ : } \frac{1}{x} = -7 \Rightarrow 1 = -7x \Rightarrow -\frac{1}{7} = x $$

$$ x = \left\{-\frac{2}{3},-\frac{1}{7}\right\} $$

**6.**

$$ \frac{1}{x} - \frac{11}{\sqrt{x}} + 18 = 0 $$

$$ u = \frac{1}{\sqrt{x}} $$

$$ u^2 = \left(\frac{1}{\sqrt{x}}\right)^2 = \frac{1^2}{(\sqrt{x})^2} = \frac{1}{x} $$

$$ u^2 - 11u + 18 = 0 $$

$$ (u - 9)(u - 2) = 0 $$

$$ u = \{9, 2\} $$

$$ u = 9\text{ : } \frac{1}{\sqrt{x}} = 9 \Rightarrow 1 = 9\sqrt{x} \Rightarrow \frac{1}{9} = \sqrt{x} = \left(\frac{1}{9}\right)^2 = x \Rightarrow \frac{1}{81} = x $$

$$ u = 2\text{ : } \frac{1}{\sqrt{x}} = 2 \Rightarrow 1 = 2\sqrt{x} \Rightarrow \frac{1}{2} = \sqrt{x} \Rightarrow \left(\frac{1}{2}\right)^2 = x \Rightarrow \frac{1}{4} = x$$

$$ x = \left\{\frac{1}{81}, \frac{1}{4}\right\} $$

---

## Assignment Problems

Solve each of the following equations.

**1.**

$$ 8x^6 + 215x^3 - 27 = 0 $$

$$ u = x^3 $$

$$ u^2 = (x^3)^2 $$

$$ 8u^2 + 215u - 27 = 0 $$

$$ u = \frac{-(215) \pm \sqrt{(215)^2 - 4(8)(-27)}}{2(8)} $$

$$ u = \frac{-215 \pm 217}{16} $$

$$ u = \frac{-215 + 217}{16} = \frac{1}{8} $$

$$ u = \frac{-215 - 217}{16} = -27 $$

$$ u = \left\{\frac{1}{8}, -27\right\} $$

$$ u = \frac{1}{8}\text{ : } x^3 = \frac{1}{8} \Rightarrow \sqrt[3]{x^3} = \sqrt[3]{\frac{1}{8}} \Rightarrow x = \frac{1}{2} $$

$$ u = -27\text{ : } x^3 = -27 \Rightarrow \sqrt[3]{x^3} = \sqrt[3]{-27}
\Rightarrow x = -3 $$

$$ x = \left\{\frac{1}{2}, -3\right\} $$

**2.**

$$ x^{\frac{4}{3}} - 13x^{\frac{2}{3}} + 36 = 0 $$

$$ u = x^{\frac{2}{3}} $$

$$ u^2 = (x^\frac{2}{3})^2 = x^{\frac{4}{3}} $$

$$ u^2 - 13u + 36 = 0 $$

$$ (u - 9)(u - 4) = 0 $$

$$ u = \{9, 4\} $$

$$ u = 9\text{ : } x^{\frac{2}{3}} = 9 \Rightarrow x = (\sqrt{9})^3 \Rightarrow x = (3)^3 \Rightarrow x = 27 $$

$$ u = 4\text{ : } x^{\frac{2}{3}} = 4 \Rightarrow x = (2)^3 \Rightarrow x = (\sqrt{4})^3 = 8 $$

$$ x = \{27, 8\} $$

**3.**

$$ 32x^{-10} - 31x^{-5} - 1 = 0 $$

$$ u = x^{-5} $$

$$ u^2 = (x^{-5})^2 = x^{-10} $$

$$ 32u^2 - 31u - 1 = 0 $$

$$ (32u + 1)(u - 1) = 0 $$

$$ 32u + 1 = 0 $$

$$ 32u = -1 $$

$$ u = -\frac{1}{32} $$

$$ u - 1 = 0 $$

$$ u = 1 $$

$$ u = \left\{-\frac{1}{32}, 1\right\} $$

$$ u = -\frac{1}{32}\text{ : } x^{-5} = -\frac{1}{32} \Rightarrow \frac{1}{x^5} = -\frac{1}{32} \Rightarrow -32x^5 = 1 \Rightarrow x^5 = -\frac{1}{32} \Rightarrow x = \sqrt[5]{-\frac{1}{32}} \Rightarrow x = -2$$

$$ u = 1\text{ : } x^{-5} = 1 \Rightarrow \frac{1}{x^5} = 1 \Rightarrow x^5 = 1 \Rightarrow \sqrt[5]{x^5} = \sqrt[5]{1} \Rightarrow x = 1 $$

$$ x = \{-2, 1\} $$

**4.**

$$ x - 8\sqrt{x} + 15 = 0 $$

$$ u = \sqrt{x} $$

$$ u^2 = (\sqrt{x})^2 = x $$

$$ u^2 - 8u + 15 = 0 $$

$$ (u - 3)(u - 5) = 0 $$

$$ u = \{3, 5\} $$

$$ u = 3\text{ : } \sqrt{x} = 3 \Rightarrow (\sqrt{x})^2 = (3)^2 \Rightarrow x =
9$$

$$ u = 5\text{ : } \sqrt{x} = 5 \Rightarrow (\sqrt{x})^2 = (5)^2 \Rightarrow x =
25$$

$$ x = \{9, 25\} $$

**5.**

$$ x^{-\frac{1}{2}} - 13x^{-\frac{1}{4}} + 30 = 0 $$

$$ u = x^{-\frac{1}{4}} $$

$$ u^2 = (x^{-\frac{1}{4}})^2 = x^{-\frac{1}{2}} $$

$$ u^2 - 13u + 30 = 0 $$

$$ (u - 3)(u - 10) = 0 $$

$$ u = \{3, 10\} $$

$$ u = 3 \text{ : } x^{-\frac{1}{4}} = 3 \Rightarrow x^{\frac{1}{4}} = \frac{1}{3} \Rightarrow x = \left(\frac{1}{3}\right)^4 = \frac{1}{81} $$

$$ u = 10 \text{ : } x^{-\frac{1}{4}} = 10 \Rightarrow x^{\frac{1}{4}} = \frac{1}{10} \Rightarrow x = \left(\frac{1}{10}\right)^4 = \frac{1}{10000}$$

$$ x = \left\{\frac{1}{81}, \frac{1}{10000}\right\}$$

**6.**

$$ x^{-6} - 3x^{-3} - 28 = 0 $$

$$ u = x^{-3} $$

$$ u^2 = (x^{-3})^2 = x^{-6} $$

$$ u^2 - 3u - 28 = 0 $$

$$ (u - 7)(u + 4) = 0 $$

$$ u = \{7, -4\} $$

$$ u = 7\text{ : } x^{-3} = 7 \Rightarrow x^3 = \frac{1}{7} \Rightarrow x = \left(\frac{1}{7}\right)^{\frac{1}{3}} = \frac{1}{\sqrt[3]{7}} $$

$$ u = -4\text{ : } x^{-3} = -4 \Rightarrow x^3 = -\frac{1}{4} \Rightarrow x = \left(-\frac{1}{4}\right)^{\frac{1}{3}} = -\frac{1}{\sqrt[3]{4}} $$

$$ x = \left\{\frac{1}{\sqrt[3]{7}}, -\frac{1}{\sqrt[3]{4}}\right\} $$

**7.**

$$ x^{10} - 1024 = 0 $$

$$ u = x^5 $$

$$ u^2 = (x^5)^2 = x^{10} $$

$$ u^2 - 1024 = 0 $$

$$ (u - 32)(u + 32) = 0 $$

$$ u = \{32, -32\} $$

$$ u = 32 \text{ : } x^5 = 32 \Rightarrow x = \sqrt[5]{32} \Rightarrow x = 2 $$

$$ u = -32 \text{ : } x^5 = -32 \Rightarrow x = \sqrt[5]{-32} \Rightarrow x = -2 $$

$$ x = \{2, -2\} $$

**8.**

$$ x^4 - 8x^2 + 5 = 0 $$

$$ u = x^2 $$

$$ u^2 = (x^2)^2 = x^4 $$

$$ u^2 - 8u + 5 = 0 $$

$$ u = \frac{-(-8) \pm \sqrt{(-8)^2 - 4(1)(5)}}{2(1)} $$

$$ u = \frac{8 \pm 2\sqrt{11}}{2} $$

$$ u = 4 \pm \sqrt{11} $$

$$ u = 4 + \sqrt{11}\text{ : } x^2 = 4 + \sqrt{11} \Rightarrow x = (2 + \sqrt{11})^{\frac{1}{2}} $$

$$ u = 4 - \sqrt{11}\text{ : } x^2 = 4 - \sqrt{11} \Rightarrow x = (2 - \sqrt{11})^{\frac{1}{2}} $$

$$ x = \left\{(2 + \sqrt{11})^{\frac{1}{2}}, (2 - \sqrt{11})^{\frac{1}{2}}\right\} $$

**9.**

$$ \frac{1}{x^4} + \frac{10}{x^2} + 22 = 0 $$

$$ u = \frac{1}{x^2} $$

$$ u^2 = \left(\frac{1}{x^2}\right)^2 = \frac{1}{x^4} $$

$$ u^2 + 10u + 22 = 0 $$

$$ u = \frac{-(10) \pm \sqrt{(10)^2 - 4(1)(22)}}{2(1)} $$

$$ u = \frac{-10 \pm 2\sqrt{3}}{2} $$

$$ u = -5 \pm \sqrt{3} $$

$$ u = -5 + \sqrt{3} \text{ : } \frac{1}{x^2} = -5 + \sqrt{3} \Rightarrow x^2 = \frac{1}{-5 + \sqrt{3}} \Rightarrow x = \frac{1}{(-5 + \sqrt{3})^{\frac{1}{2}}} $$

$$ u = -5 - \sqrt{3} \text{ : } \frac{1}{x^2} = -5 - \sqrt{3} \Rightarrow x^2 = \frac{1}{-5 - \sqrt{3}} \Rightarrow x = \frac{1}{(-5 - \sqrt{3})^{\frac{1}{2}}} $$

$$ x = \left\{\frac{1}{(-5 + \sqrt{3})^{\frac{1}{2}}}, \frac{1}{(-5 - \sqrt{3})^{\frac{1}{2}}} \right\} $$
