# Section 1.10 : Common Graphs

The purpose of this section is to make sure that you’re familiar with the graphs
of many of the basic functions that you’re liable to run across in a calculus
class.

---

**Example 1** Graph $y = -\dfrac{2}{5}x + 3$.

This is a line in the slope intercept form

$$ y = mx + b $$

In this case the line has a $y$ intercept of $(0, b)$ and a slope of $m$. Recall
that slope can be thought of as

$$ m = \frac{\text{rise}}{\text{run}} $$

Note that if the slope is negative we tend to think of the rise as a fall.

The slope allows us to get a second point on the line. Once we have any point on
the line and the slope we move right by run and up/down by rise depending on the
sign. This will be a second point on the line.

In this case we know $(0, 3)$ is a point on the line and the slope is
$-\dfrac{2}{5}$. So starting at $(0, 3)$ we'll move $5$ to the right (_i.e._
$0 \rightarrow 5$) and down $2$ (_i.e._ $3 \rightarrow 1$) to get $(5, 1)$ as a
second point on the line. Once we've got two points on a line all we need to do
is plot the two points and connect them with a line.

Here's the sketch for this line.

![image 1.10_1](./1.10_1.png)

---

**Example 2** Graph $f(x) = \mid x \mid$

There really isn’t much to this problem outside of reminding ourselves of what
absolute value is. Recall that the absolute value function is defined as,

$$  $$

$$
\mid x \mid =
\begin{cases}
x \text{ if } x \geq 0 \\
-x \text{ if } x < 0
\end{cases}
$$

The graph is then,

![image 1.10_2](./1.10_2.png)

---

**Example 3** Graph $f(x) = -x^2 + 2x + 3$.

This is a parabola in the general form.

$$ f(x) = ax^2 + bx + c $$

In this form, the $x$-coordinate of the vertex (the highest or lowest point on
the parabola) is $x = -\dfrac{b}{2a}$ and the $y$-coordinate is
$y = f\left(-\dfrac{b}{2a}\right)$. So, for our parabola the coordinates of the
vertex will be.

$$ x = -\frac{2}{2(-1)} = 1 $$

$$ y = f(1) = -(1)^2 + 2(1) + 3 = 4 $$

So, the vertex for this parabola is $(1, 4)$.

We can also determine which direction the parabola opens from the sign of $a$.
If $a$ is positive the parabola opens up and if $a$ is negative the parabola
opens down. In our case the parabola opens down.

Now, because the vertex is above the $x$-axis and the parabola opens down we
know that we'll have $x$-intercepts (_i.e._ values of $x$ for which we'll have
$f(x) = 0$) on this graph. So, we'll solve the following.

$$ -x^2 + 2x + 3 = 0 $$

$$ x^2 - 2x - 3 = 0 $$

$$ (x - 3)(x + 1) = 0 $$

So, we will have $x$-intercepts at $x = -1$ and $x = 3$. Notice that to make our
life easier in the solution process we multiplied everything by $-1$ to get the
coefficient of the $x^2$ positive. This made the factoring easier.

Here's a sketch of this parabola.

![image 1.10_3](./1.10_3.png)

---

**Example 4** Graph $f(y) = y^2 - 6yn + 5$.

Most people come out of an Algebra class capable of dealing with functions in
the form $y = f(x)$. However, many functions that you will have to deal with in
a Calculus class are in the form $x = f(y)$ and can only be easily worked with
in that form. So, you need to get used to working with functions in this form.

The nice thing about these kinds of function is that if you can deal with
functions in the form $y = f(x)$ then you can deal with functions in the form
$x = f(y)$ even if you aren't that familiar with them.

Let's first consider the equation.

$$ y = x^2 - 6x + 5 $$

This is a parabola that opens up and has a vertex of $(3, -4)$, as we know from
our work in the previous example.

For our function we have essentially the same equation except the $x$ and $y$'s
are switched around. In other words, we have a parabola in the form,

$$ x = ay^2 + by + c $$

This is the general form of this kind of parabola and this will be a parabola
that opens left or right depending on the sign of $a$. The $y$-coordinate of the
vertex is given by $y = -\dfrac{b}{2a}$ and we find the $x$-coordinate by
plugging this into the equation. So, you can see that this is very similar to
the type of parabola that you're already used to dealing with.

Now, let's get back to the example. Our functdion is a parabola that opens to
the right ($a$ is positive) and has a vertex at $(-4, 3)$. The vertex is to the
left of the $y$-axis and opens to the right so we'll need the $y$-intercepts
(_i.e._ values of $y$ for which we'll have $f(y) = 0$). We find these just like
we found $x$-intercepts in the previous problem.

$$ y^2 - 6y + 5 = 0 $$

$$ (y - 5)(y - 1) = 0 $$

So, our parabola will have $y$-intercepts at $y = 1$ and $y = 5$. Here's a
sketch of the graph.

![image 1.10_4](./1.10_4.png)

---

**Example 5** Graph $x^2 + 2x + y^2 - 8y + 8 = 0$.

To determine just what kind of graph we’ve got here we need to complete the
square on both the $x$ and the $y$.

$$ x^2 + 2x + y^2 - 8y + 8 = 0 $$

$$ x^2 + 2x + 1 - 1 + y^2 - 8y + 16 - 16 + 8 = 0 $$

$$ (x + 1)^2 + (y - 4)^2 = 9 $$

Recall that to complete the square we take the half of the coefficient of the
$x$ (or the $y$), square this and then add and subtract it to the equation.

Upon doing this we see that we have a circle and it’s now written in standard
form.

$$ (x - h)^2 + (y - k)^2 = r^2 $$

When circles are in this form we can easily identify the center $(h, k)$ and
radius $r$. Once we have these we can graph the circle simply by starting at the
center and moving right, left, up and down by $r$ to get the rightmost,
leftmost, top most and bottom most points respectively.

Our circle has a center at $(-1, 4)$ and a radius of $3$. Here's a sketch of
this circle.

![image 1.10_5](./1.10_5.png)

---

**Example 6** Graph $\dfrac{(x - 2)^2}{9} + 4(y + 2)^2 = 1$.

This is an ellipse. The standard form of the ellipse is

$$ \frac{(x - h)^2}{a^2} + \frac{(y - k)^2}{b^2} = 1 $$

This is an ellipse with center $(h, k)$ and the right most and left most points
are a distance of $a$ from the center and the top most and bottom most points
are a distance of $b$ away from the center.

The ellipse for this problem has center $(2, -2)$ and has $a = 3$ and $b =
\dfrac{1}{2}$. Note that to get the $b$ we're really rewriting the equation as,

$$ \frac{(x - 2)^2}{9} + \frac{(y + 2)^2}{\dfrac{1}{4}} = 1 $$

to get it into standard form.

Here's a sketch of the ellipse.

![image 1.10_6](./1.10_6.png)

---

**Example 7** Graph $\dfrac{(x + 1)^2}{9} - \dfrac{(y - 2)^2}{4} = 1$.

This is a hyperbola. There are actually two standard forms for a hyperbola. Here
are the basics for each form.

$$ \text{Form} \quad \quad \quad \frac{(x - h)^2}{a^2} - \frac{(y - k)^2}{b^2} = 1 \quad \quad \quad \frac{(y - k)^2}{b^2} - \frac{(x - h)^2}{a^2} = 1 $$

$$ \text{Center} \quad \quad \quad (h, k) \quad \quad \quad (h, k) $$

$$ \text{Opens} \quad \quad \quad \text{Opens right and left} \quad \quad \quad \text{Opens up and down} $$

$$ \text{Vertices} \quad \quad \quad a \text{ units right and left of center} \quad \quad \quad b \text{ units up and down from center} $$

$$ \text{Slope of Asymptotes} \quad \quad \quad \pm \frac{b}{a} \quad \quad \quad \pm \frac{b}{a} $$

So, what does all this mean? First, notice that one of the terms is positive and
the other is negative. This will determine which direction the two parts of the
hyperbola open. If the $x$ term is positive the hyperbola opens left and right.
Likewise, if the $y$ term is positive the hyperbola opens up and down.

The asymptotes of a hyperbola are two lines that intersect at the center and
have the slopes listed above. As you move farther out from the center the graph
will get closer and closer to the asymptotes.

For the equation listed here the hyperbola will open left and right. Its center
is $(-1, 2)$. The two vertices are $(-4, 2)$ and $(2, 2)$. The asymptotes will
have slopes $\pm \dfrac{2}{3}$.

Here is a sketch of this hyperbola. Note that the asymptotes are denoted by the
two dashed lines.

![image 1.10_7](./1.10_7.png)

---

**Example 8** Graph $f(x) = \mathbf{e}^x$ and $g(x) = \mathbf{e}^{-x}$.

There really isn’t a lot to this problem other than making sure that both of
these exponentials are graphed somewhere.

These will both show up with some regularity in later sections and their
behavior as $x$ goes to both plus and minus infinity will be needed and from
this graph we can clearly see this behavior.

![image 1.10_8](./1.10_8.png)

---

**Example 9** Graph $f(x) = \ln(x)$.

This has already been graphed once in this review, but this puts it here with
all the other “important” graphs.

![image 1.10_9](./1.10_9.png)

---

**Example 10** Graph $y = \sqrt{x}$.

This one is fairly simple, we just need to make sure that we can graph it when
need be.

![image 1.10_10](./1.10_10.png)

Remember that the domain of the square root function is $x \geq 0$.

---

**Example 11** Grpah $y = x^3$.

Again, there really isn’t much to this other than to make sure it’s been graphed
somewhere so we can say we’ve done it.

![image 1.10_11](./1.10_11.png)

---

**Example 12** Graph $y = \cos(x)$.

There really isn't a whole lot to this one. Here's the graph for
$-4\pi \leq x \leq 4\pi$.

![image 1.10_12](./1.10_12.png)

Let’s also note here that we can put all values of $x$ into cosine (which won’t
be the case for most of the trig functions) and so the domain is all real
numbers. Also note that

$$ -1 \leq \cos(x) \leq 1 $$

It is important to notice that cosine will never be larger than $1$ or smaller
than $-1$. This will be useful on occasion in a calculus class. In general we
can say that

$$ -R \leq R\cos(\omega x) \leq R $$

---

**Example 13** Graph $y = \sin(x)$.

As with the previous problem there really isn’t a lot to do other than graph it.
Here is the graph for $-4\pi \leq x \leq 4\pi$.

![image 1.10_13](./1.10_13.png)

From this graph we can see that sine has the same range that cosine does. In
general

$$ -R \leq R\sin(\omega x) \leq R $$

As with cosine, sine itself will never be larger than $1$ and never smaller than
$-1$. Also the domain of sine is all real numbers.

---

**Example 14** Graph $y = \tan(x)$.

In the case of tangent we have to be careful when plugging $x$'s in since
tangent doesn't exist wherever cosine is zero (remember that
$\tan x = \dfrac{\sin x}{\cos x}$). Tangent will not exist at

$$ x = \dots, -\frac{5\pi}{2}, -\frac{3\pi}{2}, -\frac{\pi}{2}, \frac{\pi}{2}, \frac{3\pi}{2}, \frac{5\pi}{2}, \dots $$

and the graph will have asymptotes at these points. Here is the graph of tangent
on the range $-\dfrac{5\pi}{2} < x < \dfrac{5\pi}{2$a.}$

![image 1.10_14](./1.10_14.png)

---

**Example 15** Graph $y = \sec(x)$.

As with tangent we will have to avoid $x$'s for which cosine is zero (remember
that $\sec x = \dfrac{1}{\cos x}$). Secant will not exist at

$$ x = \dots, -\frac{5\pi}{2}, -\frac{3\pi}{2}, -\frac{\pi}{2}, \frac{\pi}{2}, \frac{3\pi}{2}, \frac{5\pi}{2}, \dots $$

and the graph will have asymptotes at these points. Here is the graph of secant
on the range $-\dfrac{5\pi}{2} < x < \dfrac{5\pi}{2}$.

![image 1.10_15](./1.10_15.png)

Notice that the graph is always greater than $1$ or less than $-1$. This should
not be terribly surprising. Recall that

$$ -1 \leq \cos(x) \leq 1 $$

So, one divided by something less than one will be greater than $1$. Also
$\dfrac{1}{\pm 1} = \pm 1$ and so we get the following ranges for secant.

$$ \sec(\omega x) \geq 1 \quad \text{ and } \quad \sec(\omega x) \leq -1 $$

---

Note that we did not graph cotangent or cosecant here. However, they are similar
to the graphs of tangent and secant and you should be able to do quick sketches
of them given the work above if needed.

Finally, note that we did not cover any of the basic transformations that are
often used in graphing functions here. The practice problems for this section
have quite a few problems designed to help you remember them. If you know the
basic transformations it often makes graphing a much simpler process so if you
are not comfortable with them you should work through the practice problems for
this section.

---

## Practice Problems

Without using a graphing calculator sketch the graph of each of the following.

**1.** $y = \dfrac{4}{3}x - 2$

**Solution**

**2.** $f(x) = \mid x - 3 \mid$

**Solution**

**3.** $g(x) = \sin(x) + 6$

**Solution**

**4.** $f(x) = \ln(x) - 5$

**Solution**

**5.** $h(x) = \cos\left(x + \dfrac{\pi}{2}\right)$

**Solution**

**6.** $h(x) = (x - 3)^2 + 4$

**Solution**

**7.** $W(x) = \mathbf{e}^{x + 2} - 3$

**Solution**

**8.** $f(y) = (y - 1)^2 + 2$

**Solution**

**9.** $R(x) = -\sqrt{x}$

**Solution**

**10.** $g(x) = \sqrt{-x}$

**Solution**

**11.** $h(x) = 2x^2 - 3x + 4$

**Solution**

**12.** $f(y) = -4y^2 + 8yn + 3$

**Solution**

**13.** $(x + 1)^2 + (y - 5)^2 = 9$

**Solution**

**14.** $x^2 - 4x + y^2 - 6y - 87 = 0$

**Solution**

**15.** $25(x + 2)^2 + \dfrac{y^2}{4} = 1$

**Solution**

**16.** $x^2 + \dfrac{(y - 6)^2}{9} = 1$

**Solution**

**17.** $\dfrac{x^2}{36} - \dfrac{y^2}{49} = 1$

**Solution**

**18.** $(y + 2)^2 - \dfrac{(x + 4)^2}{16} = 1$

**Solution**

---

## Assignment Problems

Without using a graphing calculator sketch the graph of each of the following.

**1.** $y = -2x + 7$

**Solution**

**2.** $f(x) = \mid x + 4 \mid$

**Solution**

**3.** $g(x) = \sqrt{x} - 5$

**Solution**

**4.** $g(x) = \tan\left(x + \dfrac{\pi}{3}\right)$

**Solution**

**5.** $f(x) = \sec(x) + 2$

**Solution**

**6.** $h(x) = \mid x + 2 \mid - 4$

**Solution**

**7.** $Q(x) = \mathbf{e}^{-x - 3} + 6$

**Solution**

**8.** $V(x) = \sqrt{x - 6} + 3$

**Solution**

**9.** $g(x) = \sin\left(x + \dfrac{\pi}{6}\right) - 1$

**Solution**

**10.** $h(x) = (x + 6)^2 - 8$

**Solution**

**11.** $W(y) = (y + 5)^2 + 3$

**Solution**

**12.** $f(y) = (y - 9)^2 - 2$

**Solution**

**13.** $f(x) = (x - 1)^2 + 6$

**Solution**

**14.** $R(x) = -\ln(x)$

**Solution**

**15.** $g(x) = \ln(-x)$

**Solution**

**16.** $h(x) = x^2 + 8x - 1$

**Solution**

**17.** $Y(x) = -3x^2 - 6x + 5$

**Solution**

**18.** $f(y) = -y^2 - 4y - 2$

**Solution**

**19.** $h(y) = 2y^2 + 2y - 3$

**Solution**

**20.** $x^2 - 6x + y^2 + 8y + 24 = 0$

**Solution**

**21.** $x^2 + y^2 + 10y = -9$

**Solution**

**22.** $\dfrac{(x + 4)^2}{25} + \dfrac{(y + 2)^2}{25} = 1$

**Solution**

**23.** $x^2 - 2x + 4y^2 - 16y + 16 = 0$

**Solution**

**24.** $\dfrac{(x + 6)^2}{4} + 16(y - 5)^2 = 1$

**Solution**

**25.** $\dfrac{(y - 1)^2}{25} - \dfrac{(x - 3)^2}{4} = 1$

**Solution**

**26.** $(x - 4)^2 - 9(y + 7)^2 = 1$

**Solution**
