# Section 1.6 : Solving Trig Equations With Calculators, Part II

Because this document is also being prepared for viewing on the web we split
this section into two parts to keep the size of the pages to a minimum.

Also, as with the last few examples in the previous part of this section we are
not going to be looking for solutions in an interval in order to save space. The
important part of these examples is to find the solutions to the equation. If
we’d been given an interval it would be easy enough to find the solutions that
actually fall in the interval.

In all the examples in the previous section all the arguments, the $3t$ ,
$\dfrac{\alpha}{7}$, etc., were fairly simple. Let’s take a look at an example
that has a slightly more complicated looking argument.

---

**Example 1** Solve $5\cos(2x - 1) = -3$.

**Solution**

Note that the argument here is not really all that complicated but the addition
of the "$-1$" often seems to confuse people so we need to a quick example with
this kind of argument. The solution process is identical to all the problems
we’ve done to this point so we won’t be putting in much explanation. Here is the
solution.

$$ \cos(2x - 1) = -\frac{3}{5} \quad \Rightarrow \quad 2x - 1 = \cos^{-1}\left(-\frac{3}{5}\right) = 2.2143 $$

This angle is in the second quadrant and so we can use either $-2.2143$ or
$2\pi - 2.2143 = 4.0689$ for the second angle. As usual for these notes we'll
use the positive one. Therefore the two angles are,

$$ 2x - 1 = 2.2143 + 2\pi n \text{, } \quad n = 0, \pm 1, \pm 2, \dots $$

$$ 2x - 1 = 4.0689 + 2\pi n \text{, } \quad n = 0, \pm 1, \pm 2, \dots $$

Now, we still need to find the actual values of $x$ that are the solutions.
These are found in the same manner as all the problems above. We’ll first add
$1$ to both sides and then divide by $2$. Doing this gives,

$$ x = 1.6072 + \pi n \text{, } \quad n = 0, \pm 1, \pm 2, \dots $$

$$ x = 2.5345 + \pi n \text{, } \quad n = 0, \pm 1, \pm 2, \dots $$

---

So, in this example we saw an argument that was a little different from those
seen previously, but not all that different when it comes to working the
problems so don’t get too excited about it.

We now need to move into a different type of trig equation. All of the trig
equations solved to this point (the previous example as well as the previous
section) were, in some way, more or less the “standard” trig equation that is
usually solved in a trig class. There are other types of equations involving
trig functions however that we need to take a quick look at. The remaining
examples show some of these different kinds of trig equations.

---

**Example 2** Solve $2\cos(6y) + 11\cos(6y)\sin(3y) = 0$.

**Solution**

So, this definitely doesn’t look like any of the equations we’ve solved to this
point and initially the process is different as well. First, notice that there
is a $\cos(6y)$ in each term, so let’s factor that out and see what we have.

$$ \cos(6y)(2 + 11\sin(3y)) = 0 $$

We now have a product of two terms that is zero and so we know that we must
have,

$$ \cos(6y) = 0 \quad \text{ OR } \quad 2 + 11\sin(3y) = 0 $$

Now, at this point we have two trig equations to solve and each is identical to
the type of equation we were solving earlier. Because of this we won’t put in
much detail about solving these two equations.

First, solving $\cos(6y) = 0$ gives,

$$ 6y = \frac{\pi}{2} + 2\pi n \quad \Rightarrow \quad y = \frac{\pi}{12} + \frac{\pi n}{3} \text{, } \quad n = 0, \pm 1, \pm 2, \dots $$

$$ 6y = \frac{3\pi}{2} + 2\pi n \quad \Rightarrow \quad y = \frac{\pi}{4} + \frac{\pi n}{3} \quad n = 0, \pm 1, \pm 2, \dots $$

Next, solving $2 + 11\sin(3y) = 0$ gives,

$$ 3y = 6.1004 + 2\pi n \quad \Rightarrow \quad y = 2.0335 + \frac{2\pi n}{3} \text{, } \quad n = 0, \pm 1, \pm 2, \dots $$

$$ 3y = 3.3244+ 2\pi n \quad \Rightarrow \quad y = 1.1081 + \frac{2\pi n}{3} \text{, } \quad n = 0, \pm 1, \pm 2, \dots $$

Remember that in these notes we tend to take positive angles and so the first
solution here is in fact $2\pi - 0.1828$ where our calculator gave us $-0.1828$
as the answer when using the inverse sine function.

The solutions to this equation are then,

$$ y = \frac{\pi}{12} + \frac{\pi n}{3} \text{, } \quad n = 0, \pm 1, \pm 2, \dots $$

$$ y = \frac{\pi}{4} + \frac{\pi n}{3} \text{, } \quad n = 0, \pm 1, \pm 2, \dots $$

$$ y = 2.0335 + \frac{2\pi n}{3} \text{, } \quad n = 0, \pm 1, \pm 2, \dots $$

$$ y = 1.1081 + \frac{2\pi n}{3} \text{, } \quad n = 0, \pm 1, \pm 2, \dots $$

---

This next example also involves “factoring” trig equations but in a slightly
different manner than the previous example.

---

**Example 3** Solve
$4\sin^2\left(\dfrac{t}{3}\right) - 3\sin\left(\dfrac{t}{3}\right) = 1$.

**Solution**

Before solving this equation let’s solve an apparently unrelated equation.

$$ 4x^2 - 3x = 1 \quad \Rightarrow \quad 4x^2 - 3x - 1 = (4x + 1)(x - 1) = 0 \quad \Rightarrow \quad x = -\frac{1}{4},1 $$

This is an easy (or at least we hope it’s easy at this point) equation to solve.
The obvious question then is, why did we do this? Well, if you compare the two
equations you’ll see that the only real difference is that the one we just
solved has an $x$ everywhere and the equation we want to solve has a sine. What
this tells us is that we can work the two equations in exactly the same way.

We will first “factor” the equation as follows,

$$ 4\sin^{2}\left(\frac{t}{3}\right) - 3\sin\left(\frac{t}{3}\right) - 1 =  \left(4\sin\left(\frac{t}{3}\right) + 1\right)\left(\sin\left(\frac{5}{3}\right) - 1\right) = 0 $$

Now, set each of the two factors equal to zero and solve for the sine,

$$ \sin\left(\frac{t}{3}\right) = -\frac{1}{4} \quad \sin\left(\frac{t}{3}\right) = 1 $$

We now have two trig equations that we can easily (hopefully…) solve at this
point. We’ll leave the details to you to verify that the solutions to each of
these and hence the solutions to the original equation are,

$$ t = 18.0915 + 6\pi n \text{, } \quad n = 0, \pm 1, \pm 2, \dots $$

$$ t = 10.1829 + 6\pi n \text{, } \quad n = 0, \pm 1, \pm 2, \dots $$

$$ t = \frac{3\pi}{2} + 6\pi n \text{, } \quad n = 0, \pm 1, \pm 2, \dots $$

The first two solutions are from the first equation and the third solution is
from the second equation.

---

Let’s work one more trig equation that involves solving a quadratic equation.
However, this time, unlike the previous example this one won’t factor and so
we’ll need to use the quadratic formula.

---

**Example 4** Solve $8\cos^{2}(1 - x) + 13\cos(1 - x) - 5 = 0$.

**Solution**

Now, as mentioned prior to starting the example this quadratic does not factor.
However, that doesn’t mean all is lost. We can solve the following equation with
the quadratic formula (you do
[remember](https://tutorial.math.lamar.edu/Classes/Alg/SolveQuadraticEqnsII.aspx#Solve_QuadII_QuadFormula)
this and how to use it right?),

$$ 8t^2 + 13t - 5 = 0 \quad \Rightarrow \quad t = \frac{-13 \pm \sqrt{329}}{16} = 0.3211, -1.9461 $$

So, if we can use the quadratic formula on this then we can also use it on the
equation we’re asked to solve. Doing this gives us,

$$ \cos(1 - x) = 0.3211 \quad \text{ OR } \quad \cos(1 - x) = -1.9461 $$

Now, recall
[Example 9](https://tutorial.math.lamar.edu/Classes/CalcI/TrigEquations_CalcI.aspx#Rev_TrigEqnCalc_Ex9)
from the previous section. In that example we noted that
$-1 \leq \cos(\theta) \leq 1$ and so the second equation will have no solutions.
Therefore, the solutions to the first equation will yield the only solutions to
our original equation. Solving this gives the following set of solutions,

$$ x = -0.2439 - 2\pi n \text{, } \quad n = 0, \pm 1, \pm 2, \dots $$

$$ x = -4.0393 - 2\pi n \text{, } \quad n = 0, \pm 1, \pm 2, \dots $$

Note that we did get some negative numbers here and that does seem to violate
the general form that we’ve been using in most of these examples. However, in
this case the "-" are coming about when we solved for $x$ after computing the
inverse cosine in our calculator.

---

There is one more example in this section that we need to work that illustrates
another way in which factoring can arise in solving trig equations. This
equation is also the only one where the variable appears both inside and outside
of the trig equation. Not all equations in this form can be easily solved,
however some can so we want to do a quick example of one.

---

**Example 5** Solve $5x\tan(8x) = 3x$.

**Solution**

First, before we even start solving we need to make one thing clear. **DO NOT
CANCEL AN $x$ FROM BOTH SIDES!!!** While this may seem like a natural thing to
do it **WILL** cause us to lose a solution here.

So, to solve this equation we’ll first get all the terms on one side of the
equation and then factor an $x$ out of the equation. If we can cancel an $x$
from all terms then it can be factored out. Doing this gives,

$$ 5x\tan(8x) - 3x = x(5\tan(8x) - 3) = 0 $$

Upon factoring we can see that we must have either,

$$ x = 0 \quad \text{ OR } \quad \tan(8x) = \frac{3}{5} $$

Note that if we’d canceled the $x$ we would have missed the first solution. Now,
we solved an equation with a tangent in it in
[Example 5](https://tutorial.math.lamar.edu/Classes/CalcI/TrigEquations_CalcI.aspx#Rev_TrigEqnCalc_Ex5)
of the previous section so we’ll not go into the details of this solution here.
Here is the solution to the trig equation.

$$ x = 0.0676 + \frac{\pi n}{4} \text{, } \quad n = 0, \pm 1, \pm 2, \dots $$

$$ x = 0.4603 + \frac{\pi n}{4} \text{, } \quad n = 0, \pm 1, \pm 2, \dots $$

The complete set of solutions then to the original equation are,

$$ x = 0 \text{, } \quad n = 0, \pm 1, \pm 2, \dots $$

$$ x = 0.0676 + \frac{\pi n}{4} \text{, } \quad n = 0, \pm 1, \pm 2, \dots $$

$$ x = 0.4603 + \frac{\pi n}{4} \text{, } \quad n = 0, \pm 1, \pm 2, \dots $$

---

## Practice Problems

Find the solution(s) to the following equations. If an interval is given find
only those solutions that are in the interval. If no interval is given find all
solutions to the equation. These will require the use of a calculator so use at
least $4$ decimal places in your work.

Find all the solution(s) to the following equations. These will require the use
of a calculator so use at least $4$ decimal places in your work.

**1.** $3 - 14\sin(12t + 7) = 13$

**Solution**

$$ 3 - 14\sin(12t + 7) = 13 $$

$$ -14\sin(12t + 7) = 10 $$

$$ \sin(12t + 7) = -\frac{5}{7} $$

Quadrants III and IV.

$$ \sin^{-1}\left(-\frac{5}{7}\right) = 12t + 7 $$

$$ 12t + 7 = -0.7956 $$

First angle as positive:

$$ 2\pi + (-0.7956) = 5.4876 $$

Second angle:

$$ \pi + 0.7956 = 3.9372 $$

Calculating final answer:

$$ 12t + 7 = 3.9372 + 2\pi n \text{, } \quad n = 0, \pm 1, \pm 2, \dots $$

$$ 12t + 7 = 5.4876 + 2\pi n \text{, } \quad n = 0, \pm 1, \pm 2, \dots $$

$$ 12t = -3.0628 + 2\pi n \text{, } \quad n = 0, \pm 1, \pm 2, \dots $$

$$ 12t = -1.5124 + 2\pi n \text{, } \quad n = 0, \pm 1, \pm 2, \dots $$

Answers:

$$ \boxed{t = -0.2552 + \frac{\pi n}{6} \text{, } \quad n = 0, \pm 1, \pm 2, \dots} $$

$$ \boxed{t = -0.1260 + \frac{\pi n}{6} \text{, } \quad n = 0, \pm 1, \pm 2, \dots} $$

**2.** $3\sec(4 - 9z) - 24 = 0$

**Solution**

$$ 3\sec(4 - 9z) - 24 = 0 $$

$$ 3\sec(4 - 9z) = 24 $$

$$ \sec(4 - 9z) = 8 $$

$$ \cos(4 - 9z) = \frac{1}{8} $$

Quadrants I and IV.

$$ \cos^{-1}\left(\frac{1}{8}\right) = 4 - 9z $$

$$ 4 - 9z = 1.4455  $$

Second Angle:

$$ 2\pi - 1.4455 = 4.8377 $$

Calculating Answer:

$$ 4 - 9z = 1.4455 + 2\pi n \text{, } \quad n = 0, \pm 1, \pm 2, \dots $$

$$ 4 - 9z = 4.8377 + 2\pi n \text{, } \quad n = 0, \pm 1, \pm 2, \dots $$

$$ -9z = -2.5545 + 2\pi n \text{, } \quad n = 0, \pm 1, \pm 2, \dots $$

$$ -9z = 0.8377 + 2\pi n \text{, } \quad n = 0, \pm 1, \pm 2, \dots $$

Answers:

$$ z = 0.2838 - \frac{2\pi n}{9} \text{, } \quad n = 0, \pm 1, \pm 2, \dots $$

$$ z = -0.0931 - \frac{2\pi n}{9} \text{, } \quad n = 0, \pm 1, \pm 2, \dots $$

**3.** $4\sin(x + 2) - 15\sin(x + 2)\tan(4x) = 0$

**Solution**

$$ 4\sin(x + 2) - 15\sin(x + 2)\tan(4x) = 0 $$

$$ \sin(x + 2)(4 - 15\tan(4x)) = 0$$

$$ \sin(x + 2) = 0 $$

This Sine lies at $0$/$2\pi$ and also at $\pi$.

$$ \sin^{-1}(0) = x + 2 $$

$$ x + 2 = 0 $$

Find second angle:

$$ \pi + 0 = 3.1416 $$

$$ x + 2 = 3.1416 $$

$$ 4 - 15\tan(4x) = 0 $$

$$ -15\tan(4x) = -4 $$

$$ \tan(4x) = \frac{4}{15} $$

Quadrants I and III.

$$ \tan^{-1}\left(\frac{4}{15}\right) = 0.2606 $$

$$ 4x = 0.2606 $$

Second Angle:

$$ \pi + 0.2606 = 3.4022 $$

$$ 4x = 3.4022 $$

$$ x + 2 = 0 + 2\pi n \text{, } \quad n = 0, \pm 1, \pm 2, \dots $$

$$ x + 2 = 3.1416 + 2\pi n \text{, } \quad n = 0, \pm 1, \pm 2, \dots $$

$$ 4x = 0.2606 + 2\pi n \text{, } \quad n = 0, \pm 1, \pm 2, \dots $$

$$ 4x = 3.4022 + 2\pi n \text{, } \quad n = 0, \pm 1, \pm 2, \dots $$

Answers:

$$ \boxed{x = -2 + 2\pi n \text{, } \quad n = 0, \pm 1, \pm 2, \dots} $$

$$ \boxed{x = 1.1416 + 2\pi n \text{, } \quad n = 0, \pm 1, \pm 2, \dots} $$

$$ \boxed{x = 0.0652 + \frac{\pi n}{2} \text{, } \quad n = 0, \pm 1, \pm 2, \dots} $$

$$ \boxed{x = 0.8506 + \frac{\pi n}{2} \text{, } \quad n = 0, \pm 1, \pm 2, \dots} $$

**4.**
$3\cos\left(\dfrac{3y}{7}\right)\sin\left(\dfrac{y}{2}\right) + 14\cos\left(\dfrac{3y}{7}\right) = 0$

**Solution**

$$ 3\cos\left(\dfrac{3y}{7}\right)\sin\left(\dfrac{y}{2}\right) + 14\cos\left(\dfrac{3y}{7}\right) = 0 $$

$$ \cos\left(\frac{3y}{7}\right)\left(3\sin\left(\frac{y}{2}\right) + 14\right) = 0 $$

$$ \cos\left(\frac{3y}{7}\right) = 0 $$

Lies on axes. At Angles $\dfrac{\pi}{2}$ and $\dfrac{3\pi}{2}$.

$$ \cos^{-1}(0) = \frac{3y}{7} $$

$$ \frac{3y}{7} = \frac{\pi}{2} $$

$$ \frac{3y}{7} = \frac{3\pi}{2} $$

$$ 3\sin\left(\frac{y}{2}\right) + 14 = 0 $$

$$ 3\sin\left(\frac{y}{2}\right) = -14 $$

$$ \sin\left(\frac{y}{2}\right) = -\frac{14}{3} $$

$$ -1 \leq \sin\theta \leq 1 $$

$$ \sin\left(\frac{y}{2}\right) < -1 $$

No solution set from this factor. Moving on...

$$ \frac{3y}{7} = \frac{\pi}{2} + 2\pi n \text{, } \quad n = 0, \pm 1, \pm 2, \dots $$

$$ \frac{3y}{7} = \frac{3\pi}{2} + 2\pi n \text{, } \quad n = 0, \pm 1, \pm 2, \dots $$

But this can be further reduced to a single answer where occurrences are at
every $\pi$:

$$ \frac{3y}{7} = \frac{\pi}{2} + \pi n \text{, } \quad n = 0, \pm 1, \pm 2, \dots $$

$$ 3y = \frac{7\pi}{2} + 7\pi n \text{, } \quad n = 0, \pm 1, \pm 2, \dots $$

Answer:

$$ \boxed{y = \frac{7\pi}{6} + \frac{7\pi n}{3} \text{, } \quad n = 0, \pm 1, \pm 2, \dots} $$

**5.** $7\cos^{2}(3x) - \cos(3x) = 0$

**Solution**

$$ 7\cos^{2}(3x) - \cos(3x) = 0 $$

$$ \cos(3x)(7\cos(3x) - 1) = 0 $$

$$ \cos(3x) = 0 $$

Occurrences at $\dfrac{\pi}{2}$ and $\dfrac{3\pi}{2}$.

$$ \cos^{-1}(0) = 3x $$

$$ 3x = \frac{\pi}{2} + 2\pi n \text{, } \quad n = 0, \pm 1, \pm 2, \dots $$

$$ 3x = \frac{3\pi}{2} + 2\pi n \text{, } \quad n = 0, \pm 1, \pm 2, \dots $$

Further reduced to:

$$ 3x = \frac{\pi}{2} + \pi n \text{, } \quad n = 0, \pm 1, \pm 2, \dots $$

$$ 7\cos(3x) - 1 = 0 $$

$$ 7\cos(3x) = 1 $$

$$ \cos(3x) = \frac{1}{7} $$

Quadrants I and IV.

$$ \cos^{-1}\left(\frac{1}{7}\right) = 3x $$

$$ 3x = 1.4274 $$

Second angle:

$$ 3x = 2\pi - 1.4274  $$

$$ 3x = 4.8558 $$

Three answers not yet fully calculated are:

$$ 3x = \frac{\pi}{2} + \pi n \text{, } \quad n = 0, \pm 1, \pm 2, \dots $$

$$ 3x = 1.4274 + 2\pi n \text{, } \quad n = 0, \pm 1, \pm 2, \dots $$

$$ 3x = 4.8558 + 2\pi n \text{, } \quad n = 0, \pm 1, \pm 2, \dots $$

Answers:

$$ \boxed{x = \frac{\pi}{6} + \frac{\pi n}{3} \text{, } \quad n = 0, \pm 1, \pm 2, \dots} $$

$$ \boxed{x = 0.4758 + \frac{2\pi n}{3} \text{, } \quad n = 0, \pm 1, \pm 2, \dots} $$

$$ \boxed{x = 1.6186 + \frac{2\pi n}{3} \text{, } \quad n = 0, \pm 1, \pm 2, \dots} $$

**6.** $\tan^{2}\left(\dfrac{w}{4}\right) = \tan\left(\dfrac{w}{4}\right) + 12$

**Solution**

$$ \tan^{2}\left(\dfrac{w}{4}\right) = \tan\left(\dfrac{w}{4}\right) + 12 $$

$$ \tan^{2}\left(\dfrac{w}{4}\right) - \tan\left(\dfrac{w}{4}\right) - 12 = 0 $$

$$ \left(\tan\left(\frac{w}{4}\right) - 4\right)\left(\tan\left(\frac{w}{4}\right) + 3 \right) = 0 $$

$$ \tan\left(\frac{w}{4}\right) - 4 = 0 $$

$$ \tan\left(\frac{w}{4}\right) = 4 $$

Quandrants I and III.

$$ \tan^{-1}(4) = \frac{w}{4} $$

$$ \frac{w}{4} = 1.3258 $$

Find second angle:

$$ 1.3258 + \pi = 4.4674 $$

$$ \frac{w}{4} = 4.4674 $$

$$ \tan\left(\frac{w}{4}\right) + 3 = 0 $$

$$ \tan\left(\frac{w}{4}\right) = -3 $$

Quandrants II and IV.

$$ \tan^{-1}(-3) = \frac{w}{4} $$

$$ \frac{w}{4} = -1.2490 $$

Find positive angle:

$$ 2\pi + (-1.2490) = 5.0342 $$

$$ \frac{w}{4} = 5.0342 $$

Find second angle:

$$ 5.0342 - \pi = 1.8926 $$

$$ \frac{w}{4} = 1.8926 $$

Four answers thus far are:

$$ \frac{w}{4} = 1.3258 + 2\pi n \text{, } \quad n = 0, \pm 1, \pm 2, \dots $$

$$ \frac{w}{4} = 4.4674 + 2\pi n \text{, } \quad n = 0, \pm 1, \pm 2, \dots $$

$$ \frac{w}{4} = 5.0342 + 2\pi n \text{, } \quad n = 0, \pm 1, \pm 2, \dots $$

$$ \frac{w}{4} = 1.8926 + 2\pi n \text{, } \quad n = 0, \pm 1, \pm 2, \dots $$

Answers:

$$ \boxed{w = 5.3032 + 8\pi n \text{, } \quad n = 0, \pm 1, \pm 2, \dots} $$

$$ \boxed{w = 17.8696 + 8\pi n \text{, } \quad n = 0, \pm 1, \pm 2, \dots} $$

$$ \boxed{w = 20.1368 + 8\pi n \text{, } \quad n = 0, \pm 1, \pm 2, \dots} $$

$$ \boxed{w = 7.5704 + 8\pi n \text{, } \quad n = 0, \pm 1, \pm 2, \dots} $$

**7.** $4\csc^{2}(1 - t) + 6 = 25\csc(1 - t)$

**Solution**

$$ 4\csc^{2}(1 - t) + 6 = 25\csc(1 - t) $$

$$ 4\csc^{2}(1 - t) - 25\csc(1 - t) + 6 = 0 $$

Substitute:

$$ x = \csc(1 - t) $$

$$ 4x^2 - 25x + 6 = 0 $$

Quadratic Formula:

$$ x = \frac{-(-25) \pm \sqrt{(-25)^2 - 4(4)(6)}}{2(4)} $$

$$ x = \frac{25 \pm 23}{8} $$

$$ x = \frac{25 + 23}{8} $$

$$ x = 6 $$

$$ x = \frac{25 - 23}{8} $$

$$ x = \frac{1}{4} $$

Resubstitute back in cosecant:

$$ \csc(1 - t) = 6 $$

$$ \csc(1 - t) = \frac{1}{4} $$

Substitute cosecant for sine:

$$ \sin(1 - t) = \frac{1}{6} $$

$$ \sin(1 - t) = 4 $$

Evaluate:

$$ \sin(1 - t) = \frac{1}{6} $$

Quandrants I and II.

$$ \sin^{-1}\left(\frac{1}{6}\right) = 1 - t $$

$$ 1 - t = 0.1674 $$

Find second angle:

$$ 1 - t = \pi - 0.1674 $$

$$ 1 - t = 2.9742 $$

Evaluate:

$$ \sin(1 - t) = 4 $$

$$ -1 \leq \sin\theta \leq 1 $$

$$ \sin(1 - t) > 1 $$

No real answers for this factor.

Our two answers prior to evaluating are:

$$ 1 - t = 0.1674 + 2\pi n \text{, } \quad n = 0, \pm 1, \pm 2, \dots $$

$$ 1 - t = 2.9742 + 2\pi n \text{, } \quad n = 0, \pm 1, \pm 2, \dots $$

Further evaluating:

$$ -t = -0.8326 + 2\pi n \text{, } \quad n = 0, \pm 1, \pm 2, \dots $$

$$ -t = 1.9742 + 2\pi n \text{, } \quad n = 0, \pm 1, \pm 2, \dots $$

Answers:

$$ \boxed{t = 0.8326 - 2\pi n \text{, } \quad n = 0, \pm 1, \pm 2, \dots} $$

$$ \boxed{t = -1.9742 - 2\pi n \text{, } \quad n = 0, \pm 1, \pm 2, \dots} $$

**8.** $4y\sec(7y) = -21y$

**Solution**

$$ 4y\sec(7y) = -21y $$

$$ 4y\sec(7y) + 21y = 0 $$

$$ y(4\sec(7y) + 21) = 0 $$

$$ y = 0 $$

$$ 4\sec(7y) + 21 = 0 $$

$$ 4\sec(7y) = -21 $$

$$ \sec(7y) = -\frac{21}{4} $$

$$ \cos(7y) = -\frac{4}{21} $$

Quandrants II and III.

$$ \cos^{-1}\left(-\frac{4}{21}\right) = 7y $$

$$ 7y = 1.7624 $$

Second angle:

$$ 7y = 2\pi - 1.7624 $$

$$ 7y = 4.5208 $$

Our three answers not fully evaluated are:

$$ y = 0 $$

$$ 7y = 1.7624 + 2\pi n \text{, } \quad n = 0, \pm 1, \pm 2, \dots $$

$$ 7y = 4.5208 + 2\pi n \text{, } \quad n = 0, \pm 1, \pm 2, \dots $$

Answers:

$$ \boxed{y = 0} $$

$$ \boxed{y = 0.2518 + \frac{2\pi n}{7} \text{, } \quad n = 0, \pm 1, \pm 2, \dots} $$

$$ \boxed{y = 0.6458 + \frac{2\pi n}{7} \text{, } \quad n = 0, \pm 1, \pm 2, \dots} $$

**9.** $10x^2\sin(3x + 2) = 7x\sin(3x + 2)$

**Solution**

$$ 10x^2\sin(3x + 2) = 7x\sin(3x + 2) $$

$$ 10x^2\sin(3x + 2) - 7x\sin(3x + 2) = 0 $$

$$ x\sin(3x + 2)(10x - 7) = 0 $$

Our three factors are:

$$ x = 0 $$

$$ \sin(3x + 2) = 0 $$

$$ 10x - 7 = 0 $$

Evalute the last one for simplicity:

$$ 10x = 7 $$

$$ x = \frac{7}{10} $$

Evaluate sine:

$$ \sin(3x + 2) = 0 $$

Lies on $0$/$2\pi$ and $\pi$.

$$ \sin^{-1}(0) = 3x + 2  $$

$$ 3x + 2 = 0 $$

Second angle

$$ 3x + 2 = \pi $$

When further simplified, this means:

$$ 3x + 2 = \pi n \text{, } \quad n = 0, \pm 1, \pm 2, \dots $$

Further evaluated:

$$ 3x = \pi n - 2 \text{, } \quad n = 0, \pm 1, \pm 2, \dots $$

$$ x = \frac{\pi n - 2}{3} \text{, } \quad n = 0, \pm 1, \pm 2, \dots $$

$$ x = \frac{\pi n}{3} - \frac{2}{3} \text{, } \quad n = 0, \pm 1, \pm 2, \dots $$

Answers:

$$ \boxed{x = 0} $$

$$ \boxed{x = \frac{7}{10}} $$

$$ \boxed{x = \frac{\pi n}{3} - \frac{2}{3} \text{, } \quad n = 0, \pm 1, \pm 2, \dots} $$

**10.** $(2t - 3)\tan\left(\dfrac{6t}{11}\right) = 15 - 10t$

**Solution**

$$ (2t - 3)\tan\left(\dfrac{6t}{11}\right) = 15 - 10t $$

$$ (2t - 3)\tan\left(\dfrac{6t}{11}\right) = -5(2t - 3) $$

$$ \tan\left(\dfrac{6t}{11}\right) = -5 $$

Quadrants II and IV.

$$ \tan^{-1}(-5) = \frac{6t}{11} $$

$$ \frac{6t}{11} = -1.3734 $$

Positive first angle:

$$ 2\pi + (-1.3734) = 4.9098 $$

$$ \frac{6t}{11} = 4.9098 $$

Second angle:

$$ 4.9098 - \pi = 1.7682 $$

$$ \frac{6t}{11} = 1.7682 $$

Our two answers prior to evaluation are:

$$ \frac{6t}{11} = 4.9098 + 2\pi n \text{, } \quad n = 0, \pm 1, \pm 2, \dots $$

$$ \frac{6t}{11} = 1.7682 + 2\pi n \text{, } \quad n = 0, \pm 1, \pm 2, \dots $$

Further evaluation:

$$ 6t = 54.0078 + 22\pi n \text{, } \quad n = 0, \pm 1, \pm 2, \dots $$

$$ 6t = 19.4502 + 22\pi n \text{, } \quad n = 0, \pm 1, \pm 2, \dots $$

Answers:

$$ \boxed{t = 9.0013 + \frac{11\pi n}{3} \text{, } \quad n = 0, \pm 1, \pm 2, \dots} $$

$$ \boxed{t = 3.2417 + \frac{11\pi n}{3} \text{, } \quad n = 0, \pm 1, \pm 2, \dots} $$

---

## Assignment Problems

Find all the solution(s) to the following equations. These will require the use
of a calculator so use at least $4$ decimal places in your work.

**1.** $22\cos(8 - x) + 10 = 0$

**Solution**

**2.** $10\tan(4x + 10) - 7 = 31$

**Solution**

**3.**
$4\tan\left(\dfrac{w}{3}\right)\sin(2w) - \tan\left(\dfrac{w}{3}\right) = 0$

**Solution**

**4.** $3\tan(4z)\sec(2z - 1) + \sec(2z - 1) = 0$

**Solution**

**5.** $2 - \sin(2y) = 3\sin^{2}(2y)$

**Solution**

**6.** $4\cos^{2}(2t + 5) - 4\cos(2t + 5) = -1$

**Solution**

**7.** $6 - 5\sin^{2}\left(\dfrac{x}{4}\right) = 7\sin\left(\dfrac{x}{4}\right)$

**Solution**

**8.** $2 = 2\tan^{2}(8t) + 3\tan(8t)$

**Solution**

**9.** $35\csc(4z) = z^3\csc(4z)$

**Solution**

**10.** $3t = 8t \cos(5 + t)$

**Solution**

**11.** $(5x + 1)\sin\left(\dfrac{x - 6}{2}\right) + 25x + 5 = 0$

**Solution**
