# Section 1.9 : Exponential And Logarithm Equations

In this section we’ll take a look at solving equations with exponential
functions or logarithms in them.

We’ll start with equations that involve exponential functions. The main property
that we’ll need for these equations is,

$$ \log_{b}b^x = x $$

---

**Example 1** Solve $7 + 15\mathbf{e}^{1 - 3z} = 10$.

**Solution**

The first step is to get the exponential all by itself on one side of the
equation with a coefficient of one.

$$ 7 + 15\mathbf{e}^{1 - 3z} = 10 $$

$$ 15\mathbf{e}^{1 - 3z} = 3 $$

$$ \mathbf{e}^{1 - 3z} = \frac{1}{5} $$

Now, we need to get the $z$ out of the exponent so we can solve for it. To do
this we will use the property above. Since we have an $\mathbf{e}$ in the
equation we’ll use the natural logarithm. First, we take the logarithm of both
sides and then use the property to simplify the equation.

$$ \ln(\mathbf{e}^{1 - 3z}) = \ln\left(\frac{1}{5}\right) $$

$$ 1 - 3z = \ln\left(\frac{1}{5}\right) $$

All we need to do now is solve this equation for $z$.

$$ 1 - 3z = \ln\left(\frac{1}{5}\right) $$

$$ -3z = -1 + \ln\left(\frac{1}{5}\right) $$

$$ z = -\frac{1}{3}\left(-1 + \ln\left(\frac{1}{5}\right)\right) = 0.8698126372 $$

---

**Example 2** Solve $10^{t^2 - t} = 100$.

**Solution**

Now, in this case it looks like the best logarithm to use is the common
logarithm since left hand side has a base of $10$. There’s no initial
simplification to do, so just take the log of both sides and simplify.

$$ \log 10^{t^2 - t} = \log 100 = \log 10^2 = 2 $$

$$ t^2 - t = 2 $$

At this point, we’ve just got a quadratic that can be solved

$$ t^2 - t - 2 = 0 $$

$$ (t - 2)(t + 1) = 0 $$

So, it looks like the solutions in this case are $t = 2$ and $t = -1$.

---

Now that we’ve seen a couple of equations where the variable only appears in the
exponent we need to see an example with variables both in the exponent and out
of it.

---

**Example 3** Solve $x - x\mathbf{e}^{5x + 2} = 0$.

The first step is to factor an $x$ out of both terms.

**DO NOT DIVIDE AN $x$ FROM BOTH TERMS!!!!**

Note that it is very tempting to “simplify” the equation by dividing an $x$ out
of both terms. However, if you do that you’ll miss a solution as we’ll see.

$$ x - x\mathbf{e}^{5x + 2} = 0 $$

$$ x(1 - \mathbf{e}^{5x + 2}) = 0 $$

So, it’s now a little easier to deal with. From this we can see that we get one
of two possibilities.

$$ x = 0 \quad \quad \text{ OR } \quad \quad 1 - \mathbf{e}^{5x + 2} = 0 $$

The first possibility has nothing more to do, except notice that if we had
divided both sides by an $x$ we would have missed this one so be careful. In the
second possibility we’ve got a little more to do. This is an equation similar to
the first two that we did in this section.

$$ \mathbf{e}^{5x + 2} = 1 $$

$$ 5x + 2 = \ln 1 $$

$$ 5x + 2 = 0 $$

$$ x = -\frac{2}{5} $$

Don't forget that $\ln 1 = 0$.

So, the two solutions are $x = 0$ and $x = -\dfrac{2}{5}$.

---

The next equation is a more complicated (looking at least…) example similar to
the previous one.

---

**Example 4** Solve $5(x^2 - 4) = (x^2 - 4)\mathbf{e}^{7 - x}$.

**Solution**

As with the previous problem do NOT divide an $x^2 − 4$ out of both sides. Doing
this will lose solutions even though it “simplifies” the equation. Note however,
that if you can divide a term out then you can also factor it out if the
equation is written properly.

So, the first step here is to move everything to one side of the equation and
then to factor out the $x^2 − 4$.

$$ 5(x^2 - 4) - (x^2 - 4)\mathbf{e}^{7 - x} = 0 $$

$$ (x^2 - 4)(5 - \mathbf{e}^{7 - x}) = 0 $$

At this point all we need to do is set each factor equal to zero and solve each.

$$ x^2 - 4 = 0 \quad \quad \quad \quad 5 - \mathbf{e}^{7 - x} = 0 $$

$$ x = \pm 2 \quad \quad \quad \quad \mathbf{e}^{7 - x} = 5 $$

$$ x = \pm 2 \quad \quad \quad \quad 7 - x = \ln(5) $$

$$ x = \pm 2 \quad \quad \quad \quad x = 7 - \ln(5) = 5.390562088 $$

The three solutions are then $x = \pm 2$ and $x = 5.3906$.

---

As a final example let’s take a look at an equation that contains two different
exponentials.

---

**Example 5** Solve $4\mathbf{e}^{1 + 3x} - 9\mathbf{e}^{5 - 2x} = 0$.

**Solution**

The first step here is to get one exponential on each side and then we’ll divide
both sides by one of them (which doesn’t matter for the most part) so we’ll have
a quotient of two exponentials. The quotient can then be simplified and we’ll
finally get both coefficients on the other side. Doing all of this gives,

$$ 4\mathbf{e}^{1 + 3x} = 9\mathbf{e}^{5 - 2x} $$

$$ \frac{\mathbf{e}^{1 + 3x}}{\mathbf{e}^{5 - 2x}} = \frac{9}{4} $$

$$ \mathbf{e}^{1 + 3x - (5 - 2x)} = \frac{9}{4} $$

$$ \mathbf{e}^{5x - 4} = \frac{9}{4} $$

Note that while we said that it doesn’t really matter which exponential we
divide out by doing it the way we did here we’ll avoid a negative coefficient on
the $x$. Not a major issue, but those minus signs on coefficients are really
easy to lose on occasion.

This is now in a form that we can deal with so here’s the rest of the solution.

$$ \mathbf{e}^{5x - 4} = \frac{9}{4} $$

$$ 5x - 4 = \ln\left(\frac{9}{4}\right) $$

$$ 5x = 4 + \ln\left(\frac{9}{4}\right) $$

$$ x = \frac{1}{5}\left(4 + \ln\left(\frac{9}{4}\right)\right) = 0.9621860432 $$

This equation has a single solution of $x = 0.9622$.

---

Now let’s take a look at some equations that involve logarithms. The main
property that we’ll be using to solve these kinds of equations is,

$$ b^{\log_{b}x} = x $$

---

**Example 6** Solve $3 + 2\ln\left(\dfrac{x}{7} + 3\right) = -4$.

**Solution**

This first step in this problem is to get the logarithm by itself on one side of
the equation with a coefficient of $1$.

$$ 2\ln\left(\frac{x}{7} + 3\right) = -7 $$

$$ \ln\left(\frac{x}{7} + 3\right) = -\frac{7}{2} $$

Now, we need to get the $x$ out of the logarithm and the best way to do that is
to “exponentiate” both sides using $\mathbf{e}$. In other words,

$$ \mathbf{e}^{\ln\left(\frac{x}{7} + 3\right)} = \mathbf{e}^{-\frac{7}{2}} $$

So, using the property above with $\mathbf{e}$, since there is a natural
logarithm in the equation, we get,

$$ \frac{x}{7} + 3 = \mathbf{e}^{-\frac{7}{2}} $$

Now all that we need to do is solve this for $x$.

$$ \frac{x}{7} + 3 = \mathbf{e}^{-\frac{7}{2}} $$

$$ \frac{x}{7} = -3 + \mathbf{e}^{-\frac{7}{2}} $$

$$ x = 7\left(-3 + \mathbf{e}^{-\frac{7}{2}}\right) = -20.78861832 $$

At this point we might be tempted to say that we’re done and move on. However,
we do need to be careful. Recall from the previous
[section](https://tutorial.math.lamar.edu/Classes/CalcI/LogFcns.aspx#Log_Prop)
that we can’t plug a negative number into a logarithm. This, by itself, doesn’t
mean that our answer won’t work since its negative. What we need to do is plug
it into the logarithm and make sure that $\dfrac{x}{7} + 3$ will not be
negative. I’ll leave it to you to verify that this is in fact positive upon
plugging our solution into the logarithm and so $x = −20.78861832$ is a solution
to the equation.

---

Let’s now take a look at a more complicated equation. Often there will be more
than one logarithm in the equation. When this happens we will need to use one or
more of the following properties to combine all the logarithms into a single
logarithm. Once this has been done we can proceed as we did in the previous
example.

$$ \log_{b}(xy) = \log_{b}(x) + \log_{b}(y) \quad \log_{b}\left(\frac{x}{y}\right) = \log_{b}(x) - \log_{b}(y) \quad \log_{b}(x^r) = r\log_{b}(x) $$

---

**Example 7** Solve $2\ln\left(\sqrt{7}\right) - \ln(1 - x) = 2$.

**Solution**

First get the two logarithms combined into a single logarithm.

$$ 2\ln\left(\sqrt{x}\right) - \ln(1 - x) = 2 $$

$$ \ln\left(\left(\sqrt{x}\right)^2\right) - \ln(1 - x) = 2 $$

$$ \ln(x) - \ln(1 - x) = 2 $$

$$ \ln\left(\frac{x}{1 - x}\right) = 2 $$

Now, exponentiate both sides and solve for $x$.

$$ \frac{x}{1 - x} = \mathbf{e}^2 $$

$$ x = \mathbf{e}^2(1 - x) $$

$$ x = \mathbf{e}^2 - \mathbf{e}^2x $$

$$ x(1 + \mathbf{e}^2) = \mathbf{e}^2 $$

$$ x = \frac{\mathbf{e}^2}{1 + \mathbf{e}^2} = 0.8807970780 $$

The solution work here was a little messy but this is work that you will need to
be able to do on occasion so make sure you can do it!

Finally, we just need to make sure that the solution, $x = 0.8807970780$,
doesn’t produce negative numbers in both of the original logarithms. It doesn’t,
so this is in fact our solution to this problem.

---

Let’s take a look at another example.

---

**Example 8** Solve $\log x + \log(x - 3) = 1$.

**Solution**

As with the last example, first combine the logarithms into a single logarithm.

$$ \log x + \log(x - 3) = 1 $$

$$ \log\left(x(x - 3)\right) = 1 $$

Now exponentiate, using $10$ this time instead of $\mathbf{e}$ because we've got
common logs in the equation, both sides.

$$ 10^{\log(x^2 - 3x)} = 10^1 $$

$$ x^2 - 3x = 10 $$

$$ x^2 - 3x - 10 = 0 $$

$$ (x - 5)(x + 2) = 0 $$

So, potentital solutions are $x = 5$ and $x = -2$. Note, however that if we plug
$x = -2$ into either of the two original logarithms we would get negative
numbers so this can't be a solution. We can however, use $x = 5$.

Therefore, the solution to this equation is $x = 5$.

---

When solving equations with logarithms it is important to check your potential
solutions to make sure that they don’t generate logarithms of negative numbers
or zero. It is also important to make sure that you do the checks in the
**original** equation. If you check them in the second logarithm above (after
we’ve combined the two logs) both solutions will appear to work! This is because
in combining the two logarithms we’ve actually changed the problem. In fact, it
is this change that introduces the extra solution that we couldn’t use!

Also, be careful in solving equations containing logarithms to not get locked
into the idea that you will get two potential solutions and only one of these
will work. It is possible to have problems where both are solutions and where
neither are solutions.

There is one more problem that we should work.

---

**Example 9** Solve $\ln(x - 2) + \ln(x + 1) = 2$.

**Solution**

The first step of this problem is the same as we’ve been doing up to this point.
So, let’s combine the logarithms.

$$ \ln\left((x - 2)(x + 1)\right) = 2 $$

$$ \ln(x^2 - x - 2) = 2 $$

Now we can exponentiate both sides with respect to $\mathbf{e}$ to eliminate the
logarithm. Doing this along with a little simplification gives,

$$ x^2 - x - 2 = \mathbf{e}^2 $$

$$ x^2 - x - 2 - \mathbf{e}^2 = 0 $$

We’ve reached the point of this problem. We need to solve this quadratic and
without the $\mathbf{e}^2$ everyone would be able to do that. However, with the
$\mathbf{e}^2$ people tend to decide that they can’t do it.

This is just a quadratic equation and everyone in this class should be able to
solve that. The only difference between this quadratic equation and those you
are probably used to seeing is that there are numbers in it that are not
integers, or at worst, fractions. In this case the constant in the quadratic is
just $-2 - \mathbf{e}^2$ and so all we need to do is use the quadratic formula
to get the solutions.

The solutions to this quadratic equation are,

$$ x = \frac{1 \pm \sqrt{1 - 4(1)(-2 - \mathbf{e}^2)}}{2} = \frac{1 \pm \sqrt{9 + 4\mathbf{e}^2}}{2} = -2.6047, 3.6047 $$

Do not get excited about the “messy” solutions to this quadratic. We will get
these kinds of solutions on occasion.

The last step to this problem is to check the two solutions to the quadratic
equation in the original equation. Doing that we can see that the first
solution, $-2.6047$, will give negative numbers in the logarithms and so can’t
be a solution. On the other hand, the second solution, $3.6047$, does not give
negative numbers in the logarithms and so is okay.

The solution to the original equation is $x = 3.6047$.

---

## Practice Problems

For problems 1 – 12 find all the solutions to the given equation. If there is no
solution to the equation clearly explain why.

**1.** $12 - 4\mathbf{e}^{7 + 3x} = 7$

**Solution**

**2.** $1 = 10 - 3\mathbf{e}^{z^2 - 2z}$

**Solution**

**3.** $2t - t\mathbf{e}^{6t - 1} = 0$

**Solution**

**4.** $4x + 1 = (12x + 3)\mathbf{e}^{x^2 - 2}$

**Solution**

**5.** $2\mathbf{e}^{3y + 8} - 11\mathbf{e}^{5 - 10y} = 0$

**Solution**

**6.** $14\mathbf{e}^{6 - x} + \mathbf{e}^{12x - 7} = 0$

**Solution**

**7.** $1 - 8\ln\left(\dfrac{2x - 1}{7}\right) = 14$

**Solution**

**8.** $\ln(y - 1) = 1 + \ln(3y + 2)$

**Solution**

**9.** $\log(w) + \log(w - 21) = 2$

**Solution**

**10.** $2\log(z) - \log(7z - 1) = 0$

**Solution**

**11.** $16 = 17^{t - 2} + 11$

**Solution**

**12.** $2^{3 - 8w} - 7 = 11$

**Solution**

---

> **Compound Interest.** If we put $P$ dollars into an account that earns
> interest at a rate of $r$ (written as a decimal as opposed to the standard
> percent) for $t$ years then,
>
> a. if interest is compounded $m$ times per year we will have,
>
> $$ A = P\left(1 + \frac{r}{m}\right)^{tm} $$
>
> dollars after $t$ years.
>
> b. if interest is compounded continuously we will have,
>
> $$ A = P\mathbf{e}^{rt} $$
>
> dollars after $t$ years.

**13.** We have $10,000 to invest for 44 months. How much money will we have if
we put the money into an account that has an annual interest rate of 5.5% and
interest is compounded

**(a)** quarterly

**Solution**

**(b)** monthly

**Solution**

**\(c\)** continuously

**Solution**

**14.** We are starting with $5000 and we're goint to put it into an account
that earns an annual interest rate of 12%. How long should we leave the money in
the account in order to double our money if interest is compounded

**(a)** quarterly

**Solution**

**(b)** monthly

**Solution**

**\(c\)** continuously

**Solution**

---

> **Exponential Growth/Decay** Many quantities inm the world can be modeled (at
> least for a short time) by the exponential growth/decay equation.
>
> $$ Q = Q_{0}\mathbf{e}^{kt} $$
>
> If $k$ is positive we will get exponential growth and if $k$ is negative we
> will get exponential decay.

**15.** A population of bacteria initially has 250 present and in 5 days there
will be 1600 bacteria present.

**(a)** Determine the exponential growth equation for this population.

**Solution**

**(b)** How long will it take for the population to grow from its initial
population of 250 to a population of 2000?

**Solution**

**16.** We initially have 100 grams of a radioactive element and in 1250 years
there will be 80 grams left.

**(a)** Determine the exponential decay equation for this element.

**Solution**

**(b)** How long will it take for half of the element to decay?

**Solution**

**\(c\)** How long will it take until there is only 1 gram of the element left?

**Solution**

---

## Assignment Problems

For problems 1 – 17 find all the solutions to the given equation. If there is no
solution to the equation clearly explain why.

**1.** $15 = 12 + 5\mathbf{e}^{10w - 7}$

**Solution**

**2.** $4\mathbf{e}^{2x + x^2} - 7 = 2$

**Solution**

**3.** $8 + 3\mathbf{e}^{4 - 9z} = 1$

**Solution**

**4.** $4t^2 - 3t^2\mathbf{e}^{2 - t} = 0$

**Solution**

**5.** $7x + 16x\mathbf{e}^{x^3 - 5x} = 0$

**Solution**

**6.** $3\mathbf{e}^{7t} - 12\mathbf{e}^{8t + 5} = 0$

**Solution**

**7.** $2y\mathbf{e}^{y^2} - 7y\mathbf{e}^{1 - 5y} = 0$

**Solution**

**8.** $16 + 4\ln(x + 2) = 7$

**Solution**

**9.** $3 - 11\ln\left(\frac{z}{3 - z}\right) = 1$

**Solution**

**10.** $2\log(w) - \log(3w + 7) = 1$

**Solution**

**11.** $\ln(3x + 1) - \ln(x) = -2$

**Solution**

**12.** $t\log(6t + 1) - 3t^2\log(6t + 1) = 0$

**Solution**

**13.** $2\log(z) - \log(z^2 + 4z + 1) = 0$

**Solution**

**14.** $\ln(x) + \ln(x - 2) = 3$

**Solution**

**15.** $11 - 5^{9w - 1} = 3$

**Solution**

**16.** $12 + 20^{7 - 2t} = 50$

**Solution**

**17.** $1 + 3^{z^2 - 2} = 5$

**Solution**

---

> **Compound Interest.** If we put $P$ dollars into an account that earns
> interest at a rate of $r$ (written as a decimal as opposed to the standard
> percent) for $t$ years then,
>
> a. if interest is compounded $m$ times per year we will have,
>
> $$ A = P\left(1 + \frac{r}{m}\right)^{tm} $$
>
> dollars after $t$ years.
>
> b. if interest is compounded continuously we will have,
>
> $$ A = P\mathbf{e}^{rt} $$
>
> dollars after $t$ years.

**18.** We have $2,500 to invest and 80 months. How much money will we have if
we put the money into an account that has an annual interest rate of 9% and
interest is compounded

**(a)** quarterly

**Solution**

**(b)** monthly

**Solution**

**\(c\)** continuously

**Solution**

**19.** We are starting with $60,000 and we’re going to put it into an account
that earns an annual interest rate of 7.5%. How long will it take for the money
in the account to reach $100,000 if the interest is compounded

**(a)** quarterly

**Solution**

**(b)** monthly

**Solution**

**\(c\)** continuously

**Solution**

**20.** Suppose that we put some money in an account that has an annual interest
rate of 10.25%. How long will it take to triple our money if the interest is
compounded

**(a)** quarterly

**Solution**

**(b)** monthly

**Solution**

**\(c\)** continuously

**Solution**

---

> **Exponential Growth/Decay** Many quantities inm the world can be modeled (at
> least for a short time) by the exponential growth/decay equation.
>
> $$ Q = Q_{0}\mathbf{e}^{kt} $$
>
> If $k$ is positive we will get exponential growth and if $k$ is negative we
> will get exponential decay.

**21.** A population of bacteria initially has 90,000 present and in 2 weeks
there will be 200,000 bacteria present.

**(a)** Determine the exponential growth equation for this population.

**Solution**

**(b)** How long will it take for the population to grow from its initial
population of 90,000 to a population of 150,000?

**Solution**

**22.** We initially have 2 kg grams of some radioactive element and in 7250
years there will be 1.5 kg left.

**(a)** Determine the exponential decay equation for this element.

**Solution**

**(b)** How long will it take for half of the element to decay?

**Solution**

**\(c\)** How long will it take until there is 250 grams of the element left?

**Solution**

**23.** For a particular radioactive element the value of $k$ in the exponential
decay equation is given by $k = 0.000825$.

**(a)** How long will it take for a quarter of the element to decay?

**Solution**

**(b)** How long will it take for half of the element to decay?

**Solution**

**\(c\)** How long will it take 90% of the element to decay?

**Solution**
